## Problem

Let $a, b, c \neq 0$ such that $a^2+b^2+c^2=2(ab+bc+ca)$. Find the largest constant $C$ such that the following inequality holds for all $a, b, c$ satisfying the given condition:
$$
(a+b+c)\left(\frac{1}{a}+\frac{1}{b}+\frac{1}{c}\right) \geq C
$$

## Query

Task description: Please solve the problem with clear, rigorous, and logically sound steps. At the end of your response, state your answer in exactly this format: 'The answer is $C=X$', where X is your calculated numerical bound value. Example: 'The answer is $C=1$'.

Problem: Let $a, b, c \neq 0$ such that $a^2+b^2+c^2=2(ab+bc+ca)$. Find the largest constant $C$ such that the following inequality holds for all $a, b, c$ satisfying the given condition:
$$
(a+b+c)\left(\frac{1}{a}+\frac{1}{b}+\frac{1}{c}\right) \geq C
$$

Solution:

## Response

To solve the problem, we need to analyze the condition given by \( a^2 + b^2 + c^2 = 2(ab + ac + bc) \). This indicates a certain relationship among \( a \), \( b \), and \( c \).

### Step 1: Simplifying the Condition

We rewrite the condition as follows:

\[
a^2 + b^2 + c^2 - 2(ab + ac + bc) = 0
\]

This can be expressed as:

\[
\frac{1}{2} \left((a-b)^2 + (b-c)^2 + (c-a)^2\right) = 0
\]

Thus, we conclude that \( a = b = c \).

### Step 2: Substituting into the Inequality

Assuming \( a = b = c \) (let \( a = b = c = k \) for some non-zero \( k \)), we substitute into the inequality:

\[
(3k)\left(\frac{1}{k} + \frac{1}{k} + \frac{1}{k}\right) \geq C
\]

This simplifies to:

\[
3k \cdot \frac{3}{k} = 9
\]

### Step 3: Finding \( C \)

From our derivations, we observe that for \( a = b = c \):

\[
9 \geq C
\]

Thus, the largest constant \( C \) such that the inequality holds for all \( a, b, c \) satisfying the original condition is:

\[
C = 9
\]

### Conclusion

Hence, we summarize our findings:

The answer is '"'"'The answer is $C=9$'"'"'.