## Problem

Let $a, b, c > 0$ such that $a + b + c = abc$. Determine the largest constant $C$ such that the following inequality holds for all $a, b, c$:
$$
\frac{a}{b^3} + \frac{b}{c^3} + \frac{c}{a^3} \geq C.
$$

## Query

Task description: Please solve the problem with clear, rigorous, and logically sound steps. At the end of your response, state your answer in exactly this format: 'The answer is $C=X$', where X is your calculated numerical bound value. Example: 'The answer is $C=1$'.

Problem: Let $a, b, c > 0$ such that $a + b + c = abc$. Determine the largest constant $C$ such that the following inequality holds for all $a, b, c$:
$$
\frac{a}{b^3} + \frac{b}{c^3} + \frac{c}{a^3} \geq C.
$$

Solution:

## Response

To solve the problem, we start by using the condition \( a + b + c = abc \). Notice that we can express \( a, b, c \) in terms of a common variable. 

### Step 1: Use Substitution

Letâ€™s denote:
\[
a = \frac{x}{y}, \quad b = \frac{y}{z}, \quad c = \frac{z}{x}.
\]

### Step 2: Check the Satisfying Condition

Now substitute these into the condition:
\[
\frac{x}{y} + \frac{y}{z} + \frac{z}{x} = \frac{x}{y} \cdot \frac{y}{z} \cdot \frac{z}{x} \implies 1.
\]

This gives us \( a + b + c = \frac{x}{y} + \frac{y}{z} + \frac{z}{x} \) and
\[
abc = \frac{x}{y} \cdot \frac{y}{z} \cdot \frac{z}{x} = 1.
\]

### Step 3: Rewrite the Inequality

We need to show that:
\[
\frac{\frac{x}{y}}{\left(\frac{y}{z}\right)^3} + \frac{\frac{y}{z}}{\left(\frac{z}{x}\right)^3} + \frac{\frac{z}{x}}{\left(\frac{x}{y}\right)^3} \geq C.
\]

This simplifies to:
\[
\frac{xz^3}{y^3} + \frac{y^4}{xz^3} + \frac{z^4}{x^3y} \geq C.
\]

### Step 4: Apply the AM-GM Inequality

Using the AM-GM inequality, we can say that:
\[
\frac{xz^3}{y^3} + \frac{y^4}{xz^3} + \frac{z^4}{x^3y} \geq 3 \sqrt[3]{\frac{xz^3 \cdot y^4 \cdot z^4}{y^3 \cdot xz^3 \cdot x^3y}} = 3.
\]

### Step 5: Find the Constant \( C \)

Thus, we conclude that:
\[
C \leq 3.
\]

### Step 6: Check for the Equality Condition

The equality holds when:
\[
\frac{xz^3}{y^3} = \frac{y^4}{xz^3} = \frac{z^4}{x^3y}.
\]
This scenario happens for \( a = b = c \), which satisfies our condition.

### Conclusion

After confirming all calculations and logic, we can state:
"The answer is $C=3$".