## Problem

Let $x$ and $y$ be two positive real numbers such that $x + y = 1$. Determine the largest constant $C$ such that the following inequality holds for all $x, y$:

$$
\left(1+\frac{1}{x}\right)\left(1+\frac{1}{y}\right) \geq C.
$$

## Query

Task description: Please solve the problem with clear, rigorous, and logically sound steps. At the end of your response, state your answer in exactly this format: 'The answer is $C=X$', where X is your calculated numerical bound value. Example: 'The answer is $C=1$'.

Problem: Let $x$ and $y$ be two positive real numbers such that $x + y = 1$. Determine the largest constant $C$ such that the following inequality holds for all $x, y$:

$$
\left(1+\frac{1}{x}\right)\left(1+\frac{1}{y}\right) \geq C.
$$

Solution:

## Response

To solve the problem of finding the largest constant \( C \) such that 

\[
\left(1+\frac{1}{x}\right)\left(1+\frac{1}{y}\right) \geq C
\]

holds for all positive \( x \) and \( y \) with the constraint \( x + y = 1 \), we will follow the steps outlined below.

### Step 1: Rewrite the Inequality

We start by expanding the left-hand side of the inequality:

\[
\left(1+\frac{1}{x}\right)\left(1+\frac{1}{y}\right) = 1 + \frac{1}{x} + \frac{1}{y} + \frac{1}{xy}
\]

### Step 2: Substitute the Constraint

Given \( y = 1 - x \), we can rewrite the terms involving \( y \):

\[
\frac{1}{y} = \frac{1}{1 - x}
\]

Then, substituting this into our expression gives:

\[
1 + \frac{1}{x} + \frac{1}{1 - x} + \frac{1}{x(1 - x)}
\]

### Step 3: Simplify the Expression

Now we simplify:

\[
= 1 + \frac{1}{x} + \frac{1}{1 - x} + \frac{1}{x(1 - x)}
\]

### Step 4: Analyze the Function Behavior

Let's denote \( f(x) = 1 + \frac{1}{x} + \frac{1}{1 - x} + \frac{1}{x(1 - x)} \).

We need to find the minimum of \( f(x) \) over the interval \( (0, 1) \). 

### Step 5: Calculate the Derivative

Calculating the derivative \( f'(x) \):

\[
f'(x) = -\frac{1}{x^2} + \frac{1}{(1 - x)^2} - \frac{1}{x^2(1-x)} + \frac{1}{(1-x)x^2} = -\frac{1}{x^2} + \frac{1}{(1-x)^2}
\]

Setting \( f'(x) = 0 \) gives:

\[
\frac{1}{(1-x)^2} = \frac{1}{x^2}
\]

Cross multiplying and simplifying results in:

\[
x^2 = (1 - x)^2
\]

This leads to:

\[
x = \frac{1}{2}
\]

### Step 6: Evaluate the Function at \(x = \frac{1}{2}\)

Now, substituting \( x = \frac{1}{2} \) back into \( f \):

\[
f\left(\frac{1}{2}\right) = 1 + \frac{1}{\frac{1}{2}} + \frac{1}{\frac{1}{2}} + \frac{1}{\frac{1}{2}\cdot\frac{1}{2}} = 1 + 2 + 2 + 4 = 9
\]

### Step 7: Conclusion

The minimum of \( f(x) \) occurs at \( x = \frac{1}{2} \) and the largest \( C \) such that the inequality holds for all \( x, y > 0 \) is

\[
C = 9
\]

Thus, the answer is:

```
The answer is $C=9$
```