## Problem

Let $x, y, z \in [0,1]$. Determine the minimal constant $C$ such that the following inequality holds for all $x, y, z$:
$$
x(x-y)(z-x) \leq C.
$$

## Query

Task description: Please solve the problem with clear, rigorous, and logically sound steps. At the end of your response, state your answer in exactly this format: 'The answer is $C=X$', where X is your calculated numerical bound value. Example: 'The answer is $C=1$'.

Problem: Let $x, y, z \in [0,1]$. Determine the minimal constant $C$ such that the following inequality holds for all $x, y, z$:
$$
x(x-y)(z-x) \leq C.
$$

Solution:

## Response

To determine the minimal constant \( C \) such that the inequality 

\[
x(x-y)(z-x) \leq C
\]

holds for all \( x, y, z \in [0, 1] \), let's go step by step.

### Step 1: Understand the Expression
The expression \( x(x-y)(z-x) \) is a product of three terms:
- \( x \): ranges from \( 0 \) to \( 1 \).
- \( (x-y) \): changes depending on the values of \( x \) and \( y \) (which also range from \( 0 \) to \( 1 \)).
- \( (z-x) \): also depends on \( z \) and ranges between \( 0 \) and \( 1-x \).

### Step 2: Analyze Critical Cases
We will analyze cases where \( x \), \( y \), and \( z \) take on their boundary values (0 or 1), as these often yield extrema. 
1. **Case 1**: \( x = 0 \)
   \[
   0(0 - y)(z - 0) = 0 \leq C
   \]
   Hence, \( C \) can be any positive number.

2. **Case 2**: \( x = 1 \)
   \[
   1(1 - y)(z - 1) = (1 - y)(z - 1)
   \]
   This expression is non-positive since \( z - 1 \leq 0 \) and \( (1 - y) \geq 0 \). Thus, it is also less than or equal to 0.

3. **Case 3**: \( y = 0 \) and \( z = 1 \) when \( x \) varies in \( [0, 1] \):
   \[
   x(x-0)(1-x) = x^2(1-x)
   \]

   To find the maximum of \( x^2(1-x) \), we will calculate its derivative:
   \[
   f(x) = x^2(1 - x)
   \]
   \[
   f'(x) = 2x(1 - x) - x^2 = 2x - 3x^2 = x(2 - 3x)
   \]

   Setting the derivative to zero gives two critical points:
   \[
   x = 0 \quad \text{and} \quad 2 - 3x = 0 \Rightarrow x = \frac{2}{3}
   \]

   Evaluating \( f(x) \):
   - \( f(0) = 0 \)
   - \( f\left(\frac{2}{3}\right) = \left(\frac{2}{3}\right)^2\left(1 - \frac{2}{3}\right) = \frac{4}{9} \cdot \frac{1}{3} = \frac{4}{27} \)
   - \( f(1) = 0 \)

Thus, the maximum value of \( x^2(1-x) \) occurs at \( x = \frac{2}{3} \) and is \( \frac{4}{27} \).

### Step 3: Conclude the Properties of \( C \)
Since the maximum value of \( x(x-y)(z-x) \) is \( \frac{4}{27} \), we conclude that \( C \) must at least be this value:

\[
C \geq \frac{4}{27}
\]

### Final Conclusion
To ensure that the inequality holds for all \( x, y, z \in [0, 1] \), we can conclude that the minimum value of \( C \) is 

\[
C = \frac{4}{27}.
\]

Thus, the final answer is:

```
'The answer is $C=\frac{4}{27}$'
```