## Problem

Let $a, b > 0$ and $a + b \leq \frac{3}{2}$. Find the smallest constant $C$ such that the following inequality holds for all $a, b$ satisfying the given constraint:
$$
\frac{a}{a^2+1} + \frac{4b}{b^2+4} \leq C.
$$

## Query

Task description: Please solve the problem with clear, rigorous, and logically sound steps. At the end of your response, state your answer in exactly this format: 'The answer is $C=X$', where X is your calculated numerical bound value. Example: 'The answer is $C=1$'.

Problem: Let $a, b > 0$ and $a + b \leq \frac{3}{2}$. Find the smallest constant $C$ such that the following inequality holds for all $a, b$ satisfying the given constraint:
$$
\frac{a}{a^2+1} + \frac{4b}{b^2+4} \leq C.
$$

Solution:

## Response

To find the smallest constant \( C \) such that 

\[
\frac{a}{a^2 + 1} + \frac{4b}{b^2 + 4} \leq C
\]

holds for all \( a, b > 0 \) respecting the constraint \( a + b \leq \frac{3}{2} \), let’s analyze each term in the inequality step by step.

### Step 1: Analyze the function \( \frac{a}{a^2 + 1} \)

We start by observing the function:

\[
f(a) = \frac{a}{a^2 + 1}
\]

To find the maximum of this function, we can take its derivative:

\[
f'(a) = \frac{(a^2 + 1)(1) - a(2a)}{(a^2 + 1)^2} = \frac{1 - a^2}{(a^2 + 1)^2}
\]

Setting \( f'(a) = 0 \):

\[
1 - a^2 = 0 \quad \Rightarrow \quad a = 1
\]

Now we need to verify if this is a maximum by evaluating the second derivative or testing the values. Calculate:

- \( f(0) = 0 \)
- \( f(1) = \frac{1}{1^2 + 1} = \frac{1}{2} \)
- \( f(a) \to 0 \) as \( a \to \infty \)

Thus, \( f(a) \) attains its maximum value of \( \frac{1}{2} \) at \( a = 1 \).

### Step 2: Analyze the function \( \frac{4b}{b^2 + 4} \)

Next, we analyze:

\[
g(b) = \frac{4b}{b^2 + 4}
\]

Similarly, we find its maximum by taking the derivative:

\[
g'(b) = \frac{(b^2 + 4)(4) - 4b(2b)}{(b^2 + 4)^2} = \frac{4(b^2 + 4 - 2b^2)}{(b^2 + 4)^2} = \frac{4(4 - b^2)}{(b^2 + 4)^2}
\]

Setting \( g'(b) = 0 \):

\[
4 - b^2 = 0 \quad \Rightarrow \quad b = 2
\]

Verify this is a maximum by checking the values:

- \( g(0) = 0 \)
- \( g(2) = \frac{4 \cdot 2}{2^2 + 4} = \frac{8}{8} = 1 \)
- \( g(b) \to 0 \) as \( b \to \infty \)

Thus, \( g(b) \) attains its maximum value of \( 1 \) at \( b = 2 \).

### Step 3: Find values of \( a \) and \( b \)

Given the constraint \( a + b \leq \frac{3}{2} \), we shouldn’t exceed this sum while maximally utilizing both functions. 

- Consider \( a = 1, b = \frac{1}{2} \):
  - \( 1 + \frac{1}{2} = \frac{3}{2} \)
  
Calculating:

\[
f(1) + g\left(\frac{1}{2}\right) = \frac{1}{2} + \frac{4 \cdot \frac{1}{2}}{(\frac{1}{2})^2 + 4} = \frac{1}{2} + \frac{2}{\frac{1}{4} + 4} = \frac{1}{2} + \frac{2}{\frac{17}{4}} = \frac{1}{2} + \frac{8}{17}
\]

Now, simplifying the expression:

\[
\frac{1}{2} = \frac{17}{34}, \quad \text{so we have } \frac{17}{34} + \frac{8}{17} = \frac{17}{34} + \frac{16}{34} = \frac{33}{34}
\]

### Step 4: Conclusion

The calculations suggest the maximum sum we can reach under the given constraint is \( \frac{33}{34} \). Therefore, we set \( C \) to this maximum value:

\[
C = \frac{33}{34}
\]

Thus, the smallest constant \( C \) satisfying the original inequality is:

\[
\text{The answer is } C = \frac{33}{34}
\] 

Final answer format:

``` 
'The answer is $C=\frac{33}{34}$'
```