## Problem

Let $x, y$ be positive real numbers such that $x + y = 2$. Determine the smallest constant $C$ such that the following inequality holds for all $x, y$:

$$
x^3 y^3 (x^3 + y^3) \leq C.
$$

## Query

Task description: Please solve the problem with clear, rigorous, and logically sound steps. At the end of your response, state your answer in exactly this format: 'The answer is $C=X$', where X is your calculated numerical bound value. Example: 'The answer is $C=1$'.

Problem: Let $x, y$ be positive real numbers such that $x + y = 2$. Determine the smallest constant $C$ such that the following inequality holds for all $x, y$:

$$
x^3 y^3 (x^3 + y^3) \leq C.
$$

Solution:

## Response

To find the smallest constant \( C \) such that the inequality 

\[
x^3 y^3 (x^3 + y^3) \leq C
\]

holds for all positive real numbers \( x \) and \( y \) satisfying \( x + y = 2 \), we follow these steps:

### Step 1: Express \( x \) and \( y \) in terms of a single variable
Let \( x + y = 2 \). We can express \( y \) as \( y = 2 - x \).

### Step 2: Rewrite the inequality
Substituting \( y \) into the inequality gives us:

\[
x^3 (2 - x)^3 (x^3 + (2 - x)^3) \leq C.
\]

### Step 3: Simplify \( (2 - x)^3 \)
Expanding \( (2 - x)^3 \):

\[
(2 - x)^3 = 8 - 12x + 6x^2 - x^3.
\]

### Step 4: Analyze \( x^3 + (2 - x)^3 \)
Now we can write:

\[
x^3 + (2 - x)^3 = x^3 + 8 - 12x + 6x^2 - x^3 = 8 - 12x + 6x^2.
\]

### Step 5: Set up our function to maximize
We want to find a maximum of the function:

\[
f(x) = x^3 (2 - x)^3 (8 - 12x + 6x^2)
\]

for \( x \in (0, 2) \).

### Step 6: Use symmetry
Notice that the function is symmetric around \( x = 1 \). Therefore, we only need to evaluate \( f(1) \):

Calculating \( f(1) \):

- First, \( x^3 = 1^3 = 1 \) and \( (2 - x)^3 = (2-1)^3 = 1\).
- Second, \( 8 - 12 \cdot 1 + 6 \cdot 1^2 = 8 - 12 + 6 = 2 \).

Thus, 

\[
f(1) = 1 \cdot 1 \cdot 2 = 2.
\]

### Step 7: Evaluate the endpoints
We should also verify the values at the endpoints \( x = 0 \) and \( x = 2 \):

- For \( x = 0 \) (then \( y = 2 \)):
    
    \[
    f(0) = 0^3 \cdot 2^3 \cdot (0^3 + 2^3) = 0.
    \]

- For \( x = 2 \) (then \( y = 0 \)):
    
    \[
    f(2) = 2^3 \cdot 0^3 \cdot (2^3 + 0^3) = 0.
    \]

### Step 8: Conclusion
The maximum value of \( f(x) \) occurs at \( x = 1 \), which gives \( f(1) = 2 \). Hence, the smallest constant \( C \) that satisfies the inequality for all positive reals \( x \) and \( y \) such that \( x + y = 2 \) is

\[
C = 2.
\]

### Final Answer
Therefore, 

```
The answer is $C=2$.
```