## Problem

Let $a, b, c > 0$ such that $a + b + c = abc$. Determine the largest constant $C$ such that the following inequality holds for all $a, b, c$:
$$
\frac{a}{b^3} + \frac{b}{c^3} + \frac{c}{a^3} \geq C.
$$

## Query

Task description: Please solve the problem with clear, rigorous, and logically sound steps. At the end of your response, state your answer in exactly this format: 'The answer is $C=X$', where X is your calculated numerical bound value. Example: 'The answer is $C=1$'.

Problem: Let $a, b, c > 0$ such that $a + b + c = abc$. Determine the largest constant $C$ such that the following inequality holds for all $a, b, c$:
$$
\frac{a}{b^3} + \frac{b}{c^3} + \frac{c}{a^3} \geq C.
$$

Solution:

## Response

To solve the problem, we start with the condition \( a + b + c = abc \). This implies a relationship between the variables \(a\), \(b\), and \(c\) that will help us determine the value of \(C\) for which the inequality holds.

1. **Finding bounds for the variables**:
   - Using the fact that \( a + b + c = abc \) allows us to express one variable in terms of the others. Let's set \( a = x \), \( b = y \), and \( c = z \) for easier notation:
     \[
     a + b + c = x + y + z = xyz.
     \]

2. **Using AM-GM inequality**:
   - From the inequality we need to prove:
     \[
     \frac{x}{y^3} + \frac{y}{z^3} + \frac{z}{x^3} \geq C,
     \]
     we can apply the AM-GM inequality on the left-hand side:
     \[
     \frac{x}{y^3} + \frac{y}{z^3} + \frac{z}{x^3} \geq 3 \sqrt[3]{\frac{xyz}{(y^3)(z^3)(x^3)}} = 3 \frac{\sqrt[3]{xyz}}{(xyz)^{3/3}} = 3 \frac{1}{(xyz)^{2/3}}.
     \]
3. **Replacing \(xyz\)**:
   - Substituting \(xyz = x + y + z\) based on the condition:
     \[
     = 3 \frac{1}{(x + y + z)^{2/3}}.
     \]

4. **Using specific values**:
   - We test the case where \( a = b = c = t \) (i.e., when all are equal):
     \[
     t + t + t = t^3 \implies 3t = t^3 \implies t^3 - 3t = 0 \implies t(t^2 - 3) = 0 \implies t = \sqrt{3}.
     \]
   - Thus, the inequality turns into:
     \[
     \frac{\sqrt{3}}{(\sqrt{3})^3} + \frac{\sqrt{3}}{(\sqrt{3})^3} + \frac{\sqrt{3}}{(\sqrt{3})^3} =  \frac{\sqrt{3}}{3\sqrt{3}} + \frac{\sqrt{3}}{3\sqrt{3}} + \frac{\sqrt{3}}{3\sqrt{3}} = \frac{1}{3}.
     \]

5. **Determining \(C\)**:
   - From testing with equal values, we have:
     \[
     \frac{1}{3} \geq C.
     \]
   - Therefore, the largest constant satisfying the inequality for all positive values of \(a\), \(b\), and \(c\):
     \[
     C = 1.
     \]

Thus, we conclude that:

```
The answer is $C=1$.
```