## Problem

Given $k > 1$ and $a, b, c > 0$ with $abc = k^3$, find the largest constant $C$ such that the following inequality holds for all $a, b, c$:

$$
\sum_{\text{cyc}}\left(\frac{1}{1+a}+\frac{1}{1+bc}\right) \geq C\left(\frac{1}{1+k}+\frac{1}{1+k^2}\right).
$$

## Query

Task description: Please solve the problem with clear, rigorous, and logically sound steps. At the end of your response, state your answer in exactly this format: 'The answer is $C=X$', where X is your calculated numerical bound value. Example: 'The answer is $C=1$'.

Problem: Given $k > 1$ and $a, b, c > 0$ with $abc = k^3$, find the largest constant $C$ such that the following inequality holds for all $a, b, c$:

$$
\sum_{\text{cyc}}\left(\frac{1}{1+a}+\frac{1}{1+bc}\right) \geq C\left(\frac{1}{1+k}+\frac{1}{1+k^2}\right).
$$

Solution:

## Response

To find the largest constant \( C \) for the given inequality:

\[
\sum_{\text{cyc}}\left(\frac{1}{1+a}+\frac{1}{1+bc}\right) \geq C\left(\frac{1}{1+k}+\frac{1}{1+k^2}\right)
\]

where \( k > 1 \) and \( abc = k^3 \) with \( a, b, c > 0 \), we can follow these steps:

### Step 1: Analyze the left-hand side

We start with the left-hand side of the inequality:

\[
L = \sum_{\text{cyc}} \left(\frac{1}{1+a} + \frac{1}{1+bc}\right),
\]

which expands to:

\[
L = \frac{1}{1+a} + \frac{1}{1+b} + \frac{1}{1+c} + \frac{1}{1+bc} + \frac{1}{1+ca} + \frac{1}{1+ab}.
\]

### Step 2: Simplify the right-hand side

Next, we rewrite the right-hand side:

\[
R = C\left(\frac{1}{1+k} + \frac{1}{1+k^2}\right).
\]

### Step 3: Use substitutions \( a = kx, b = ky, c = kz \)

Since \( abc = k^3 \), we let:

\[
a = kx, \quad b = ky, \quad c = kz
\]

where \( xyz = 1 \) (i.e., \( x, y, z > 0 \)). Thus:

\[
k^3xyz = k^3 \implies xyz = 1.
\]

Now substituting these back into \( L \):

\[
L = \frac{1}{1+kx} + \frac{1}{1+ky} + \frac{1}{1+kz} + \frac{1}{1+k^2 yz} + \frac{1}{1+k^2 xz} + \frac{1}{1+k^2 xy}.
\]

### Step 4: Examine limits as \( k \to 1 \)

When \( k = 1 \) (as a special case), the expression can simplify:

\[
L = 3 \cdot \frac{1}{1+1} + 3 \cdot \frac{1}{1+1} = 3 \cdot \frac{1}{2} + 3 \cdot \frac{1}{2} = 3.
\]

And:

\[
R = C\left(\frac{1}{2} + \frac{1}{2}\right) = C.
\]

Thus, we find \( C \leq 3 \).

### Step 5: General case analysis

As \( k \) increases, consider symmetry in variable definitions:

Testing \( a = b = c = k \), we find that:

\[
L = 2 + 3 \cdot \frac{1}{1+k^2}.
\]

Setting \( L \geq 3R \):

\[
2 + 3 \cdot \frac{1}{1+k^2} \geq C \cdot 2 \implies 1 + \frac{3}{2(1+k^2)} \geq C.
\]

### Step 6: Finding maximum \( C \)

For \( k \to \infty \):

\[
L \to 3, \quad R \to C \cdot 1 = C.
\]

### Conclusion

Thus, the maximum value that satisfies all scenarios whilst maintaining the inequality is:

\[
C = 1.
\]

Hence, the final answer is:

```
The answer is $C=1$.
```