## Problem

Let $a, b, c \geq 0$ be non-negative real numbers such that $a + b + c = 1$. Consider the following inequality:
$$
7(ab + bc + ca) \quad () \quad 3 + 9abc.
$$

Determine the correct inequality relation to fill in the blank.

Options:

(A) $\leq$ 

(B) $\geq$

(C) $=$ 

(D) $<$

(E) $>$

(F) None of the above

## Query

Task description: Please solve the problem with clear, rigorous, and logically sound steps. At the end of your response, state your answer in exactly this format: 'The answer is (Letter) Symbol', where Letter is one of the given options. Example: 'The answer is (A) $\leq$'.

Problem: Let $a, b, c \geq 0$ be non-negative real numbers such that $a + b + c = 1$. Consider the following inequality:
$$
7(ab + bc + ca) \quad () \quad 3 + 9abc.
$$

Determine the correct inequality relation to fill in the blank.

Options:

(A) $\leq$ 

(B) $\geq$

(C) $=$ 

(D) $<$

(E) $>$

(F) None of the above

Solution:

## Response

To solve the inequality \( 7(ab + bc + ca) \) and determine its relationship with \( 3 + 9abc \) under the constraint \( a + b + c = 1 \) (where \( a, b, c \geq 0 \)), we will follow these steps:

### Step 1: Analyze the expressions

1. Since \( a, b, c \geq 0 \) and \( a + b + c = 1 \):
   - \( ab + bc + ca \) can be maximized and minimized under these constraints.
   - \( abc \) will also vary accordingly.

### Step 2: Apply known inequalities

2. We can use the identity:
   \[
   (a + b + c)^2 = a^2 + b^2 + c^2 + 2(ab + ac + bc)
   \]
   Hence,
   \[
   1 = a^2 + b^2 + c^2 + 2(ab + ac + bc)
   \]
   Rearranging gives:
   \[
   ab + ac + bc = \frac{1 - (a^2 + b^2 + c^2)}{2}
   \]

### Step 3: Estimate maximum values

3. To explore the maximum of \( ab + ac + bc \):
   - By the Cauchy-Schwarz inequality:
   \[
   (a + b + c)^2 \geq 3(ab + ac + bc)
   \]
   thus:
   \[
   1 \geq 3(ab + ac + bc) \Rightarrow ab + ac + bc \leq \frac{1}{3}
   \]

4. Therefore:
   \[
   7(ab + ac + bc) \leq 7 \cdot \frac{1}{3} = \frac{7}{3}
   \]

### Step 4: Analyze the term \( 3 + 9abc \)

5. For \( abc \):
   - Let \( a = x, b = y, c = 1 - x - y \):
   \[
   abc = xy(1 - x - y)
   \]
   - The maximum value of \( abc \) will occur at specific values of \( a, b, c \).
   - Using symmetry, for maximum \( abc \), we can assume \( a = b = c \), i.e., \( a = b = c = \frac{1}{3} \):
   \[
   abc = \left(\frac{1}{3}\right)^3 = \frac{1}{27}
   \]
   It gives:
   \[
   3 + 9abc = 3 + 9 \cdot \frac{1}{27} = 3 + \frac{1}{3} = \frac{10}{3}
   \]

### Step 5: Comparing the two sides

6. We now have:
   \[
   7(ab + ac + bc) \leq \frac{7}{3} \quad \text{and} \quad 3 + 9abc = \frac{10}{3}
   \]
   Thus, we observe:
   \[
   \frac{7}{3} < \frac{10}{3}
   \]

### Conclusion

Therefore, the correct relation to fill in the blank is:

\[
7(ab + ac + bc) < 3 + 9abc
\]

Thus:

```
'The answer is (D) <'
```