## Problem

Let $a, b, c \in (0,1)$. Consider the following inequality:
$$
\sqrt{a b c} + \sqrt{(1-a)(1-b)(1-c)} \quad () \quad 1.
$$

Determine the correct inequality relation to fill in the blank.

Options:

(A) $\leq$ 

(B) $\geq$

(C) $=$ 

(D) $<$

(E) $>$

(F) None of the above

## Query

Task description: Please solve the problem with clear, rigorous, and logically sound steps. At the end of your response, state your answer in exactly this format: 'The answer is (Letter) Symbol', where Letter is one of the given options. Example: 'The answer is (A) $\leq$'.

Problem: Let $a, b, c \in (0,1)$. Consider the following inequality:
$$
\sqrt{a b c} + \sqrt{(1-a)(1-b)(1-c)} \quad () \quad 1.
$$

Determine the correct inequality relation to fill in the blank.

Options:

(A) $\leq$ 

(B) $\geq$

(C) $=$ 

(D) $<$

(E) $>$

(F) None of the above

Solution:

## Response

To solve the inequality 

\[
\sqrt{abc} + \sqrt{(1-a)(1-b)(1-c)} \quad () \quad 1,
\]

where \(a, b, c \in (0,1)\), we analyze both terms in the expression.

### Step 1: Bound each term

1. **Bounding \(\sqrt{abc}\)**:
   - Since \(a, b, c \in (0, 1)\), it follows that \(abc < 1\). Therefore, \(\sqrt{abc} < 1\).

2. **Bounding \(\sqrt{(1-a)(1-b)(1-c)}\)**:
   - Similarly, since \(1-a, 1-b, 1-c \in (0, 1)\), we have \((1-a)(1-b)(1-c) < 1\), hence \(\sqrt{(1-a)(1-b)(1-c)} < 1\).

### Step 2: Total maximum value

The sum of the maximum values of \(\sqrt{abc}\) and \(\sqrt{(1-a)(1-b)(1-c)}\) is:

\[
\sqrt{abc} + \sqrt{(1-a)(1-b)(1-c)} < 1 + 1 = 2.
\]

However, since both components are strictly less than 1, we can more carefully analyze their potential sums.

### Step 3: Analyze for extreme cases

**Case 1: When \(a = b = c = \frac{1}{2}\)**
- We calculate:
    \[
    \sqrt{abc} = \sqrt{\left(\frac{1}{2}\right)^3} = \sqrt{\frac{1}{8}} = \frac{1}{2\sqrt{2}} \approx 0.354.
    \]
  
    \[
    \sqrt{(1-a)(1-b)(1-c)} = \sqrt{\left(\frac{1}{2}\right)^3} = \frac{1}{2\sqrt{2}} \approx 0.354.
    \]

Thus,

\[
\sqrt{abc} + \sqrt{(1-a)(1-b)(1-c)} = 0.354 + 0.354 \approx 0.707 < 1.
\]

**Case 2: When \(a = 1\), \(b = 1\), and \(c = 1\)**
- In this case, both terms become \(0\), leading to:
\[
\sqrt{1} + \sqrt{0} = 1 + 0 = 1.
\]

---

### Conclusion

Through these bounds and evaluations, we find:

- The sum of \(\sqrt{abc}\) and \(\sqrt{(1-a)(1-b)(1-c)}\) can reach, but never exceed \(1\), in the open interval \( (0,1) \).
- Thus, the inequality relation to fill in is:

\[
\sqrt{abc} + \sqrt{(1-a)(1-b)(1-c)} \leq 1.
\]

So, the answer is:

```plaintext
'The answer is (A) $\leq$'
```