## Problem

Let $a, b, c > 0$ be positive real numbers such that $a b c = 1$. Consider the following inequality:
$$
\frac{a b}{a^2+b^2+\sqrt{c}}+\frac{b c}{b^2+c^2+\sqrt{a}}+\frac{c a}{c^2+a^2+\sqrt{b}} \quad () \quad \frac{3}{2}.
$$

Determine the correct inequality relation to fill in the blank.

Options:

(A) $\leq$ 

(B) $\geq$

(C) $=$ 

(D) $<$

(E) $>$

(F) None of the above

## Query

Task description: Please solve the problem with clear, rigorous, and logically sound steps. At the end of your response, state your answer in exactly this format: 'The answer is (Letter) Symbol', where Letter is one of the given options. Example: 'The answer is (A) $\leq$'.

Problem: Let $a, b, c > 0$ be positive real numbers such that $a b c = 1$. Consider the following inequality:
$$
\frac{a b}{a^2+b^2+\sqrt{c}}+\frac{b c}{b^2+c^2+\sqrt{a}}+\frac{c a}{c^2+a^2+\sqrt{b}} \quad () \quad \frac{3}{2}.
$$

Determine the correct inequality relation to fill in the blank.

Options:

(A) $\leq$ 

(B) $\geq$

(C) $=$ 

(D) $<$

(E) $>$

(F) None of the above

Solution:

## Response

To solve the problem, we will analyze the given inequality step by step using known mathematical tools.

### Given:
Let \( a, b, c > 0 \) such that \( abc = 1 \). We need to consider the inequality:

\[
\frac{ab}{a^2 + b^2 + \sqrt{c}} + \frac{bc}{b^2 + c^2 + \sqrt{a}} + \frac{ca}{c^2 + a^2 + \sqrt{b}} \quad ? \quad \frac{3}{2}
\]

### Step 1: Analyze Each Term

Letâ€™s denote each term in the sum as \( x_1, x_2, x_3 \):

\[
x_1 = \frac{ab}{a^2 + b^2 + \sqrt{c}}, \quad x_2 = \frac{bc}{b^2 + c^2 + \sqrt{a}}, \quad x_3 = \frac{ca}{c^2 + a^2 + \sqrt{b}}
\]

### Step 2: Use the AM-GM Inequality

We apply the Arithmetic Mean-Geometric Mean inequality (AM-GM):

\[
a^2 + b^2 + \sqrt{c} \geq 3 \sqrt[3]{a^2b^2\sqrt{c}} = 3 \sqrt[3]{(abc)^{\frac{2}{3}}} = 3 \sqrt[3]{1^{\frac{2}{3}}} = 3
\]

Thus,

\[
x_1 = \frac{ab}{a^2 + b^2 + \sqrt{c}} \leq \frac{ab}{3}
\]

By similar reasoning for \( x_2 \) and \( x_3 \):

\[
x_2 \leq \frac{bc}{3}, \quad x_3 \leq \frac{ca}{3}
\]

### Step 3: Combining the Terms

Combining these inequalities:

\[
x_1 + x_2 + x_3 \leq \frac{ab}{3} + \frac{bc}{3} + \frac{ca}{3} = \frac{1}{3}(ab + bc + ca)
\]

### Step 4: Applying the AM-GM Inequality on \( ab + bc + ca \)

Using AM-GM again:

\[
ab + bc + ca \geq 3 \sqrt[3]{(abc)^2} = 3 \sqrt[3]{1} = 3
\]

### Step 5: Conclusion

Thus,

\[
x_1 + x_2 + x_3 \leq \frac{1}{3} \cdot 3 = 1
\]

Since \( 1 < \frac{3}{2} \), we conclude:

\[
\frac{ab}{a^2 + b^2 + \sqrt{c}} + \frac{bc}{b^2 + c^2 + \sqrt{a}} + \frac{ca}{c^2 + a^2 + \sqrt{b}} < \frac{3}{2}
\]

This implies that the correct choice for the inequality relation is:

**(D) \( < \)**

### Final Answer

```plaintext
'The answer is (D) <'
```