## Problem

Let $a, b, c > 0$ be positive real numbers such that $ab + bc + ca = 1$. Consider the following inequality:
$$
a b c\left(a+\sqrt{a^2+1}\right)\left(b+\sqrt{b^2+1}\right)\left(c+\sqrt{c^2+1}\right) \quad () \quad 2.
$$

Determine the correct inequality relation to fill in the blank.

Options:

(A) $\leq$ 

(B) $\geq$

(C) $=$ 

(D) $<$

(E) $>$

(F) None of the above

## Query

Task description: Please solve the problem with clear, rigorous, and logically sound steps. At the end of your response, state your answer in exactly this format: 'The answer is (Letter) Symbol', where Letter is one of the given options. Example: 'The answer is (A) $\leq$'.

Problem: Let $a, b, c > 0$ be positive real numbers such that $ab + bc + ca = 1$. Consider the following inequality:
$$
a b c\left(a+\sqrt{a^2+1}\right)\left(b+\sqrt{b^2+1}\right)\left(c+\sqrt{c^2+1}\right) \quad () \quad 2.
$$

Determine the correct inequality relation to fill in the blank.

Options:

(A) $\leq$ 

(B) $\geq$

(C) $=$ 

(D) $<$

(E) $>$

(F) None of the above

Solution:

## Response

To solve the given inequality problem, we start by analyzing the expression

\[
abc\left(a+\sqrt{a^2+1}\right)\left(b+\sqrt{b^2+1}\right)\left(c+\sqrt{c^2+1}\right).
\]

### Step 1: Understand components of the product

We recognize that \( a + \sqrt{a^2 + 1} \) can be rewritten to facilitate comparison:

\[
a + \sqrt{a^2 + 1} = \sqrt{(a + \sqrt{a^2 + 1})^2} = \sqrt{a^2 + 2a + (a^2 + 1)} = \sqrt{2a^2 + 2a + 1}.
\]

However, we can keep \( a + \sqrt{a^2 + 1} \) as is for now.

### Step 2: Rewrite the product and bound it

Let's denote:

\[
X = abc\left(a+\sqrt{a^2+1}\right)\left(b+\sqrt{b^2+1}\right)\left(c+\sqrt{c^2+1}\right).
\]

We know by AM-GM inequality that for any positive \( x \),

\[
x + \sqrt{x^2 + 1} \geq 2 \sqrt{xy} \Rightarrow \left(a + \sqrt{a^2+1}\right) \geq \sqrt{2}a.
\]

Thus we can bound each term:

\[
\left(a+\sqrt{a^2+1}\right) \geq \sqrt{2} a,
\]
\[
\left(b+\sqrt{b^2+1}\right) \geq \sqrt{2} b,
\]
\[
\left(c+\sqrt{c^2+1}\right) \geq \sqrt{2} c.
\]

### Step 3: Substitute and compare

Substituting these back in:

\[
X \geq abc \cdot \sqrt{2}a \cdot \sqrt{2}b \cdot \sqrt{2}c = 2\sqrt{2}a^2b^2c^2.
\]

### Step 4: Analyze the constraint

Given the condition:

\[
ab + bc + ca = 1,
\]

using the AM-GM inequality, we find:

\[
ab + bc + ca \geq 3\sqrt[3]{(abc)^2} \Rightarrow \frac{1}{3} \geq 3\sqrt[3]{(abc)^2} \Rightarrow abc \leq \frac{1}{3\sqrt{3}}.
\]

### Step 5: Combine results and evaluate

Now, consider the right-hand side:

\[
X \geq 2\sqrt{2}a^2b^2c^2.
\]

To find a numeric relation, substitute \( a = b = c = \frac{1}{3\sqrt{3}} \):

Calculating each:

1. \( abc = \left(\frac{1}{3\sqrt{3}}\right)^3 = \frac{1}{27\sqrt{27}} \).
2. From the substitution above, calculate \( 2\sqrt{2} \left(\frac{1}{3\sqrt{3}}\right)^2 \).

Comparing the left-hand and right-hand sides shows it leads to:

\[
X \leq \frac{1}{3} \cdot 1 = \frac{1}{3}.
\]

### Conclusion

As the right-hand side does not exceed \( \frac{1}{3} \) when substituting back and analyzing the constraints, it follows that the original inequality holds:

\[
abc\left(a+\sqrt{a^2+1}\right)\left(b+\sqrt{b^2+1}\right)\left(c+\sqrt{c^2+1}\right) \leq 2.
\]

Thus, the completed inequality is:

\[
\boxed{A}.
\]

The answer is '"'"'The answer is (A) $\leq$'"'"'.