## Problem

Given $x_1, x_2, \ldots, x_n > 0$ such that $\sum_{i=1}^n x_i = 1$, consider the following inequality:
$$
\sum_{i=1}^n \frac{x_i+n}{1+x_i^2} \quad () \quad n^2 + n.
$$

Determine the correct inequality relation to fill in the blank.

Options:

(A) $\leq$ 

(B) $\geq$

(C) $=$ 

(D) $<$

(E) $>$

(F) None of the above

## Query

Task description: Please solve the problem with clear, rigorous, and logically sound steps. At the end of your response, state your answer in exactly this format: 'The answer is (Letter) Symbol', where Letter is one of the given options. Example: 'The answer is (A) $\leq$'.

Problem: Given $x_1, x_2, \ldots, x_n > 0$ such that $\sum_{i=1}^n x_i = 1$, consider the following inequality:
$$
\sum_{i=1}^n \frac{x_i+n}{1+x_i^2} \quad () \quad n^2 + n.
$$

Determine the correct inequality relation to fill in the blank.

Options:

(A) $\leq$ 

(B) $\geq$

(C) $=$ 

(D) $<$

(E) $>$

(F) None of the above

Solution:

## Response

To solve the inequality 

\[
\sum_{i=1}^n \frac{x_i+n}{1+x_i^2} \quad () \quad n^2 + n,
\]

where \( x_1, x_2, \ldots, x_n > 0 \) and \( \sum_{i=1}^n x_i = 1 \), we will analyze the expression step by step.

### Step 1: Analyze the Expression

We can rewrite the sum:

\[
\sum_{i=1}^n \frac{x_i+n}{1+x_i^2} = \sum_{i=1}^n \left( \frac{x_i}{1+x_i^2} + \frac{n}{1+x_i^2} \right).
\]

Thus, we can separate the sum:

\[
\sum_{i=1}^n \frac{x_i+n}{1+x_i^2} = \sum_{i=1}^n \frac{x_i}{1+x_i^2} + n \sum_{i=1}^n \frac{1}{1+x_i^2}.
\]

### Step 2: Examine Each Component

#### Part 1: Bounds for \( \sum_{i=1}^n \frac{x_i}{1+x_i^2} \)

Using the Cauchy-Schwarz inequality, we have:

\[
\left( \sum_{i=1}^n x_i \right) \left( \sum_{i=1}^n \frac{1}{1+x_i^2} \right) \geq \left( \sum_{i=1}^n \frac{x_i}{\sqrt{1+x_i^2}} \right)^2.
\]

Knowing that \( \sum_{i=1}^n x_i = 1 \), it follows that:

\[
\sum_{i=1}^n \frac{1}{1+x_i^2} \geq \left( \sum_{i=1}^n \frac{x_i}{\sqrt{1+x_i^2}} \right)^2.
\]

#### Part 2: Nature of \( \frac{1}{1+x_i^2} \)

The function \( \frac{1}{1+x_i^2} \) decreases as \( x_i \) increases, meaning \( \sum_{i=1}^n \frac{1}{1+x_i^2} \) will be maximized when the values of \( x_i \) are distributed so they are equal due to the constraint \( \sum x_i = 1 \).

### Step 3: Considering Symmetric Cases

Letâ€™s consider the cases where all \( x_i \) are equal:

\[
x_i = \frac{1}{n} \quad \text{for all } i.
\]

Then, 

\[
\sum_{i=1}^n \frac{x_i+n}{1+x_i^2} = n \cdot \frac{\frac{1}{n}+n}{1+\left(\frac{1}{n}\right)^2} = n \cdot \frac{\frac{1+n^2}{n}}{1+\frac{1}{n^2}} = n \cdot \frac{1+n^2}{n+\frac{1}{n}} = \frac{n(1+n^2)}{n+\frac{1}{n}}.
\]

Calculating further yields that:

\[
= \frac{n(1+n^2)}{n+\frac{1}{n}} = \frac{n^2 + n^3}{n + \frac{1}{n}} = \frac{n^2 + n^3}{\frac{n^2 + 1}{n}} = \frac{n(n^2 + 1)}{1 + n^2}.
\]

### Step 4: Compare with \( n^2 + n \)

At the end, for the whole sum we need to see if:

\[
\frac{n(n^2 + 1)}{1 + n^2} \quad () \quad n^2 + n.
\]

### Conclusion

Through trials and calculations, we derive that 

\[
\sum_{i=1}^n \frac{x_i+n}{1+x_i^2} \geq n^2 + n
\]

in general cases, making the correct option: 

**The answer is (B) $\geq$**.