## Problem

Let $x, y, z \in \mathbb{R}$ such that $x^2 + 2y^2 + z^2 = \frac{2}{5} a^2$, where $a > 0$. Consider the following expression:
$$
|x - y + z| \quad () \quad a.
$$

Determine the correct inequality relation to fill in the blank.

Options:

(A) $\leq$ 

(B) $\geq$

(C) $=$ 

(D) $<$

(E) $>$

(F) None of the above

## Query

Task description: Please solve the problem with clear, rigorous, and logically sound steps. At the end of your response, state your answer in exactly this format: 'The answer is (Letter) Symbol', where Letter is one of the given options. Example: 'The answer is (A) $\leq$'.

Problem: Let $x, y, z \in \mathbb{R}$ such that $x^2 + 2y^2 + z^2 = \frac{2}{5} a^2$, where $a > 0$. Consider the following expression:
$$
|x - y + z| \quad () \quad a.
$$

Determine the correct inequality relation to fill in the blank.

Options:

(A) $\leq$ 

(B) $\geq$

(C) $=$ 

(D) $<$

(E) $>$

(F) None of the above

Solution:

## Response

To solve the problem, we start with the equation given:

\[
x^2 + 2y^2 + z^2 = \frac{2}{5} a^2,
\]

where \( a > 0 \). We need to analyze the expression:

\[
|x - y + z|.
\]

### Step 1: Using the Cauchy-Schwarz Inequality

We can employ the Cauchy-Schwarz inequality in the following context:

Given two sequences \( (1, 1, 1) \) and \( (x, -y, z) \):

\[
|x - y + z|^2 \leq (1^2 + 1^2 + 1^2)(x^2 + y^2 + z^2).
\]

This gives:

\[
|x - y + z|^2 \leq 3(x^2 + 2y^2 + z^2).
\]

### Step 2: Substituting the Given Condition

Substituting \( x^2 + 2y^2 + z^2 \) from the original equation:

\[
|x - y + z|^2 \leq 3\left(\frac{2}{5} a^2\right) = \frac{6}{5} a^2.
\]

Taking the square root on both sides, we find:

\[
|x - y + z| \leq \sqrt{\frac{6}{5}} a.
\]

### Step 3: Evaluating the Comparison

We need to compare \( |x - y + z| \) with \( a \):

\[
|x - y + z| \leq \sqrt{\frac{6}{5}} a.
\]

Now, note that:

\[
\sqrt{\frac{6}{5}} \approx 1.095.
\]

Thus, we have:

\[
|x - y + z| \leq \sqrt{\frac{6}{5}} a > a.
\]

### Step 4: Conclusion 

Therefore, we have confirmed that:

\[
|x - y + z| < a,
\]

since \( \sqrt{\frac{6}{5}} a > a \). 

This leads us to the conclusion, as we found that \( |x - y + z| \) is less than \( a \).

### Final Statement

Thus, the correct inequality to fill in the blank is:

'"'"'The answer is (D) $<$'"'"'.