## Problem

Let $a, b, c$ be positive real numbers such that $abc = 1$. Consider the following inequality:
$$
\sum \frac{1}{b(a+b)} \quad () \quad \frac{5}{3}.
$$

Determine the correct inequality relation to fill in the blank.

Options:

(A) $\leq$ 

(B) $\geq$

(C) $=$ 

(D) $<$

(E) $>$

(F) None of the above

## Query

Task description: Please solve the problem with clear, rigorous, and logically sound steps. At the end of your response, state your answer in exactly this format: 'The answer is (Letter) Symbol', where Letter is one of the given options. Example: 'The answer is (A) $\leq$'.

Problem: Let $a, b, c$ be positive real numbers such that $abc = 1$. Consider the following inequality:
$$
\sum \frac{1}{b(a+b)} \quad () \quad \frac{5}{3}.
$$

Determine the correct inequality relation to fill in the blank.

Options:

(A) $\leq$ 

(B) $\geq$

(C) $=$ 

(D) $<$

(E) $>$

(F) None of the above

Solution:

## Response

To solve the inequality 

\[
\sum \frac{1}{b(a+b)} \quad () \quad \frac{5}{3}
\]

given the condition \( abc = 1 \), we will proceed with the following steps:

### Step 1: Symmetry and Homogeneity
Since \( a, b, c \) are positive real numbers such that \( abc = 1 \), we can apply the method of substitution. Letâ€™s denote \( a = \frac{x}{y}, b = \frac{y}{z}, c = \frac{z}{x} \), which maintains the condition \( abc = 1 \).

### Step 2: Rewrite the Expression
The expression to evaluate becomes:
\[
\frac{1}{b(a+b)} = \frac{1}{\frac{y}{z}\left(\frac{x}{y} + \frac{y}{z}\right)} = \frac{z}{y\left(x + \frac{y^2}{z}\right)} = \frac{z}{xy + y^2}
\]
Now rewriting the symmetric sum:
\[
\sum \frac{1}{b(a+b)} = \sum \frac{z}{xy + y^2}
\]

### Step 3: Apply Cauchy-Schwarz Inequality
Using Cauchy-Schwarz inequality on \(\sum \frac{1}{b(a+b)}\), we have:

\[
\left( \sum \frac{1}{b(a+b)} \right) \left( \sum b(a+b) \right) \geq (1+1+1)^2 = 9
\]

### Step 4: Calculate the Denominator
Calculating the sums,
\[
\sum b(a+b) = \sum b(a) + \sum b(b) = \sum ab + \sum b^2
\]
By AM-GM, \( \sum ab \geq 3\sqrt[3]{(abc)^2} = 3 \), and 
\( a + b + c \geq 3\sqrt[3]{abc} = 3 \). 

Thus, we arrive at:
\[
\sum b(a+b) \geq 2(ab + ac + bc) \geq 3
\]

### Step 5: Final Calculation
From Cauchy-Schwarz, we have:
\[
\sum \frac{1}{b(a+b)} \geq \frac{9}{\sum b(a+b)} \geq \frac{9}{3} = 3
\]

### Step 6: Verifying Against \( \frac{5}{3} \)
Since \( 3 > \frac{5}{3} \), we consider:

\[
\sum \frac{1}{b(a+b)} > \frac{5}{3}
\]

### Conclusion
So we conclude that:

\[
\sum \frac{1}{b(a+b)} > \frac{5}{3}
\]

Thus, the correct option to fill in the blank is:

```
The answer is (E) $>$.
```