## Problem

Let $a, b, c$ be positive numbers. Consider the following inequality:
$$
\frac{a^2}{b} + \frac{b^2}{c} + \frac{4c^2}{a} \quad () \quad -3a + b + 7c.
$$

Determine the correct inequality relation to fill in the blank.

Options:

(A) $\leq$ 

(B) $\geq$

(C) $=$ 

(D) $<$

(E) $>$

(F) None of the above

## Query

Task description: Please solve the problem with clear, rigorous, and logically sound steps. At the end of your response, state your answer in exactly this format: 'The answer is (Letter) Symbol', where Letter is one of the given options. Example: 'The answer is (A) $\leq$'.

Problem: Let $a, b, c$ be positive numbers. Consider the following inequality:
$$
\frac{a^2}{b} + \frac{b^2}{c} + \frac{4c^2}{a} \quad () \quad -3a + b + 7c.
$$

Determine the correct inequality relation to fill in the blank.

Options:

(A) $\leq$ 

(B) $\geq$

(C) $=$ 

(D) $<$

(E) $>$

(F) None of the above

Solution:

## Response

To solve the problem, we need to analyze the given inequality:

\[
\frac{a^2}{b} + \frac{b^2}{c} + \frac{4c^2}{a} \quad () \quad -3a + b + 7c
\]

We will explore the left-hand side and the right-hand side separately and ascertain how they compare to each other.

### Step 1: Analyze the Left-Hand Side

The left-hand side is:

\[
LHS = \frac{a^2}{b} + \frac{b^2}{c} + \frac{4c^2}{a}
\]

Using the **AM-GM Inequality**:

\[
\frac{a^2}{b} + \frac{b^2}{c} + \frac{4c^2}{a} \geq 3\sqrt[3]{\frac{a^2}{b} \cdot \frac{b^2}{c} \cdot \frac{4c^2}{a}}
\]

Calculating the product gives:

\[
\frac{a^2}{b} \cdot \frac{b^2}{c} \cdot \frac{4c^2}{a} = \frac{4a^2b^2c^2}{abc} = 4abc
\]

Thus,

\[
LHS \geq 3\sqrt[3]{4abc}
\]

### Step 2: Analyze the Right-Hand Side

The right-hand side is:

\[
RHS = -3a + b + 7c
\]

### Step 3: Ultimately Compare LHS and RHS

Now, we need to find the relationship between \( LHS \) and \( RHS \). It is easier to experiment with various values for \( a, b, c \):

1. **Let \( a = 1, b = 1, c = 1 \):**
   \[
   LHS = \frac{1^2}{1} + \frac{1^2}{1} + \frac{4 \cdot 1^2}{1} = 1 + 1 + 4 = 6
   \]
   \[
   RHS = -3 \cdot 1 + 1 + 7 = 5
   \]
   So, \( LHS = 6 \) and \( RHS = 5 \). This suggests \( 6 \geq 5 \).

2. **Let \( a = 1, b = 2, c = 2 \):**
   \[
   LHS = \frac{1^2}{2} + \frac{2^2}{2} + \frac{4 \cdot 2^2}{1} = \frac{1}{2} + 2 + 16 = 18.5
   \]
   \[
   RHS = -3 \cdot 1 + 2 + 7 = 6
   \]
   So, \( LHS = 18.5 \) and \( RHS = 6 \). This suggests \( 18.5 \geq 6 \).

3. **Let \( a = 1, b = 3, c = 1 \):**
   \[
   LHS = \frac{1^2}{3} + \frac{3^2}{1} + \frac{4 \cdot 1^2}{1} = \frac{1}{3} + 9 + 4 = \frac{1}{3} + 13 = \frac{40}{3} \approx 13.33
   \]
   \[
   RHS = -3 \cdot 1 + 3 + 7 = 7
   \]
   So, \( LHS \approx 13.33 \) and \( RHS = 7 \). This supports \( LHS \geq RHS \).

### Conclusion

From the tests above and the established inequality from the AM-GM approach, the general relation we see consistently is:

\[
\frac{a^2}{b} + \frac{b^2}{c} + \frac{4c^2}{a} \geq -3a + b + 7c
\]

Thus, the correct choice to fill in the inequality is:

**Answer:**

'''"The answer is (B) $\geq$"'''