## Problem

Let $a, b, c$ be positive real numbers. Consider the following inequality:
$$
\sum_{cyc} \frac{b+c}{\sqrt{(a+b)(a+c)}} \quad () \quad 2 \sum_{cyc} \frac{2a}{2b+c}.
$$

Determine the correct inequality relation to fill in the blank.

Options:

(A) $\leq$ 

(B) $\geq$

(C) $=$ 

(D) $<$

(E) $>$

(F) None of the above

## Query

Task description: Please solve the problem with clear, rigorous, and logically sound steps. At the end of your response, state your answer in exactly this format: 'The answer is (Letter) Symbol', where Letter is one of the given options. Example: 'The answer is (A) $\leq$'.

Problem: Let $a, b, c$ be positive real numbers. Consider the following inequality:
$$
\sum_{cyc} \frac{b+c}{\sqrt{(a+b)(a+c)}} \quad () \quad 2 \sum_{cyc} \frac{2a}{2b+c}.
$$

Determine the correct inequality relation to fill in the blank.

Options:

(A) $\leq$ 

(B) $\geq$

(C) $=$ 

(D) $<$

(E) $>$

(F) None of the above

Solution:

## Response

To solve the inequality involving positive real numbers \(a\), \(b\), and \(c\):

### Given Inequality

We need to analyze and compare the following expressions:
\[
S_1 = \sum_{cyc} \frac{b+c}{\sqrt{(a+b)(a+c)}}
\]
and 
\[
S_2 = 2 \sum_{cyc} \frac{2a}{2b+c}.
\]

### Step 1: Analyzing \(S_1\)

First, let's rewrite \(S_1\) based on the cyclic nature of the sum:
\[
S_1 = \frac{b+c}{\sqrt{(a+b)(a+c)}} + \frac{c+a}{\sqrt{(b+c)(b+a)}} + \frac{a+b}{\sqrt{(c+a)(c+b)}}.
\]

We'll use the Cauchy-Schwarz inequality to estimate \(S_1\):
\[
\left(\sum_{cyc} \frac{b+c}{\sqrt{(a+b)(a+c)}}\right)^2 \leq \left(\sum_{cyc} (b+c)\right) \left(\sum_{cyc} \frac{1}{(a+b)(a+c)}\right).
\]

### Step 2: Estimating \(S_2\)

Now, letâ€™s analyze \(S_2\):
\[
S_2 = 2\left(\frac{2a}{2b+c} + \frac{2b}{2c+a} + \frac{2c}{2a+b}\right).
\]

By applying the Cauchy-Schwarz inequality again:
\[
S_2 = 2 \cdot \sum_{cyc} \frac{2a}{2b+c} \geq 2 \cdot \frac{(2a + 2b + 2c)^2}{\sum_{cyc} (2b+c)}.
\]

### Step 3: Comparing \(S_1\) and \(S_2\)

Now we need to compare these two expressions. Through testing cases where \(a = b = c\) leads to straightforward numerical evaluations. 

Let \( a = b = c = 1 \):
1. **Calculate \(S_1\)**:
   \[
   S_1 = 3 \cdot \frac{2}{\sqrt{4}} = 3 \cdot 1 = 3.
   \]
2. **Calculate \(S_2\)**:
   \[
   S_2 = 2 \cdot 3 \cdot \frac{2}{2} = 2 \cdot 3 = 6.
   \]

From this calculation, \(S_1 = 3\) and \(S_2 = 6\).

### Conclusion

Since \(S_1 < S_2\) in this case, we can conjecture that generally:
\[
S_1 < S_2.
\]
Therefore, we conclude that the inequality to fill the blank is:
\[
\sum_{cyc} \frac{b+c}{\sqrt{(a+b)(a+c)}} < 2 \sum_{cyc} \frac{2a}{2b+c}.
\]

Thus, the answer is:
'''The answer is (D) $<$'''