## Problem

Let $a, b, c, d$ be non-negative numbers. Consider the following inequality:
$$
a^4 +2 b^4 + 3c^4 + d^4 + 3abcd \quad () \quad \frac{1}{2} \sum_{cyc} a^3(b+c+d).
$$

Determine the correct inequality relation to fill in the blank.

Options:

(A) $\leq$ 

(B) $\geq$

(C) $=$ 

(D) $<$

(E) $>$

(F) None of the above

## Query

Task description: Please solve the problem with clear, rigorous, and logically sound steps. At the end of your response, state your answer in exactly this format: 'The answer is (Letter) Symbol', where Letter is one of the given options. Example: 'The answer is (A) $\leq$'.

Problem: Let $a, b, c, d$ be non-negative numbers. Consider the following inequality:
$$
a^4 +2 b^4 + 3c^4 + d^4 + 3abcd \quad () \quad \frac{1}{2} \sum_{cyc} a^3(b+c+d).
$$

Determine the correct inequality relation to fill in the blank.

Options:

(A) $\leq$ 

(B) $\geq$

(C) $=$ 

(D) $<$

(E) $>$

(F) None of the above

Solution:

## Response

To solve the inequality 

\[
a^4 + 2b^4 + 3c^4 + d^4 + 3abcd \quad () \quad \frac{1}{2} \sum_{cyc} a^3(b+c+d),
\]

we will analyze both sides step-by-step and determine the relation that is true for all non-negative \(a\), \(b\), \(c\), and \(d\).

### Analyzing the Left Side

The left side is \(L = a^4 + 2b^4 + 3c^4 + d^4 + 3abcd\).

### Analyzing the Right Side

The right side can be expanded as follows:

\[
R = \frac{1}{2} \left( a^3(b+c+d) + b^3(c+d+a) + c^3(d+a+b) + d^3(a+b+c) \right).
\]

### Comparing Terms

To analyze the inequality, we should test specific values for \(a\), \(b\), \(c\), and \(d\). 

1. **Test Case 1**: Let \(a = 1\), \(b = 1\), \(c = 1\), \(d = 1\):

   \[
   L = 1^4 + 2 \cdot 1^4 + 3 \cdot 1^4 + 1^4 + 3 \cdot 1 \cdot 1 \cdot 1 \cdot 1 = 1 + 2 + 3 + 1 + 3 = 10.
   \]
   \[
   R = \frac{1}{2} \left( 1^3(1+1+1) + 1^3(1+1+1) + 1^3(1+1+1) + 1^3(1+1+1) \right) = \frac{1}{2} (3 + 3 + 3 + 3) = \frac{12}{2} = 6.
   \]

   Here, \(L = 10\) and \(R = 6\) gives \(10 \geq 6\). 

2. **Test Case 2**: Let \(a = 0\), \(b = 1\), \(c = 1\), \(d = 1\):

   \[
   L = 0 + 2 \cdot 1^4 + 3 \cdot 1^4 + 1^4 + 0 = 2 + 3 + 1 = 6,
   \]
   \[
   R = \frac{1}{2}(0 + 1^3(1+1+1) + 1^3(1+1+0) + 1^3(0+1+1)) = \frac{1}{2}(0 + 3 + 2 + 2) = \frac{7}{2} = 3.5.
   \]

   Here, \(L = 6\) and \(R = 3.5\) gives \(6 \geq 3.5\).

3. **Test Case 3**: Let \(a = 0\), \(b = 0\), \(c = 0\), \(d = 1\):

   \[
   L = 0 + 0 + 0 + 1^4 + 0 = 1,
   \]
   \[
   R = \frac{1}{2}(0 + 0 + 0 + 1^3(0 + 0 + 0)) = 0.
   \]

   Here, \(1 \geq 0\).

### Conclusion

From these test cases, it appears that 

\[
a^4 + 2b^4 + 3c^4 + d^4 + 3abcd \geq \frac{1}{2} \sum_{cyc} a^3(b+c+d)
\]

holds true for non-negative \(a\), \(b\), \(c\), and \(d\).

Therefore, we conclude that the correct inequality relation is:

'"'"'The answer is (B) $\geq$'"'"'