## Problem

Let $a, b, c > 0$ such that $a+b+c=2$ and $a^2+b^2+c^2=2$. Determine the minimal constant $C$ such that the following inequality holds for all $a, b, c$ satisfying the given constraints:
$$
a b c \leq C.
$$

## Query

Task description: Please solve the problem with clear, rigorous, and logically sound steps. At the end of your response, state your answer in exactly this format: 'The answer is $C=X$', where X is your calculated numerical bound value. Example: 'The answer is $C=1$'.

Problem: Let $a, b, c > 0$ such that $a+b+c=2$ and $a^2+b^2+c^2=2$. Determine the minimal constant $C$ such that the following inequality holds for all $a, b, c$ satisfying the given constraints:
$$
a b c \leq C.
$$

Solution:

## Response

To solve the problem, we start with the constraints:

1. \( a + b + c = 2 \)
2. \( a^2 + b^2 + c^2 = 2 \)

We aim to find a minimal constant \( C \) such that:

\[
abc \leq C
\]

### Step 1: Derive Additional Relationships

Using the identity:

\[
(a + b + c)^2 = a^2 + b^2 + c^2 + 2(ab + ac + bc)
\]

we substitute in our constraints:

\[
2^2 = 2 + 2(ab + ac + bc) \implies 4 = 2 + 2(ab + ac + bc) \implies ab + ac + bc = 1
\]

### Step 2: Use Symmetric Functions

Let \( a, b, c \) be the roots of the polynomial \( x^3 - px^2 + qx - r = 0 \). From our previous results, we have:

- \( p = a + b + c = 2 \)
- \( q = ab + ac + bc = 1 \)
- \( r = abc \)

### Step 3: Apply AM-GM Inequality

To apply the AM-GM inequality on \( a, b, c \):

\[
\frac{a + b + c}{3} \geq \sqrt[3]{abc}
\]

Substituting \( a + b + c = 2 \):

\[
\frac{2}{3} \geq \sqrt[3]{abc} \implies abc \leq \left(\frac{2}{3}\right)^3 = \frac{8}{27}
\]

### Step 4: Check Feasibility

Now, we must check if \( abc = \frac{8}{27} \) can be achieved within the constraints \( a + b + c = 2 \) and \( a^2 + b^2 + c^2 = 2 \).

Assuming \( a = b \) and \( c = 2 - 2a \):

1. Substitute into the second equation:
   \[
   2a^2 + (2 - 2a)^2 = 2
   \]
   \[
   2a^2 + (4 - 8a + 4a^2) = 2
   \]
   \[
   6a^2 - 8a + 2 = 0
   \]

2. Solve this quadratic using the quadratic formula:
   \[
   a = \frac{-(-8) \pm \sqrt{(-8)^2 - 4 \cdot 6 \cdot 2}}{2 \cdot 6} = \frac{8 \pm \sqrt{64 - 48}}{12}
   \]
   \[
   = \frac{8 \pm \sqrt{16}}{12} = \frac{8 \pm 4}{12}
   \]

This gives us two potential values for \( a \):

- \( a = 1 \) (thus \( b = 1 \) and \( c = 0 \))
- \( a = \frac{2}{3} \) (thus \( b = \frac{2}{3} \) and \( c = \frac{2}{3} \))

### Step 5: Calculate \( abc \)

For \( a = b = \frac{2}{3} \) and \( c = \frac{2 - 2(2/3)}{1} = \frac{2}{3} \):

\[
abc = \left(\frac{2}{3}\right)^3 = \frac{8}{27}
\]

Thus, the maximum value of \( abc \) that satisfies both conditions is indeed \( \frac{8}{27} \).

### Conclusion

Therefore, the minimal constant \( C \) such that \( abc \leq C \) for all valid \( a, b, c \) is:

\[
\boxed{\frac{8}{27}}
\]

Final answer in the specified format:

```
The answer is $C=\frac{8}{27}$
```