## Problem

Let $a, b, c \geq 0$ be real numbers such that $a^2 + b^2 + c^2 = 3$. Consider the following inequality:
$$
\sum_{cyc} \frac{a}{a+2} \quad () \quad 1.
$$

Determine the correct inequality relation to fill in the blank.

Options:

(A) $\leq$ 

(B) $\geq$

(C) $=$ 

(D) $<$

(E) $>$

(F) None of the above

## Query

Task description: Please solve the problem with clear, rigorous, and logically sound steps. At the end of your response, state your answer in exactly this format: 'The answer is (Letter) Symbol', where Letter is one of the given options. Example: 'The answer is (A) $\leq$'.

Problem: Let $a, b, c \geq 0$ be real numbers such that $a^2 + b^2 + c^2 = 3$. Consider the following inequality:
$$
\sum_{cyc} \frac{a}{a+2} \quad () \quad 1.
$$

Determine the correct inequality relation to fill in the blank.

Options:

(A) $\leq$ 

(B) $\geq$

(C) $=$ 

(D) $<$

(E) $>$

(F) None of the above

Solution:

## Response

To solve the problem, we want to analyze the inequality 

\[
\sum_{cyc} \frac{a}{a+2} \quad () \quad 1
\]

Given the condition \( a^2 + b^2 + c^2 = 3 \) for non-negative real numbers \( a, b, c \geq 0 \).

### Step-by-step Solution:

1. **Understanding the Cyclic Sum**:
   \( \sum_{cyc} \frac{a}{a+2} \) means we are summing cyclically over \( a, b, c \):
   \[
   \frac{a}{a+2} + \frac{b}{b+2} + \frac{c}{c+2}
   \]

2. **Analyzing Each Term**:
   For each \( x \geq 0 \):
   \[
   \frac{x}{x+2} = 1 - \frac{2}{x+2}
   \]
   We can rewrite the cyclic sum as:
   \[
   \sum_{cyc} \left( 1 - \frac{2}{x+2} \right) = 3 - 2 \sum_{cyc} \frac{1}{x+2}
   \]

3. **Finding the Lower Bound for Each Fraction**:
   Since \( a, b, c \) satisfy \( a^2 + b^2 + c^2 = 3 \), by the Cauchy-Schwarz inequality:
   \[
   (1^2 + 1^2 + 1^2)(\frac{1}{a+2} + \frac{1}{b+2} + \frac{1}{c+2}) \geq \left( \frac{1}{\sqrt{a+2} + \sqrt{b+2} + \sqrt{c+2}} \right)^2
   \]
   However, for simplicity, we note that \( \frac{1}{x+2} \) is decreasing.

4. **Simple Cases**:
   Let's evaluate a few simple cases to gather insights.
   - When \( a = b = c = 1 \):
     \[
     \sum_{cyc} \frac{1}{1+2} = \sum_{cyc} \frac{1}{3} = 1
     \]

   - When \( a = 0 \), \( b = 0 \), and \( c = \sqrt{3} \):
     \[
     \frac{0}{0+2} + \frac{0}{0+2} + \frac{\sqrt{3}}{\sqrt{3}+2} < 1
     \]
     Since \( \frac{\sqrt{3}}{2+\sqrt{3}} < 1 \).

5. **Conclusion from Cases**:
   It's reasonable to assert that as one variable (let's say \( c \)) approaches the whole of \( 3 \) (with others being \( 0 \)):
   \[
   \sum_{cyc} \frac{a}{a+2} \to \text{some value} < 1
   \]

From evaluating \( a=1, b=1, c=1 \) and extremes of the cyclic sum, it appears evident that:

\[
\sum_{cyc} \frac{a}{a+2} < 1
\]

### Final Determination of the Inequality
Putting this all together, the correct relation to fill in the blank is:

\[
\sum_{cyc} \frac{a}{a+2} < 1
\]

Thus, the conclusion is:

```
'The answer is (D) <'
```