## Problem

Let $a, b, c$ be positive real numbers such that $a + b + c = 1$. Consider the following inequality:
$$
a \sqrt[3]{1+b-c} + b \sqrt[3]{1+c-a} + c \sqrt[3]{1+a-b} \quad () \quad 1.
$$

Determine the correct inequality relation to fill in the blank.

Options:

(A) $\leq$ 

(B) $\geq$

(C) $=$ 

(D) $<$

(E) $>$

(F) None of the above

## Query

Task description: Please solve the problem with clear, rigorous, and logically sound steps. At the end of your response, state your answer in exactly this format: 'The answer is (Letter) Symbol', where Letter is one of the given options. Example: 'The answer is (A) $\leq$'.

Problem: Let $a, b, c$ be positive real numbers such that $a + b + c = 1$. Consider the following inequality:
$$
a \sqrt[3]{1+b-c} + b \sqrt[3]{1+c-a} + c \sqrt[3]{1+a-b} \quad () \quad 1.
$$

Determine the correct inequality relation to fill in the blank.

Options:

(A) $\leq$ 

(B) $\geq$

(C) $=$ 

(D) $<$

(E) $>$

(F) None of the above

Solution:

## Response

To analyze the inequality

\[
a \sqrt[3]{1+b-c} + b \sqrt[3]{1+c-a} + c \sqrt[3]{1+a-b} \quad \_ \quad 1
\]

given that \(a + b + c = 1\), let's define \(x = b + c\), \(y = c + a\), and \(z = a + b\). Then we rewrite the expressions inside the cube roots:

- \(1 + b - c = 1 + (b + c - c) = 1 + x - 2c\)
- \(1 + c - a = 1 + (c + a - a) = 1 + y - 2a\)
- \(1 + a - b = 1 + (a + b - b) = 1 + z - 2b\)

We analyze the behavior of each term. Since \(1 + b - c = 1 + x - 2c\), \(1 + c - a\), and \(1 + a - b\) can be expressed in terms of sums of \(a, b, c\).

### Step 1: Useful Inequality

Utilizing Jensen's Inequality is suitable here since the function \(f(t) = \sqrt[3]{t}\) is concave for \(t > 0\). Therefore, if we apply Jensen's Inequality:

\[
a \sqrt[3]{1+b-c} + b \sqrt[3]{1+c-a} + c \sqrt[3]{1+a-b} \leq \sqrt[3]{a(1+b-c) + b(1+c-a) + c(1+a-b)}
\]

### Step 2: Evaluating Right Hand Side

Now evaluating the right hand side more carefully:

\[
RHS = a(1 + b - c) + b(1 + c - a) + c(1 + a - b) = a + b + c + ab - ac + bc - ba + ca - cb = 1 + (ab + bc + ca) - (ac + ba + cb)
\]

Given \(a + b + c = 1\), we simplify and deduce properties about the left-hand side compared to the right-hand side. 

### Step 3: Restricting the Problem to a Suitable Case

We could also test simple cases: letâ€™s take special cases like \(a = b = c = \frac{1}{3}\):

\[
\frac{1}{3} \sqrt[3]{1 + \frac{1}{3} - \frac{1}{3}} + \frac{1}{3} \sqrt[3]{1 + \frac{1}{3} - \frac{1}{3}} + \frac{1}{3} \sqrt[3]{1 + \frac{1}{3} - \frac{1}{3}} = \sqrt[3]{1} = 1
\]

All these imply:

### Final Analysis

Thus through Jensen's inequality and the symmetry of the cubes, it appears that:

\[
a \sqrt[3]{1+b-c} + b \sqrt[3]{1+c-a} + c \sqrt[3]{1+a-b} \leq 1
\]

This leads us to our answer:

'"'"'The answer is (A) $\leq$'"'"'