## Problem

Let $a, b, c \in \mathbb{R}^{+}$ be positive real numbers. Consider the following inequality:
$$
\frac{a}{\sqrt{a^2+b^2}} + \frac{b}{\sqrt{2b^2+c^2}} + \frac{c}{\sqrt{3c^2+a^2}} \quad () \quad \frac{3 \sqrt{2}}{2}.
$$

Determine the correct inequality relation to fill in the blank.

Options:

(A) $\leq$ 

(B) $\geq$

(C) $=$ 

(D) $<$

(E) $>$

(F) None of the above

## Query

Task description: Please solve the problem with clear, rigorous, and logically sound steps. At the end of your response, state your answer in exactly this format: 'The answer is (Letter) Symbol', where Letter is one of the given options. Example: 'The answer is (A) $\leq$'.

Problem: Let $a, b, c \in \mathbb{R}^{+}$ be positive real numbers. Consider the following inequality:
$$
\frac{a}{\sqrt{a^2+b^2}} + \frac{b}{\sqrt{2b^2+c^2}} + \frac{c}{\sqrt{3c^2+a^2}} \quad () \quad \frac{3 \sqrt{2}}{2}.
$$

Determine the correct inequality relation to fill in the blank.

Options:

(A) $\leq$ 

(B) $\geq$

(C) $=$ 

(D) $<$

(E) $>$

(F) None of the above

Solution:

## Response

To solve the inequality 

\[
\frac{a}{\sqrt{a^2+b^2}} + \frac{b}{\sqrt{2b^2+c^2}} + \frac{c}{\sqrt{3c^2+a^2}} \quad () \quad \frac{3\sqrt{2}}{2},
\]

we can analyze each term individually. Let's denote the three fractions as follows:

- \( x_1 = \frac{a}{\sqrt{a^2 + b^2}}, \)
- \( x_2 = \frac{b}{\sqrt{2b^2 + c^2}}, \)
- \( x_3 = \frac{c}{\sqrt{3c^2 + a^2}}. \)

### Step 1: Evaluate individual terms

Using the Cauchy-Schwarz inequality for each term, we get:

1. For \( x_1 \):
   \[
   x_1 = \frac{a}{\sqrt{a^2 + b^2}} \leq \frac{a}{\sqrt{2ab}} = \frac{1}{\sqrt{2}} \sqrt{\frac{a^2}{b}}.
   \]

2. For \( x_2 \):
   \[
   x_2 = \frac{b}{\sqrt{2b^2 + c^2}} \leq \frac{b}{\sqrt{3bc}}.
   \]

3. For \( x_3 \):
   \[
   x_3 = \frac{c}{\sqrt{3c^2 + a^2}} \leq \frac{c}{\sqrt{4ac}} = \frac{1}{2} \sqrt{\frac{c^2}{a}}.
   \]

### Step 2: Sum the terms
To find a bound for the sum \( x_1 + x_2 + x_3 \), we can see that each fraction is upper-bounded by terms involving constants and squares of the respective values of \( a, b, \) and \( c \).

Adding these inequalities gives us:
\[
x_1 + x_2 + x_3 \leq \frac{1}{\sqrt{2}} + \frac{b}{\sqrt{3c}} + \frac{1}{2} \sqrt{\frac{c^2}{a}}.
\]

### Step 3: Consider equal shares
Assume all \( a, b, c \) are equal or set in a geometric proportion, then normally, through symmetry and equality conditions, we may evaluate:

Substituting \( a = b = c \) into the mixed terms and simplifying:
\[
x_1 + x_2 + x_3 = 3 \left( \frac{a}{\sqrt{a^2 + a^2}} \right) = 3 \cdot \frac{1}{\sqrt{2}} = \frac{3\sqrt{2}}{2}.
\]

### Step 4: Validating inequality 
Now we have:

\[
\frac{3 \sqrt{2}}{2} \leq \frac{3 \sqrt{2}}{2},
\]
indicating that the original inequality is indeed true since it can equal.

### Conclusion
Thus, filling in the blank, we find:

The correct relation is:

'"'"'The answer is (C) $='$"'"'.