## Problem

Let $x, y, z \in \mathbb{R}$. Consider the following expression:
$$
\frac{x^2-y^2}{2x^2+1} + \frac{y^2-z^2}{2y^2+1} + \frac{z^2-x^2}{2z^2+1} \quad () \quad 0.
$$

Determine the correct inequality relation to fill in the blank.

Options:

(A) $\leq$ 

(B) $\geq$

(C) $=$ 

(D) $<$

(E) $>$

(F) None of the above

## Query

Task description: Please solve the problem with clear, rigorous, and logically sound steps. At the end of your response, state your answer in exactly this format: 'The answer is (Letter) Symbol', where Letter is one of the given options. Example: 'The answer is (A) $\leq$'.

Problem: Let $x, y, z \in \mathbb{R}$. Consider the following expression:
$$
\frac{x^2-y^2}{2x^2+1} + \frac{y^2-z^2}{2y^2+1} + \frac{z^2-x^2}{2z^2+1} \quad () \quad 0.
$$

Determine the correct inequality relation to fill in the blank.

Options:

(A) $\leq$ 

(B) $\geq$

(C) $=$ 

(D) $<$

(E) $>$

(F) None of the above

Solution:

## Response

To solve the problem, we need to analyze the expression given:

\[
\frac{x^2 - y^2}{2x^2 + 1} + \frac{y^2 - z^2}{2y^2 + 1} + \frac{z^2 - x^2}{2z^2 + 1}
\]

We rewrite this expression term by term.

### Step 1: Breakdown the expression

1. **First term**: \( \frac{x^2 - y^2}{2x^2 + 1} \)

   Here, we note:
   \[
   x^2 - y^2 = (x+y)(x-y)
   \]
   Hence, it becomes:
   \[
   \frac{(x+y)(x-y)}{2x^2 + 1}
   \]

2. **Second term**: \( \frac{y^2 - z^2}{2y^2 + 1} \)

   Similarly:
   \[
   y^2 - z^2 = (y+z)(y-z)
   \]
   Becomes:
   \[
   \frac{(y+z)(y-z)}{2y^2 + 1}
   \]

3. **Third term**: \( \frac{z^2 - x^2}{2z^2 + 1} \)

   And:
   \[
   z^2 - x^2 = (z+x)(z-x)
   \]
   Becomes:
   \[
   \frac{(z+x)(z-x)}{2z^2 + 1}
   \]

### Step 2: Consider the overall sum

Combining these, we can rewrite it as:
\[
S = \frac{(x+y)(x-y)}{2x^2 + 1} + \frac{(y+z)(y-z)}{2y^2 + 1} + \frac{(z+x)(z-x)}{2z^2 + 1}
\]

### Step 3: Analyze behavior of each term

Notice that the denominator \(2x^2 + 1\) is always positive. Therefore, the sign of each term depends solely on the numerator.

### Step 4: Set \(x = y = z\)

Letâ€™s first test when \(x = y = z = k\). Then:
\[
S = \frac{k^2 - k^2}{2k^2 + 1} + \frac{k^2 - k^2}{2k^2 + 1} + \frac{k^2 - k^2}{2k^2 + 1} = 0
\]

This suggests \(S = 0\) when \(x = y = z\).

### Step 5: Examining extreme cases

1. **Case when \(x \to \infty\), \(y = 0\), \(z = 0\)**:
   \[
   S = \frac{x^2 - 0^2}{2x^2 + 1} + \frac{0^2 - 0^2}{2\cdot0 + 1} + \frac{0^2 - x^2}{2\cdot0 + 1}
   \]
   Simplifying:
   \[
   S \to 1 + 0 - x^2
   \]
   which tends to \(-\infty\).

2. **Case when \(x = 0\), \(y = z = k\)** yields:
   \[
   S = 0 + \frac{k^2 - k^2}{2k^2 + 1} + 0 = 0.
   \]

### Conclusion

Both examples \(x = y = z\) lead to \(S = 0\) and extreme variations drive \(S\) potentially downwards. The argument also hinges on each pair \(x, y\) and symmetrically checking against their differences.

Thus, we find that the sum:
\[
S \leq 0
\]

Based on this analysis, we fill the blank with:

'"'"'The answer is (A) $\leq$'"'"'