## Problem

Let $a, b, c > 0$ be positive real numbers such that $a + b + c = 3$. Consider the following inequality:
$$
a^2 + 4b^2 + 4b + 8c \quad () \quad 7 + 2\sqrt{2(b^2 + c^2)} + 4\sqrt{bc}.
$$

Determine the correct inequality relation to fill in the blank.

Options:

(A) $\leq$ 

(B) $\geq$

(C) $=$ 

(D) $<$

(E) $>$

(F) None of the above

## Query

Task description: Please solve the problem with clear, rigorous, and logically sound steps. At the end of your response, state your answer in exactly this format: 'The answer is (Letter) Symbol', where Letter is one of the given options. Example: 'The answer is (A) $\leq$'.

Problem: Let $a, b, c > 0$ be positive real numbers such that $a + b + c = 3$. Consider the following inequality:
$$
a^2 + 4b^2 + 4b + 8c \quad () \quad 7 + 2\sqrt{2(b^2 + c^2)} + 4\sqrt{bc}.
$$

Determine the correct inequality relation to fill in the blank.

Options:

(A) $\leq$ 

(B) $\geq$

(C) $=$ 

(D) $<$

(E) $>$

(F) None of the above

Solution:

## Response

To solve the inequality involving the positive real numbers \( a, b, c \) such that \( a + b + c = 3 \), we need to analyze the expression:

\[
a^2 + 4b^2 + 4b + 8c \quad () \quad 7 + 2\sqrt{2(b^2 + c^2)} + 4\sqrt{bc}.
\]

### Step 1: Substitute \( c \)

Since \( a + b + c = 3 \), we can express \( c \) as:

\[
c = 3 - a - b.
\]

### Step 2: Substitute \( c \) into the inequality

Substituting for \( c \):

\[
a^2 + 4b^2 + 4b + 8(3 - a - b) = a^2 + 4b^2 + 4b + 24 - 8a - 8b.
\]

Thus, the left-hand side simplifies to:

\[
a^2 + 4b^2 - 8a - 4b + 24.
\]

### Step 3: Analyze the right-hand side

The right side, \( 7 + 2\sqrt{2(b^2 + c^2)} + 4\sqrt{bc} \), requires handling \( c \) as:

\[
c^2 = (3 - a - b)^2.
\]

We can expand and rearrange as needed, but first, it might be easier to analyze the terms individually.

### Step 4: Examine a specific case

Let \( a = b = c = 1 \):

\[
LHS = 1^2 + 4(1^2) + 4(1) + 8(1) = 1 + 4 + 4 + 8 = 17.
\]

Now compute the right-hand side:

\[
RHS = 7 + 2\sqrt{2(1^2 + 1^2)} + 4\sqrt{1 \cdot 1} = 7 + 2\sqrt{4} + 4 = 7 + 4 + 4 = 15.
\]

Notice that:

\[
LHS = 17 > RHS = 15.
\]

### Step 5: Test boundary values

Assuming \( a = 3 \) (and \( b = c = 0 \)) yields:

\[
LHS = 3^2 + 0 + 0 + 0 = 9,
\]
\[
RHS = 7 + 0 + 0 = 7,
\]
\[
9 > 7.
\]

Now testing \( a = 0, b = 3, c = 0 \):

\[
LHS = 0 + 4(3^2) + 4(3) + 0 = 36 + 12 = 48,
\]
\[
RHS = 7 + 0 + 0 = 7,
\]
\[
48 > 7.
\]

### Conclusion on inequality

The inequality appears to be a strict one, indicating a general trend where:

\[
LHS > RHS
\]
for various cases tested. Therefore no \( a, b, c > 0 \) leads to the left side being less or equal to the right side under constraints.

Thus, we conclude our investigation with the chosen option being:

```plaintext
'The answer is (E) >'
```