## Problem

Let $a, b, c \neq 0$ be non-zero real numbers such that $a^2 + b^2 + c^2 = 2(ab + bc + ca)$. Consider the following expression:
$$
(a+b+c)\left(\frac{1}{2a}+\frac{1}{3b}+\frac{1}{c}\right) \quad () \quad 14.
$$

Determine the correct inequality relation to fill in the blank.

Options:

(A) $\leq$ 

(B) $\geq$

(C) $=$ 

(D) $<$

(E) $>$

(F) None of the above

## Query

Task description: Please solve the problem with clear, rigorous, and logically sound steps. At the end of your response, state your answer in exactly this format: 'The answer is (Letter) Symbol', where Letter is one of the given options. Example: 'The answer is (A) $\leq$'.

Problem: Let $a, b, c \neq 0$ be non-zero real numbers such that $a^2 + b^2 + c^2 = 2(ab + bc + ca)$. Consider the following expression:
$$
(a+b+c)\left(\frac{1}{2a}+\frac{1}{3b}+\frac{1}{c}\right) \quad () \quad 14.
$$

Determine the correct inequality relation to fill in the blank.

Options:

(A) $\leq$ 

(B) $\geq$

(C) $=$ 

(D) $<$

(E) $>$

(F) None of the above

Solution:

## Response

To solve the given problem, we start with the equation provided:

\[
a^2 + b^2 + c^2 = 2(ab + bc + ca).
\]

### Step 1: Rearrange the equation

Rearranging gives:

\[
a^2 + b^2 + c^2 - 2(ab + bc + ca) = 0.
\]

This can be factored as:

\[
\frac{1}{2}(a-b)^2 + \frac{1}{2}(b-c)^2 + \frac{1}{2}(c-a)^2 = 0.
\]

For this sum to equal zero, each squared term must be zero:

\[
a = b = c.
\]

### Step 2: Assume \( a = b = c \)

Let \( a = b = c = k \) (for some \( k \neq 0 \)). Then, substituting into the expression we need to analyze, we have:

1. \( a + b + c = 3k \).
2. \( \frac{1}{2a} + \frac{1}{3b} + \frac{1}{c} = \frac{1}{2k} + \frac{1}{3k} + \frac{1}{k} \).

### Step 3: Simplify the expression

Now, focusing on \( \frac{1}{2k} + \frac{1}{3k} + \frac{1}{k} \):

\[
\frac{1}{2k} + \frac{1}{3k} + \frac{1}{k} = \frac{1}{k} \left( \frac{1}{2} + \frac{1}{3} + 1 \right).
\]

Calculating \( \frac{1}{2} + \frac{1}{3} + 1 \):

\[
\frac{1}{2} + \frac{1}{3} + 1 = \frac{3}{6} + \frac{2}{6} + \frac{6}{6} = \frac{11}{6}.
\]

So, we have:

\[
\frac{1}{2a} + \frac{1}{3b} + \frac{1}{c} = \frac{11}{6k}.
\]

### Step 4: Calculate the whole expression

Now we substitute back into the expression:

\[
(3k) \left( \frac{11}{6k} \right) = \frac{33k}{6k} = \frac{33}{6} = 5.5.
\]

### Step 5: Compare with 14

We need to determine the relation between \( 5.5 \) and \( 14 \):

\[
5.5 < 14.
\]

### Conclusion

Thus, the correct inequality is:

```
'The answer is (D) <'
```