## Problem

Let $a, b > 0$ be positive real numbers such that $a + b \leq \frac{3}{2}$. Consider the following inequality:
$$
\frac{a}{2a^2+1} + \frac{4b}{3b^2+4} \quad () \quad \frac{7}{5}.
$$

Determine the correct inequality relation to fill in the blank.

Options:

(A) $\leq$ 

(B) $\geq$

(C) $=$ 

(D) $<$

(E) $>$

(F) None of the above

## Query

Task description: Please solve the problem with clear, rigorous, and logically sound steps. At the end of your response, state your answer in exactly this format: 'The answer is (Letter) Symbol', where Letter is one of the given options. Example: 'The answer is (A) $\leq$'.

Problem: Let $a, b > 0$ be positive real numbers such that $a + b \leq \frac{3}{2}$. Consider the following inequality:
$$
\frac{a}{2a^2+1} + \frac{4b}{3b^2+4} \quad () \quad \frac{7}{5}.
$$

Determine the correct inequality relation to fill in the blank.

Options:

(A) $\leq$ 

(B) $\geq$

(C) $=$ 

(D) $<$

(E) $>$

(F) None of the above

Solution:

## Response

To solve the problem, we need to analyze the inequality 

\[
\frac{a}{2a^2+1} + \frac{4b}{3b^2+4} \quad () \quad \frac{7}{5}
\]

given the constraints \( a, b > 0 \) and \( a + b \leq \frac{3}{2} \).

### Step 1: Analyze each term

1. **For the first term** \(\frac{a}{2a^2 + 1}\):
   - To find the maximum value of this expression with respect to \(a\), we can take its derivative. 
   - Let \(f(a) = \frac{a}{2a^2 + 1}\).
   - To find critical points, we calculate:

   \[
   f'(a) = \frac{(2a^2 + 1)(1) - a(4a)}{(2a^2 + 1)^2} = \frac{2a^2 + 1 - 4a^2}{(2a^2 + 1)^2} = \frac{1 - 2a^2}{(2a^2 + 1)^2}
   \]

   Setting \(f'(a) = 0\):

   \[
   1 - 2a^2 = 0 \quad \Rightarrow \quad a^2 = \frac{1}{2} \quad \Rightarrow \quad a = \frac{1}{\sqrt{2}} \approx 0.707
   \]

   Evaluating \(f(a)\) at \(a = \frac{1}{\sqrt{2}}\):

   \[
   f\left(\frac{1}{\sqrt{2}}\right) = \frac{\frac{1}{\sqrt{2}}}{2 \cdot \left(\frac{1}{2}\right) + 1} = \frac{\frac{1}{\sqrt{2}}}{2} = \frac{1}{2\sqrt{2}} \approx 0.3536
   \]

2. **For the second term** \(\frac{4b}{3b^2 + 4}\):

   Similarly, let \(g(b) = \frac{4b}{3b^2 + 4}\).
   - Taking the derivative:

   \[
   g'(b) = \frac{(3b^2 + 4)(4) - 4b(6b)}{(3b^2 + 4)^2} = \frac{12b^2 + 16 - 24b^2}{(3b^2 + 4)^2} = \frac{16 - 12b^2}{(3b^2 + 4)^2}
   \]

   Setting \(g'(b) = 0\):

   \[
   16 - 12b^2 = 0 \quad \Rightarrow \quad b^2 = \frac{4}{3} \quad \Rightarrow \quad b = \frac{2}{\sqrt{3}} \approx 1.1547
   \]

   Evaluating \(g(b)\) at \(b = \frac{2}{\sqrt{3}}\):

   \[
   g\left(\frac{2}{\sqrt{3}}\right) = \frac{4 \cdot \frac{2}{\sqrt{3}}}{3 \cdot \frac{4}{3} + 4} = \frac{\frac{8}{\sqrt{3}}}{8} = \frac{1}{\sqrt{3}} \approx 0.5774
   \]

### Step 2: Combine the Maximized Values

Under the conditions \(a + b \leq \frac{3}{2}\):

Letâ€™s denote the maximum sum of values:

\[
\frac{a}{2a^2 + 1} + \frac{4b}{3b^2 + 4} \approx 0.3536 + 0.5774 \approx 0.931
\]

Now we can compare this sum to \(\frac{7}{5} = 1.4\).

### Step 3: Compare to \(\frac{7}{5}\)

Since \(0.931 < 1.4\):

We conclude:

\[
\frac{a}{2a^2 + 1} + \frac{4b}{3b^2 + 4} < \frac{7}{5}
\]

### Conclusion

The correct inequality to fill in the blank is 

\[
\frac{a}{2a^2 + 1} + \frac{4b}{3b^2 + 4} \quad < \quad \frac{7}{5}.
\]

Thus, the answer is:

``'The answer is (D) $<$'``