## Problem

Let $a, b > 0$ be positive real numbers such that $a^2 + b^2 + 3 = 4ab$. Consider the following inequality:
$$
2\sqrt{2ab} - \frac{1}{2}a - b \quad () \quad \frac{1}{2}.
$$

Determine the correct inequality relation to fill in the blank.

Options:

(A) $\leq$ 

(B) $\geq$

(C) $=$ 

(D) $<$

(E) $>$

(F) None of the above

## Query

Task description: Please solve the problem with clear, rigorous, and logically sound steps. At the end of your response, state your answer in exactly this format: 'The answer is (Letter) Symbol', where Letter is one of the given options. Example: 'The answer is (A) $\leq$'.

Problem: Let $a, b > 0$ be positive real numbers such that $a^2 + b^2 + 3 = 4ab$. Consider the following inequality:
$$
2\sqrt{2ab} - \frac{1}{2}a - b \quad () \quad \frac{1}{2}.
$$

Determine the correct inequality relation to fill in the blank.

Options:

(A) $\leq$ 

(B) $\geq$

(C) $=$ 

(D) $<$

(E) $>$

(F) None of the above

Solution:

## Response

To tackle the problem, we start with the given equation:

\[
a^2 + b^2 + 3 = 4ab
\]

Rearranging this, we can express it as:

\[
a^2 + b^2 - 4ab + 3 = 0
\]

This is a quadratic in terms of \(a\):

\[
a^2 - 4ab + b^2 + 3 = 0
\]

Now, let's calculate the discriminant of this quadratic to ensure it has real solutions:

\[
D = (4b)^2 - 4 \cdot 1 \cdot (b^2 + 3)
\]
\[
D = 16b^2 - 4(b^2 + 3)
\]
\[
D = 16b^2 - 4b^2 - 12 = 12b^2 - 12 = 12(b^2 - 1)
\]

To have real \(a\), \(b^2 - 1 \geq 0\) or \(b \geq 1\). Thus, we can assume \(b \geq 1\) for valid solutions.

Now, we will manipulate the expression we need to compare with \(\frac{1}{2}\):

\[
P = 2\sqrt{2ab} - \frac{1}{2}a - b
\]

### Step 1: Substitute \(a\)

From our equation, rearranging it gives:

\[
a^2 - 4ab + b^2 + 3 = 0 \implies a^2 - 4ab + (b^2 + 3) = 0
\]

Using the quadratic formula:

\[
a = \frac{4b \pm \sqrt{D}}{2} = 2b \pm \sqrt{3} \sqrt{b^2 - 1}
\]

Thus,

\[
a = 2b \pm \sqrt{3(b^2 - 1)}
\]

Since \(a\) must be positive, we take:

\[
a = 2b + \sqrt{3(b^2 - 1)}
\]

### Step 2: Substitute \(a\) into \(P\)

Now substituting \(a\) into the expression for \(P\):

\[
P = 2\sqrt{2b(2b + \sqrt{3(b^2 - 1)})} - \frac{1}{2}(2b + \sqrt{3(b^2 - 1)}) - b
\]

Simplifying \(P\):

Let \(x = 2b + \sqrt{3(b^2 - 1)}\), then:

\[
P = 2\sqrt{4b^2 + 2b\sqrt{3(b^2 - 1)}} - b - \frac{1}{2}x
\]

To analyze \(P\), we can define a form or numerical substitution to compare with \(\frac{1}{2}\). 

### Step 3: Evaluate \(P\)

For simplicity, substitute \(b = 1\):

\[
P = 2\sqrt{2 \cdot 2} - \frac{1}{2}(2 + 0) - 1 = 4 - 1 - 1 = 2
\]

Since \(P = 2\) and we want to assess:

\[
2 \geq \frac{1}{2}
\]

It holds. Consequently, checking values greater than 1, \(P\) increases as \(b\) increases.

### Conclusion

\[
P \geq \frac{1}{2}
\]

Thus, the blank in the inequality can be filled with \( \geq \).

Finally, we conclude:

'''The answer is (B) $\geq$'''