## Problem

Let $a, b, c$ be positive real numbers such that $a b c = 1$. Consider the following inequality:
$$
\frac{1}{a} + \frac{2}{b} + \frac{1}{c} \quad () \quad 2.
$$

Determine the correct inequality relation to fill in the blank.

Options:

(A) $\leq$ 

(B) $\geq$

(C) $=$ 

(D) $<$

(E) $>$

(F) None of the above

## Query

Task description: Please solve the problem with clear, rigorous, and logically sound steps. At the end of your response, state your answer in exactly this format: 'The answer is (Letter) Symbol', where Letter is one of the given options. Example: 'The answer is (A) $\leq$'.

Problem: Let $a, b, c$ be positive real numbers such that $a b c = 1$. Consider the following inequality:
$$
\frac{1}{a} + \frac{2}{b} + \frac{1}{c} \quad () \quad 2.
$$

Determine the correct inequality relation to fill in the blank.

Options:

(A) $\leq$ 

(B) $\geq$

(C) $=$ 

(D) $<$

(E) $>$

(F) None of the above

Solution:

## Response

To solve the problem, we need to analyze the inequality 

\[
\frac{1}{a} + \frac{2}{b} + \frac{1}{c} \quad () \quad 2
\]

given that \( a, b, c \) are positive real numbers such that \( abc = 1 \).

### Step 1: Express \( a, b, c \)

Since \( abc = 1 \), we can express \( c \) in terms of \( a \) and \( b \):

\[
c = \frac{1}{ab}
\]

### Step 2: Substitute \( c \) in the Inequality

The left-hand side of the inequality becomes:

\[
\frac{1}{a} + \frac{2}{b} + \frac{1}{\frac{1}{ab}} = \frac{1}{a} + \frac{2}{b} + ab
\]

### Step 3: Analyze the Terms

Our goal is to analyze:

\[
\frac{1}{a} + \frac{2}{b} + ab \quad () \quad 2
\]

Let's denote \( x = \frac{1}{a} \) and \( y = \frac{1}{b} \). From the condition \( abc = 1 \), we have:

\[
xyz = 1 \quad \text{where} \quad x = \frac{1}{a}, \quad y = \frac{1}{b}, \quad z = \frac{1}{c}
\]

Substituting \( a \) and \( b \) gives us \( a = \frac{1}{x} \), \( b = \frac{1}{y} \), hence:

\[
z = \frac{1}{\frac{1}{x} \cdot \frac{1}{y}} = xy
\]

### Step 4: Apply the AM-GM Inequality

Now we apply the Arithmetic Mean-Geometric Mean (AM-GM) inequality to the three terms \( \frac{1}{a}, \frac{2}{b}, ab \):

\[
\frac{\frac{1}{a} + \frac{2}{b} + ab}{3} \geq \sqrt[3]{\frac{1}{a} \cdot \frac{2}{b} \cdot ab}
\]

Calculating the product for the geometric mean, we have:

\[
\frac{1}{a} \cdot \frac{2}{b} \cdot ab = 2
\]

So,

\[
\frac{\frac{1}{a} + \frac{2}{b} + ab}{3} \geq \sqrt[3]{2}
\]

Multiplying both sides by 3 gives:

\[
\frac{1}{a} + \frac{2}{b} + ab \geq 3\sqrt[3]{2}
\]

### Step 5: Evaluate \( 3\sqrt[3]{2} \)

Calculating the numeric value of \( \sqrt[3]{2} \):

\[
\sqrt[3]{2} \approx 1.2599 \implies 3\sqrt[3]{2} \approx 3.7797
\]

Since \( 3\sqrt[3]{2} > 2 \), we conclude:

\[
\frac{1}{a} + \frac{2}{b} + ab \geq 3 \sqrt[3]{2} > 2
\]

### Conclusion

Thus, the correct inequality relation that should fill in the blank is:

\[
\frac{1}{a} + \frac{2}{b} + ab \geq 2
\]

Therefore, the answer is 

```plaintext
'The answer is (B) â‰¥'
```