## Problem

Let $a, b, c \geq 0$ be non-negative real numbers such that $a^2 + b + c^2 = 1$. Consider the following inequality:
$$
\frac{1}{1+a^2} + \frac{1}{3(1+b)} + \frac{1}{1+c^2} \quad () \quad \frac{7}{4}.
$$

Determine the correct inequality relation to fill in the blank.

Options:

(A) $\leq$ 

(B) $\geq$

(C) $=$ 

(D) $<$

(E) $>$

(F) None of the above

## Query

Task description: Please solve the problem with clear, rigorous, and logically sound steps. At the end of your response, state your answer in exactly this format: 'The answer is (Letter) Symbol', where Letter is one of the given options. Example: 'The answer is (A) $\leq$'.

Problem: Let $a, b, c \geq 0$ be non-negative real numbers such that $a^2 + b + c^2 = 1$. Consider the following inequality:
$$
\frac{1}{1+a^2} + \frac{1}{3(1+b)} + \frac{1}{1+c^2} \quad () \quad \frac{7}{4}.
$$

Determine the correct inequality relation to fill in the blank.

Options:

(A) $\leq$ 

(B) $\geq$

(C) $=$ 

(D) $<$

(E) $>$

(F) None of the above

Solution:

## Response

To solve the problem, we will analyze the inequality 

\[
\frac{1}{1 + a^2} + \frac{1}{3(1 + b)} + \frac{1}{1 + c^2} \quad () \quad \frac{7}{4}
\]

given the constraint \( a^2 + b + c^2 = 1 \) where \( a, b, c \geq 0 \).

### Step 1: Understanding the constraints

We know that \( a^2 \geq 0 \), \( b \geq 0 \), and \( c^2 \geq 0 \) implies that:

\[
a^2 + b + c^2 = 1
\]

### Step 2: Express variables in terms of one variable

From the condition \( a^2 + b + c^2 = 1 \), we can set:

- \( c^2 = 1 - a^2 - b \)

Thus we can express the left-hand side of the inequality as:

\[
\frac{1}{1 + a^2} + \frac{1}{3(1 + b)} + \frac{1}{1 + (1 - a^2 - b)}
\]

This simplifies \( 1 + c^2 = 1 + (1 - a^2 - b) = 2 - a^2 - b \).

### Step 3: Analyze extremal cases

1. **Case \( a = 0, b = 0, c = 1 \)**:

Substituting these values:

\[
\frac{1}{1 + 0} + \frac{1}{3(1 + 0)} + \frac{1}{1 + 1} = 1 + \frac{1}{3} + \frac{1}{2} = 1 + 0.333 + 0.5 = 1.833
\]

2. **Case \( a = 1, b = 0, c = 0 \)**:

Substituting these values:

\[
\frac{1}{1 + 1} + \frac{1}{3(1 + 0)} + \frac{1}{1 + 0} = \frac{1}{2} + \frac{1}{3} + 1
\]

Calculating this gives us:

\[
\frac{1}{2} + \frac{1}{3} + 1 = 0.5 + 0.333 + 1 = 1.833
\]

3. **Case \( a = 0, b = 1, c = 0 \)**:

Substituting these values gives us:

\[
\frac{1}{1 + 0} + \frac{1}{3(1 + 1)} + \frac{1}{1 + 0} = 1 + \frac{1}{6} + 1 = 2 + 0.1667 = 2.1667
\]

### Step 4: Estimate upper limit

Now we need to see the upper limits of the sums when varying \( a, b, c \) under the constraint \( a^2 + b + c^2 = 1\). We see from our trials that the maximum observed was \( 1.833 \) from both \( a = 0, b = 0, c = 1 \) case and \( a = 1, b = 0, c = 0 \) case which did not exceed \( 2 \). 

### Step 5: Formulating the conclusion

From our evaluations, we can conclude that:

\[
\frac{1}{1 + a^2} + \frac{1}{3(1 + b)} + \frac{1}{1 + c^2} \leq 2
\]

Hence, it suggests that the inequality doesn't reach \( \frac{7}{4} \).

### Conclusion

Thus, filling in the blank:

\[
\frac{1}{1 + a^2} + \frac{1}{3(1 + b)} + \frac{1}{1 + c^2} \quad \leq \quad \frac{7}{4}
\]

This leads us to the final answer:

'The answer is (A) $\leq$'