## Problem

Find the smallest constant $C$ such that for all real numbers $x$ and $y$, the following inequality holds:
$$
x^2 + x + y^2 + y + C \geq x y
$$

## Query

Task description: Please solve the problem with clear, rigorous, and logically sound steps. At the end of your response, state your answer in exactly this format: 'The answer is $C=X$', where X is your calculated numerical bound value. Example: 'The answer is $C=1$'.

Problem: Find the smallest constant $C$ such that for all real numbers $x$ and $y$, the following inequality holds:
$$
x^2 + x + y^2 + y + C \geq x y
$$

Solution:

## Response

To solve the problem, we want to find the smallest constant \( C \) such that the inequality 

\[
x^2 + x + y^2 + y + C \geq xy
\]

holds for all real numbers \( x \) and \( y \). 

### Step 1: Rearranging the Inequality

We can rearrange the inequality as follows:

\[
x^2 + y^2 - xy + x + y + C \geq 0
\]

### Step 2: Analyzing the Quadratic Expression

We define a function \( f(x, y) \):

\[
f(x, y) = x^2 - xy + y^2 + x + y + C
\]

This is a quadratic function in \( x \) and \( y \).

### Step 3: Focusing on \( y \)

To analyze this further, let's first consider \( y \) as a constant and treat \( f \) as a quadratic function in \( x \):

\[
f(x) = x^2 - yx + (y^2 + x + C + y)
\]

The expression is a quadratic in \( x \) of the form \( ax^2 + bx + c \) where:

- \( a = 1 \)
- \( b = -y + 1 \)
- \( c = y^2 + C + y \)

### Step 4: Finding Conditions for Non-Negativity

For the quadratic \( f(x) \) to be non-negative for all \( x \), the discriminant must be non-positive:

\[
D = b^2 - 4ac \leq 0
\]

Calculating the discriminant, we have:

\[
D = (-y + 1)^2 - 4(1)(y^2 + C + y)
\]
\[
= (y^2 - 2y + 1) - 4(y^2 + C + y)
\]
\[
= y^2 - 2y + 1 - 4y^2 - 4C - 4y
\]
\[
= -3y^2 - 6y + 1 - 4C
\]

### Step 5: Setting Discriminant Condition

Set the discriminant less than or equal to zero:

\[
-3y^2 - 6y + 1 - 4C \leq 0
\]

This is a quadratic inequality in \( y \) that must hold for all \( y \). The condition for this quadratic to be non-positive for all \( y \) requires the leading coefficient to be negative (which it is) and the discriminant to be non-positive:

\[
D' = (-6)^2 - 4(-3)(1 - 4C) = 36 + 12(1 - 4C) = 36 + 12 - 48C = 48 - 48C \leq 0
\]

### Step 6: Solving the Discriminant Condition

From \( 48 - 48C \leq 0 \), we have:

\[
48 \leq 48C
\]

Dividing by \( 48 \):

\[
1 \leq C \implies C \geq 1
\]

### Conclusion

Thus, the smallest value for \( C \) such that the inequality holds for all real numbers \( x \) and \( y \) is:

\[
C = 1
\]

Putting this in the required format, we have:

```
'The answer is $C=1$'
```