## Problem

Let $a, b > 0$ and $a + b \leq \frac{3}{2}$. Find the smallest constant $C$ such that the following inequality holds for all $a, b$ satisfying the given constraint:
$$
\frac{a}{a^2+1} + \frac{4b}{b^2+4} \leq C.
$$

## Query

Task description: Please solve the problem with clear, rigorous, and logically sound steps. At the end of your response, state your answer in exactly this format: 'The answer is $C=X$', where X is your calculated numerical bound value. Example: 'The answer is $C=1$'.

Problem: Let $a, b > 0$ and $a + b \leq \frac{3}{2}$. Find the smallest constant $C$ such that the following inequality holds for all $a, b$ satisfying the given constraint:
$$
\frac{a}{a^2+1} + \frac{4b}{b^2+4} \leq C.
$$

Solution:

## Response

To solve the problem, we need to find the smallest constant \( C \) such that

\[
\frac{a}{a^2 + 1} + \frac{4b}{b^2 + 4} \leq C
\]

for all \( a, b > 0 \) under the constraint \( a + b \leq \frac{3}{2} \).

### Step 1: Analyze Each Term

1. **Term involving \( a \)**:
   We first analyze the function \( f(a) = \frac{a}{a^2 + 1} \).
   - Find the maximum of \( f(a) \) for \( a > 0 \).

   To do this, we differentiate \( f(a) \):

   \[
   f'(a) = \frac{(a^2 + 1)(1) - a(2a)}{(a^2 + 1)^2} = \frac{1 - a^2}{(a^2 + 1)^2}
   \]

   Setting \( f'(a) = 0 \) gives \( a^2 = 1 \) or \( a = 1 \) (since \( a > 0 \)).

   Evaluate \( f(a) \) at this critical point:

   \[
   f(1) = \frac{1}{1^2 + 1} = \frac{1}{2}
   \]

   Now, check the limits:

   - As \( a \to 0^+, f(a) \to 0 \).
   - As \( a \to \infty, f(a) \to 0 \).

   Since \( f(a) \) reaches a maximum of \( \frac{1}{2} \) at \( a = 1 \), and this aligns with our constraint \( a + b \leq \frac{3}{2} \).

2. **Term involving \( b \)**:
   Next, analyze the function \( g(b) = \frac{4b}{b^2 + 4} \).
   - Differentiate \( g(b) \):

   \[
   g'(b) = \frac{(b^2 + 4)(4) - 4b(2b)}{(b^2 + 4)^2} = \frac{4b^2 + 16 - 8b^2}{(b^2 + 4)^2} = \frac{16 - 4b^2}{(b^2 + 4)^2}
   \]

   Setting \( g'(b) = 0 \) leads to \( 4b^2 = 16 \), or \( b = 2 \) (note \( b > 0 \)).

   Evaluate \( g(b) \) at this critical point:

   \[
   g(2) = \frac{4 \cdot 2}{2^2 + 4} = \frac{8}{8} = 1
   \]

   Check the limits:

   - As \( b \to 0^+, g(b) \to 0 \).
   - As \( b \to \infty, g(b) \to 0 \).

   Thus, \( g(b) \) reaches a maximum of \( 1 \) at \( b = 2 \).

### Step 2: Applying the Constraint

Given the constraint \( a + b \leq \frac{3}{2} \), we analyze combinations of \( a \) and \( b \) to find the values for \( C \).

1. If \( a = 0 \) and \( b = \frac{3}{2} \):
   \[
   g\left(\frac{3}{2}\right) = \frac{4 \cdot \frac{3}{2}}{\left(\frac{3}{2}\right)^2 + 4} = \frac{6}{\frac{9}{4} + 4} = \frac{6}{\frac{25}{4}} = \frac{24}{25}.
   \]
   So, \( f(0) + g\left(\frac{3}{2}\right) = 0 + \frac{24}{25} = \frac{24}{25} \).

2. If \( a = \frac{3}{2} \) and \( b = 0 \):
   \[
   f\left(\frac{3}{2}\right) = \frac{\frac{3}{2}}{\left(\frac{3}{2}\right)^2 + 1} = \frac{\frac{3}{2}}{\frac{9}{4}+1} = \frac{\frac{3}{2}}{\frac{13}{4}} = \frac{6}{13}.
   \]
   So, \( f\left(\frac{3}{2}\right) + g(0) = \frac{6}{13} + 0 = \frac{6}{13} \).

3. If \( a = 1 \) and \( b = \frac{1}{2} \):
   \[
   f(1) + g\left(\frac{1}{2}\right) = \frac{1}{2} + \frac{4 \cdot \frac{1}{2}}{\left(\frac{1}{2}\right)^2 + 4} = \frac{1}{2} + \frac{2}{\frac{1}{4} + 4} = \frac{1}{2} + \frac{2}{\frac{17}{4}} = \frac{1}{2} + \frac{8}{17}.
   \]
   Evaluating gives:
   \[
   = \frac{17}{34} + \frac{16}{34} = \frac{33}{34}.
   \]

### Step 3: Determine Maximum

Examining the calculated values:

- \( \frac{24}{25} = 0.96 \)
- \( \frac{6}{13} \approx 0.46 \)
- \( \frac{33}{34} \approx 0.97 \)

The maximum constant \( C \) ensuring the inequality holds is:

\[
C = \frac{24}{25}.
\]

### Conclusion

Thus, the smallest constant \( C \) such that the inequality holds for all \( a, b \) satisfying the given constraint is:

```
The answer is $C=\frac{24}{25}$
```