## Problem

Let $x, y$ be positive real numbers such that $x + y = 2$. Determine the smallest constant $C$ such that the following inequality holds for all $x, y$:

$$
x^3 y^3 (x^3 + y^3) \leq C.
$$

## Query

Task description: Please solve the problem with clear, rigorous, and logically sound steps. At the end of your response, state your answer in exactly this format: 'The answer is $C=X$', where X is your calculated numerical bound value. Example: 'The answer is $C=1$'.

Problem: Let $x, y$ be positive real numbers such that $x + y = 2$. Determine the smallest constant $C$ such that the following inequality holds for all $x, y$:

$$
x^3 y^3 (x^3 + y^3) \leq C.
$$

Solution:

## Response

To solve the problem, we need to find the smallest constant \( C \) such that the inequality 

\[
x^3 y^3 (x^3 + y^3) \leq C
\]

holds for all positive \( x \) and \( y \) such that \( x + y = 2 \).

**Step 1: Express \( y \) in terms of \( x \)**

Given \( x + y = 2 \), we can express \( y \) as:

\[
y = 2 - x
\]

**Step 2: Substitute \( y \) into the inequality**

Now, substituting \( y \) into the inequality gives:

\[
x^3 (2 - x)^3 (x^3 + (2 - x)^3)
\]

**Step 3: Simplify the expression**

Next, we need to simplify both \( (2 - x)^3 \) and \( x^3 + (2 - x)^3 \):

1. Expand \( (2 - x)^3 \):

\[
(2 - x)^3 = 8 - 12x + 6x^2 - x^3
\]

2. Now calculate \( x^3 + (2 - x)^3 \):

\[
x^3 + (2 - x)^3 = x^3 + 8 - 12x + 6x^2 - x^3 = 8 - 12x + 6x^2
\]

**Step 4: Set the full expression**

Now, substitute back:

\[
x^3 (2 - x)^3 (8 - 12x + 6x^2)
\]

This leads to:

\[
x^3 (8 - 12x + 6x^2)(8 - 12x + 6x^2)
\]

**Step 5: Evaluate critical points**

To determine \( C \), we must find the maximum value of the expression 

\[
x^3 (2 - x)^3 (8 - 12x + 6x^2)
\]

over the interval \( 0 < x < 2 \).

**Step 6: Use symmetry and substitute \( x = 1 \)**

By symmetry in the problem (since \( x + y = 2 \)), we can evaluate at \( x = 1 \):

\[
y = 1 \implies x^3 y^3 (x^3 + y^3) = 1^3 \cdot 1^3 (1^3 + 1^3) = 1 \cdot 1 \cdot 2 = 2
\]

**Step 7: Test endpoints and explore behavior**

Now, consider endpoints:
1. As \( x \to 0 \) or \( x \to 2 \):
   - The expression tends to 0 because \( x^3 \) or \( y^3 \) will be 0.

**Conclusion: Maximum Value**

The maximum occurs at \( x = 1 \) leading to:

\[
x^3 y^3 (x^3 + y^3) \text{ is maximized at } C = 2
\]

Thus, the smallest constant \( C \) that satisfies the inequality for all \( x, y \) is:

```plaintext
'The answer is $C=2$'
```