## Problem

Let $a, b > 0$ such that $a + b = 1$. Determine the largest constant $C$ such that the following inequality holds for all $a, b$:

$$
\left(a+\frac{1}{a}\right)^2+\left(b+\frac{1}{b}\right)^2 \geq C.
$$

## Query

Task description: Please solve the problem with clear, rigorous, and logically sound steps. At the end of your response, state your answer in exactly this format: 'The answer is $C=X$', where X is your calculated numerical bound value. Example: 'The answer is $C=1$'.

Problem: Let $a, b > 0$ such that $a + b = 1$. Determine the largest constant $C$ such that the following inequality holds for all $a, b$:

$$
\left(a+\frac{1}{a}\right)^2+\left(b+\frac{1}{b}\right)^2 \geq C.
$$

Solution:

## Response

To solve the problem, we need to determine the largest constant \( C \) for which the inequality 

\[
\left(a+\frac{1}{a}\right)^2+\left(b+\frac{1}{b}\right)^2 \geq C
\]

holds true for all \( a, b > 0 \) such that \( a + b = 1 \). 

### Step 1: Analyze the inequality

First, let's rewrite the terms involved in the inequality. We have:

\[
\left(a+\frac{1}{a}\right)^2 + \left(b+\frac{1}{b}\right)^2
\]

We know that \( b = 1 - a \), so we can substitute \( b \) into the expression.

### Step 2: Simplify the expression

Now, letâ€™s denote the expression:

\[
f(a) = \left(a + \frac{1}{a}\right)^2 + \left((1-a) + \frac{1}{1-a}\right)^2
\]

### Step 3: Expand the terms

Expanding \( f(a) \):

\[
f(a) = \left(a + \frac{1}{a}\right)^2 + \left((1-a) + \frac{1}{1-a}\right)^2 
\]

Calculating the first term:

\[
\left(a + \frac{1}{a}\right)^2 = a^2 + 2 + \frac{1}{a^2}
\]

Calculating the second term:

\[
\left((1-a) + \frac{1}{1-a}\right)^2 = (1-a)^2 + 2 + \frac{1}{(1-a)^2}
\]

Thus,

\[
f(a) = a^2 + 2 + \frac{1}{a^2} + (1-a)^2 + 2 + \frac{1}{(1-a)^2}
\]

### Step 4: Combine the terms

Simplifying further:

\[
f(a) = a^2 + (1 - 2a + a^2) + 4 + \frac{1}{a^2} + \frac{1}{(1-a)^2}
\]

\[
f(a) = 2a^2 - 2a + 4 + \frac{1}{a^2} + \frac{1}{(1-a)^2}
\]

### Step 5: Analyze behavior of \( f(a) \)

Next, we can analyze the behavior of \( f(a) \) by checking its values at certain points. 

1. **At \( a = \frac{1}{2} \)**:
   - \( a = b = \frac{1}{2} \):
   \[
   f\left(\frac{1}{2}\right) = \left(\frac{1}{2}+2\right)^2 + \left(\frac{1}{2}+2\right)^2 = 2 \left(\frac{5}{2}\right)^2 = 2 \cdot \frac{25}{4} = \frac{50}{4} = 12.5
   \]

2. **As \( a \) approaches \( 0 \)**:
   - For \( a \to 0^+ \) (and thus \( b \to 1 \)):
   \[
   f(a) \to \text{undefined} \quad (\text{approaches }\infty)
   \]

### Step 6: Find \( C \)

Using the calculation at \( a = \frac{1}{2} \), we find that the minimum value occurs at this point, resulting in:

\[
C \leq 12.5
\]

### Step 7: Conclusion

Thus, the largest constant \( C \) that satisfies 

\[
\left(a+\frac{1}{a}\right)^2+\left(b+\frac{1}{b}\right)^2 \geq C
\]

for all \( a, b > 0 \) such that \( a + b = 1 \) is 

\[
C = 12.5.
\]

### Final Statement

The answer is \( C = 12.5 \).

So, 

```
'The answer is $C=12.5$'
```