## Problem

Let $a > 1$ be a real number. Determine the largest constant $C$ such that for all $n \in \mathbb{N}$, the following inequality holds:
$$
\frac{a^n-1}{n} \geq C\sqrt{a}^{n+1}-\sqrt{a}^{n-1}.
$$

## Query

Task description: Please solve the problem with clear, rigorous, and logically sound steps. At the end of your response, state your answer in exactly this format: 'The answer is $C=X$', where X is your calculated numerical bound value. Example: 'The answer is $C=1$'.

Problem: Let $a > 1$ be a real number. Determine the largest constant $C$ such that for all $n \in \mathbb{N}$, the following inequality holds:
$$
\frac{a^n-1}{n} \geq C\sqrt{a}^{n+1}-\sqrt{a}^{n-1}.
$$

Solution:

## Response

To find the largest constant \( C \) such that the inequality 

\[
\frac{a^n-1}{n} \geq C\sqrt{a}^{n+1}-\sqrt{a}^{n-1}
\]

holds for all \( n \in \mathbb{N} \) where \( a > 1 \), we can analyze the behavior of both sides of the inequality as \( n \) approaches infinity.

### Step 1: Analyze the Left Side

The left-hand side can be rewritten using properties of exponential growth. As \( n \) increases, the term \( a^n \) grows much faster than the constant \( 1 \), giving us:

\[
\frac{a^n - 1}{n} \sim \frac{a^n}{n} \quad \text{(as \( n \to \infty \))}
\]

### Step 2: Analyze the Right Side

Now let's analyze the right-hand side:

\[
C\sqrt{a}^{n+1} - \sqrt{a}^{n-1} = C a^{(n+1)/2} - a^{(n-1)/2}
\]

### Step 3: Establish Dominance

As \( n \to \infty \), the dominant term in this expression is \( C a^{(n+1)/2} \). Thus, we can express our inequalities asymptotically as follows:

\[
\frac{a^n}{n} \geq C a^{(n+1)/2}
\]

### Step 4: Simplify the Inequality

Rearranging gives:

\[
\frac{a^n}{n} \geq C a^{(n+1)/2}
\]
\[
a^n \geq C n a^{(n+1)/2}
\]
\[
a^n \geq C n a^{n/2} a^{1/2}
\]
\[
1 \geq C n a^{-n/2 + 1/2}
\]

### Step 5: Evaluate the Limit

Taking the limit as \( n \to \infty \):

\[
\lim_{n \to \infty} \frac{1}{n a^{-n/2 + 1/2}} = 0
\]

This indicates that we need to analyze for what values of \( C \) this relationship holds as \( n \to \infty \). 

### Step 6: Find the Bound for \( C \)

To maintain the inequality:

\[
n a^{-n/2 + 1/2} \to 0
\]

We can equate the leading powers of \( a \) from both sides:

Setting 

\[
C = a^{1/2}
\]

works under our analysis since substituting into our limit gives us the critical point where the left-hand side can remain larger than or equal to the right-hand side.

### Conclusion

Thus, the largest constant \( C \) such that the inequality holds for all \( n \in \mathbb{N} \) is \( C = a^{1/2} \).

Thus, the final statement is:

```plaintext
The answer is $C=a^{1/2}$
```