## Problem

Let $x, y, z \in [-1, 3]$ such that $x + y + z = 3$. Find the smallest constant $C$ such that the following inequality holds for all $x, y, z$:
$$
x^2 + y^2 + z^2 \leq C.
$$

## Query

Task description: Please solve the problem with clear, rigorous, and logically sound steps. At the end of your response, state your answer in exactly this format: 'The answer is $C=X$', where X is your calculated numerical bound value. Example: 'The answer is $C=1$'.

Problem: Let $x, y, z \in [-1, 3]$ such that $x + y + z = 3$. Find the smallest constant $C$ such that the following inequality holds for all $x, y, z$:
$$
x^2 + y^2 + z^2 \leq C.
$$

Solution:

## Response

To solve the problem, we start with the given constraints and look for the smallest constant \( C \) such that the inequality 

\[
x^2 + y^2 + z^2 \leq C
\]

holds for all \( x, y, z \in [-1, 3] \) with the condition that \( x + y + z = 3 \).

### Step 1: Use the constraint

From the constraint \( x + y + z = 3 \), we can express one of the variables in terms of the other two. Let's express \( z \):

\[
z = 3 - x - y
\]

### Step 2: Substitute into the inequality

Substituting for \( z \), we rewrite \( x^2 + y^2 + z^2 \):

\[
x^2 + y^2 + (3 - x - y)^2
\]

Expanding the squared term:

\[
= x^2 + y^2 + (9 - 6x - 6y + x^2 + y^2 + 2xy)
\]

Combining like terms gives:

\[
= 2x^2 + 2y^2 + 2xy - 6x - 6y + 9
\]

### Step 3: Analysis of bounds

Now, we need to analyze \( 2x^2 + 2y^2 + 2xy - 6x - 6y + 9 \). To find the values of \( x \) and \( y \) that maximize this expression under the constraints \( -1 \leq x, y \leq 3 \) and \( x + y \leq 3 \).

### Step 4: Calculate boundary cases

To find the maximum, we can test combinations of \( x \) and \( y \) at the boundary of the allowed values:

1. **Case 1**: \( x = 3, y = 0 \) (which gives \( z = 0 \)):
   \[
   x^2 + y^2 + z^2 = 3^2 + 0^2 + 0^2 = 9
   \]

2. **Case 2**: \( x = 0, y = 3 \) (which gives \( z = 0 \)):
   \[
   x^2 + y^2 + z^2 = 0^2 + 3^2 + 0^2 = 9
   \]

3. **Case 3**: \( x = 1, y = 1 \) (which gives \( z = 1 \)):
   \[
   x^2 + y^2 + z^2 = 1^2 + 1^2 + 1^2 = 3
   \]
  
4. **Case 4**: \( x = -1, y = 5 \) (not valid since \( y \) exceeds 3).

5. **Case 5**: \( x = 3, y = -1 \) (which gives \( z = 1 \)):
   \[
   x^2 + y^2 + z^2 = 3^2 + (-1)^2 + 1^2 = 9 + 1 + 1 = 11
   \]

### Step 5: Conclude 

From checking these boundary values, the maximum value we found was 11 when \( x = 3 \) and \( y = -1 \).

### Answer

Thus, the smallest constant \( C \) such that the inequality holds for all valid \( x, y, z \) is:

\[
\textbf{The answer is } C = 11.
\]