## Problem

Let $a, b, c \geq 0$ be non-negative real numbers such that $a + b + c = 1$. Consider the following inequality:
$$
7(ab + bc + ca) \quad () \quad 3 + 9abc.
$$

Determine the correct inequality relation to fill in the blank.

Options:

(A) $\leq$ 

(B) $\geq$

(C) $=$ 

(D) $<$

(E) $>$

(F) None of the above

## Query

Task description: Please solve the problem with clear, rigorous, and logically sound steps. At the end of your response, state your answer in exactly this format: 'The answer is (Letter) Symbol', where Letter is one of the given options. Example: 'The answer is (A) $\leq$'.

Problem: Let $a, b, c \geq 0$ be non-negative real numbers such that $a + b + c = 1$. Consider the following inequality:
$$
7(ab + bc + ca) \quad () \quad 3 + 9abc.
$$

Determine the correct inequality relation to fill in the blank.

Options:

(A) $\leq$ 

(B) $\geq$

(C) $=$ 

(D) $<$

(E) $>$

(F) None of the above

Solution:

## Response

To solve the problem, we need to analyze the expression \( 7(ab + bc + ca) \) in relation to \( 3 + 9abc \).

Given the condition \( a + b + c = 1 \) and \( a, b, c \geq 0 \), we will investigate the values for \( ab + bc + ca \) and \( abc \).

1. **Understanding the terms**:
   - The term \( ab + bc + ca \) can be rewritten in terms of \( a, b, c \).
   - The term \( abc \) represents the product of the three non-negative numbers.

2. **Using AM-GM Inequality**:
   The Arithmetic Mean-Geometric Mean (AM-GM) inequality states that:
   \[
   \frac{a + b + c}{3} \geq \sqrt[3]{abc}
   \]
   Substituting \( a + b + c = 1 \):
   \[
   \frac{1}{3} \geq \sqrt[3]{abc} \Rightarrow abc \leq \frac{1}{27}
   \]

3. **Finding \( ab + bc + ca \)**:
   Another application of AM-GM gives:
   \[
   ab + bc + ca \leq \frac{(a + b + c)^2}{3} = \frac{1^2}{3} = \frac{1}{3}.
   \]

4. **Calculating \( 7(ab + bc + ca) \)**:
   Using the upper bound for \( ab + bc + ca \):
   \[
   7(ab + bc + ca) \leq 7 \cdot \frac{1}{3} = \frac{7}{3}.
   \]

5. **Finding \( 3 + 9abc \)**:
   Since \( abc \leq \frac{1}{27} \):
   \[
   9abc \leq 9 \cdot \frac{1}{27} = \frac{1}{3}.
   \]
   Thus:
   \[
   3 + 9abc \leq 3 + \frac{1}{3} = \frac{10}{3}.
   \]

6. **Comparison**:
   Now we compare \( 7(ab + bc + ca) \) and \( 3 + 9abc \):
   \[
   \frac{7}{3} \leq \frac{10}{3} \Rightarrow 7(ab + bc + ca) \leq 3 + 9abc.
   \]

This indicates that we can fill in the blank with the symbol \( \leq \).

Thus, the correct inequality is:
``'The answer is (A) $\leq$'``.