## Problem

Let $a, b, c > 0$ be positive real numbers such that $\frac{1}{a} + \frac{1}{b} + \frac{1}{c} = \sqrt{abc}$. Consider the following inequality:
$$
abc \quad () \quad \sqrt{3(a+b+c)}.
$$
Determine the correct inequality relation to fill in the blank.

Options:

(A) $\leq$ 

(B) $\geq$

(C) $=$ 

(D) $<$

(E) $>$

(F) None of the above

## Query

Task description: Please solve the problem with clear, rigorous, and logically sound steps. At the end of your response, state your answer in exactly this format: 'The answer is (Letter) Symbol', where Letter is one of the given options. Example: 'The answer is (A) $\leq$'.

Problem: Let $a, b, c > 0$ be positive real numbers such that $\frac{1}{a} + \frac{1}{b} + \frac{1}{c} = \sqrt{abc}$. Consider the following inequality:
$$
abc \quad () \quad \sqrt{3(a+b+c)}.
$$
Determine the correct inequality relation to fill in the blank.

Options:

(A) $\leq$ 

(B) $\geq$

(C) $=$ 

(D) $<$

(E) $>$

(F) None of the above

Solution:

## Response

Let's analyze the problem step-by-step.

Given that \( a, b, c > 0 \) and that:

\[
\frac{1}{a} + \frac{1}{b} + \frac{1}{c} = \sqrt{abc},
\]

we can manipulate this equation to gain insights into the relationships between \( a, b, c \) and \( \sqrt{3(a+b+c)} \).

### Step 1: Start with the given equation

The equation can be rewritten in terms of \( xyz \):

\[
\frac{bc + ac + ab}{abc} = \sqrt{abc},
\]

which implies:

\[
bc + ac + ab = abc \sqrt{abc}.
\]

### Step 2: Use the AM-GM Inequality

By applying the Arithmetic Mean-Geometric Mean (AM-GM) inequality, we have:

\[
\frac{a+b+c}{3} \geq \sqrt[3]{abc}.
\]

Multiplying both sides by 3:

\[
a+b+c \geq 3\sqrt[3]{abc}.
\]

### Step 3: Rearrange to express \( abc \)

Now, squaring the earlier inequality gives:

\[
3(a+b+c) \geq 9 \sqrt{abc}.
\]

Thus, we can infer:

\[
abc \leq 3(a+b+c).
\]

### Step 4: Relate \( abc \) and \( \sqrt{3(a+b+c)} \)

To relate \( abc \) to \( \sqrt{3(a+b+c)} \), we know:

\[
\sqrt{3(a+b+c)} = \sqrt{3} \cdot \sqrt{a+b+c}.
\]

Using the previous AM-GM inequality, \( a+b+c \geq 3 \sqrt[3]{abc} \) leads us to consider squaring both sides:

\[
3(a+b+c) \geq 9 \cdot \sqrt[3]{abc} \Longrightarrow \sqrt{3(a+b+c)} \geq 3 \sqrt[6]{abc}.
\]

### Step 5: Final Analysis

To determine if \( abc \leq \sqrt{3(a+b+c)} \) or \( abc \geq \sqrt{3(a+b+c)} \):

Since \( \frac{1}{a} + \frac{1}{b} + \frac{1}{c} = \sqrt{abc} \), this suggests a balance that would imply:

\[
abc \geq \sqrt{3(a+b+c)}.
\]

### Conclusion

Based on our inequality analytic work, we observe that the correct relation is:

\[
abc \geq \sqrt{3(a+b+c)}.
\]

Thus, the answer to the problem is:

```
'The answer is (B) â‰¥'
```