## Problem

Let $a, b, c > 0$ be positive real numbers such that $ab + bc + ca = 1$. Consider the following inequality:
$$
a b c\left(a+\sqrt{a^2+1}\right)\left(b+\sqrt{b^2+1}\right)\left(c+\sqrt{c^2+1}\right) \quad () \quad 2.
$$

Determine the correct inequality relation to fill in the blank.

Options:

(A) $\leq$ 

(B) $\geq$

(C) $=$ 

(D) $<$

(E) $>$

(F) None of the above

## Query

Task description: Please solve the problem with clear, rigorous, and logically sound steps. At the end of your response, state your answer in exactly this format: 'The answer is (Letter) Symbol', where Letter is one of the given options. Example: 'The answer is (A) $\leq$'.

Problem: Let $a, b, c > 0$ be positive real numbers such that $ab + bc + ca = 1$. Consider the following inequality:
$$
a b c\left(a+\sqrt{a^2+1}\right)\left(b+\sqrt{b^2+1}\right)\left(c+\sqrt{c^2+1}\right) \quad () \quad 2.
$$

Determine the correct inequality relation to fill in the blank.

Options:

(A) $\leq$ 

(B) $\geq$

(C) $=$ 

(D) $<$

(E) $>$

(F) None of the above

Solution:

## Response

To solve the problem, we need to determine the relation between the term \( a b c\left(a+\sqrt{a^2+1}\right)\left(b+\sqrt{b^2+1}\right)\left(c+\sqrt{c^2+1}\right) \) and \( 2 \) under the given constraint \( ab + bc + ca = 1 \).

### Step-by-Step Solution:

1. **Understand the Terms**: 
    - Each term \( a + \sqrt{a^2 + 1} \) can be rewritten as \( a + \sqrt{a^2 + 1} \). We note that \( \sqrt{a^2 + 1} \geq a \), hence \( a + \sqrt{a^2 + 1} \geq 2a^{1/2} \).

2. **Combine the Terms**:
    - Thus, we can write:
    \[
    a + \sqrt{a^2 + 1} \geq 2\sqrt{a}
    \]
    - Similarly, for \( b \) and \( c \):
    \[
    b + \sqrt{b^2 + 1} \geq 2\sqrt{b}
    \]
    \[
    c + \sqrt{c^2 + 1} \geq 2\sqrt{c}
    \]

3. **Inequality Formation**:
    - Therefore, we have:
    \[
    (a + \sqrt{a^2 + 1})(b + \sqrt{b^2 + 1})(c + \sqrt{c^2 + 1}) \geq 8 \sqrt{abc}
    \]
    - This follows because we can apply the AM-GM inequality.

4. **Expand the Product**:
    - So:
    \[
    a b c \cdot (a + \sqrt{a^2 + 1})(b + \sqrt{b^2 + 1})(c + \sqrt{c^2 + 1}) \geq 8abc\sqrt{abc} = 8(ab c)^{3/2}
    \]

5. **Substituting the Constraint**:
    - From \( ab + bc + ca = 1 \), we can use symmetry and substitution to analyze \( abc \). Utilizing the arithmetic mean-geometric mean (AM-GM) inequality:
    \[
    \frac{ab + ac + bc}{3} \geq \sqrt[3]{(abc)^2}
    \]
    - We can relate the values of \( a, b, c \) to \( p = abc \).

6. **Bound the Expression**:
    - We know that:
    \[
    abc \leq \left( \frac{ab + ac + bc}{3} \right)^{3/2} \implies abc \leq p
    \]
    - Given \( ab + ac + bc = 1 \) leads to maximum product scenarios where \( \max(abc) \) occurs near equal values of \( a, b, c \).

7. **Final Bound**:
    - Hence, from earlier, we have:
    \[
    a b c\left(a+\sqrt{a^2+1}\right)\left(b+\sqrt{b^2+1}\right)\left(c+\sqrt{c^2+1}\right) \geq 8abc\sqrt{abc}
    \]

8. **Conclusion**:
    - Since \( abc < 1/2 \) from AM-GM application under the constraint \( ab + ac + bc = 1 \): this leads to showing that:
    \[
    8(p)^{3/2} < 2
    \]
    - Hence, this confirms that the product is indeed less than \( 2 \).

### Final Result
After analyzing and calculating, we find:

\[
\text{The answer is (A) } \leq 
\]