## Problem

Let $a, b, c$ be positive real numbers such that $abc = 1$. Consider the following inequality:
$$
\sqrt[3]{a} + \sqrt[3]{b} + \sqrt[3]{c} \quad () \quad \sqrt[3]{3(3 + a + b + c + ab + bc + ca)}.
$$

Determine the correct inequality relation to fill in the blank.

Options:

(A) $\leq$ 

(B) $\geq$

(C) $=$ 

(D) $<$

(E) $>$

(F) None of the above

## Query

Task description: Please solve the problem with clear, rigorous, and logically sound steps. At the end of your response, state your answer in exactly this format: 'The answer is (Letter) Symbol', where Letter is one of the given options. Example: 'The answer is (A) $\leq$'.

Problem: Let $a, b, c$ be positive real numbers such that $abc = 1$. Consider the following inequality:
$$
\sqrt[3]{a} + \sqrt[3]{b} + \sqrt[3]{c} \quad () \quad \sqrt[3]{3(3 + a + b + c + ab + bc + ca)}.
$$

Determine the correct inequality relation to fill in the blank.

Options:

(A) $\leq$ 

(B) $\geq$

(C) $=$ 

(D) $<$

(E) $>$

(F) None of the above

Solution:

## Response

To analyze the inequality 

\[
\sqrt[3]{a} + \sqrt[3]{b} + \sqrt[3]{c} \quad () \quad \sqrt[3]{3(3 + a + b + c + ab + bc + ca)},
\]

given the constraint \(abc = 1\), we can use the Arithmetic Mean-Geometric Mean Inequality (AM-GM).

### Step 1: Applying AM-GM

We know that the AM-GM inequality states:

\[
\frac{x_1 + x_2 + x_3}{3} \geq \sqrt[3]{x_1 x_2 x_3}
\]

for any positive real numbers \(x_1, x_2, x_3\). If we let 

\[
x_1 = \sqrt[3]{a}, \quad x_2 = \sqrt[3]{b}, \quad x_3 = \sqrt[3]{c},
\]

then we have:

\[
\sqrt[3]{a} + \sqrt[3]{b} + \sqrt[3]{c} \geq 3\sqrt[3]{\sqrt[3]{a} \cdot \sqrt[3]{b} \cdot \sqrt[3]{c}} = 3\sqrt[3]{\sqrt[3]{abc}} = 3\sqrt[3]{\sqrt[3]{1}} = 3.
\]

### Step 2: Analyzing the Right Side

Next, we consider the right side of the inequality:

\[
\sqrt[3]{3(3 + a + b + c + ab + bc + ca)}.
\]

Using the condition \(abc = 1\), we apply the AM-GM inequality again on \(a, b, c\):

\[
a + b + c \geq 3\sqrt[3]{abc} = 3,
\]

and since \(ab + ac + bc \geq 3\sqrt[3]{(abc)^2} = 3\), we deduce:

\[
a + b + c + ab + ac + bc \geq 3 + 3 = 6.
\]

### Step 3: Putting It All Together

Thus, we have:

\[
3 + a + b + c + ab + ac + bc \geq 3 + 6 = 9.
\]

Therefore, 

\[
3(3 + a + b + c + ab + ac + bc) \geq 27,
\]

which implies:

\[
\sqrt[3]{3(3 + a + b + c + ab + ac + bc)} \geq 3.
\]

### Step 4: Final Comparison

By summarizing our findings:

1. \(\sqrt[3]{a} + \sqrt[3]{b} + \sqrt[3]{c} \geq 3\).
2. \(\sqrt[3]{3(3 + a + b + c + ab + ac + bc)} \geq 3\).

At this point, since both sides are greater than or equal to 3, we cannot establish a strict inequality but can state that they are equal under the condition \(abc = 1\). 

Thus, we can conclude:

\[
\sqrt[3]{a} + \sqrt[3]{b} + \sqrt[3]{c} = \sqrt[3]{3(3 + a + b + c + ab + ac + bc)}.
\]

### Conclusion

Hence, the correct relationship to fill the blank is 

\[
\boxed{C}
\]

So, the final answer is:

``'The answer is (C) $=$''`.