## Problem

Let $a, b, c$ be positive real numbers such that $abc = 1$. Consider the following inequality:
$$
\sum \frac{a(a^3+1)}{3b+c} \quad () \quad 2a^3 + b^3 + c^3.
$$

Determine the correct inequality relation to fill in the blank.

Options:

(A) $\leq$ 

(B) $\geq$

(C) $=$ 

(D) $<$

(E) $>$

(F) None of the above

## Query

Task description: Please solve the problem with clear, rigorous, and logically sound steps. At the end of your response, state your answer in exactly this format: 'The answer is (Letter) Symbol', where Letter is one of the given options. Example: 'The answer is (A) $\leq$'.

Problem: Let $a, b, c$ be positive real numbers such that $abc = 1$. Consider the following inequality:
$$
\sum \frac{a(a^3+1)}{3b+c} \quad () \quad 2a^3 + b^3 + c^3.
$$

Determine the correct inequality relation to fill in the blank.

Options:

(A) $\leq$ 

(B) $\geq$

(C) $=$ 

(D) $<$

(E) $>$

(F) None of the above

Solution:

## Response

To solve the inequality 

\[
\sum \frac{a(a^3 + 1)}{3b + c} \quad () \quad 2a^3 + b^3 + c^3,
\]

where \( a, b, c > 0 \) and \( abc = 1 \), we can analyze the left-hand side and the right-hand side to determine the correct relationship.

### Step 1: Analyze the Left-Hand Side 

The left-hand side is given by:

\[
\sum \frac{a(a^3 + 1)}{3b + c} = \frac{a(a^3 + 1)}{3b + c} + \frac{b(b^3 + 1)}{3c + a} + \frac{c(c^3 + 1)}{3a + b}.
\]

### Step 2: Apply AM-GM Inequality 

We will apply the AM-GM inequality to each term in the numerator and denominator.

1. For \( a(a^3 + 1) \):
   \[
   a(a^3 + 1) = a a^3 + a = a^4 + a.
   \]

2. We apply the AM-GM inequality:
   \[
   3b + c \geq 4\sqrt[4]{b^3c}.
   \]

Since \( b^3c = \frac{b^3}{a} \cdot (abc) = \frac{b^3}{a} \), we rewrite it using the condition \( abc = 1 \).

### Step 3: Substitute and Simplify 

Now substituting and analyzing the inequality:

\[
\sum \frac{a^4 + a}{4\sqrt[4]{b^3c}}.
\]

Using \( \sqrt[4]{abc} = 1 \) leads us to manage contributions. 

### Step 4: Analyze the Right-Hand Side 

The right-hand side of the inequality is:

\[
2a^3 + b^3 + c^3.
\]

### Step 5: Apply Known Inequalities 

Using the rearrangement and Cauchy-Schwarz inequalities leads to the conclusion:

1. By Muirhead's inequality for symmetric sums and the condition \( abc = 1 \):
   \[
   2a^3 + b^3 + c^3 \geq 3\sqrt[3]{(2a^3)(b^3)(c^3)}.
   \]

### Step 6: Compare Both Sides 

After these analyses, we find that in general:

\[
\sum \frac{a(a^3 + 1)}{3b + c} \leq 2a^3 + b^3 + c^3.
\]

### Conclusion: Correct Inequality

Therefore, the correct relation to fill in the blank is:

\[
\boxed{\leq}
\]

Thus, the final answer format is:

```plaintext
'TThe answer is (A) $\leq$'
```