## Problem

Let $a, b, c$ be non-negative numbers such that $ab + ac + bc \neq 0$. Consider the following inequality:
$$
a^3 + b^3 + c^3 + 2abc + \frac{4a^2b^2c^2}{a^3 + b^3 + c^3 + abc} \quad () \quad \sum_{\text{cyc}}(2a^2b + 3a^2c) .
$$

Determine the correct inequality relation to fill in the blank.

Options:

(A) $\leq$ 

(B) $\geq$

(C) $=$ 

(D) $<$

(E) $>$

(F) None of the above

## Query

Task description: Please solve the problem with clear, rigorous, and logically sound steps. At the end of your response, state your answer in exactly this format: 'The answer is (Letter) Symbol', where Letter is one of the given options. Example: 'The answer is (A) $\leq$'.

Problem: Let $a, b, c$ be non-negative numbers such that $ab + ac + bc \neq 0$. Consider the following inequality:
$$
a^3 + b^3 + c^3 + 2abc + \frac{4a^2b^2c^2}{a^3 + b^3 + c^3 + abc} \quad () \quad \sum_{\text{cyc}}(2a^2b + 3a^2c) .
$$

Determine the correct inequality relation to fill in the blank.

Options:

(A) $\leq$ 

(B) $\geq$

(C) $=$ 

(D) $<$

(E) $>$

(F) None of the above

Solution:

## Response

To solve the problem, we need to analyze the given inequality and its components systematically.

### Step 1: Analyze the Left Side 
The left side of the inequality is \( a^3 + b^3 + c^3 + 2abc + \frac{4a^2b^2c^2}{a^3 + b^3 + c^3 + abc} \).

1. **Simplifying \( a^3 + b^3 + c^3 + 2abc \)**: 
   Using the identity \( a^3 + b^3 + c^3 - 3abc = (a+b+c)(a^2 + b^2 + c^2 - ab - ac - bc) \):
   \[
   a^3 + b^3 + c^3 + 2abc = (a+b+c)(a^2 + b^2 + c^2 - ab - ac - bc) + 5abc
   \]

2. **The second term**: 
   The term \( \frac{4a^2b^2c^2}{a^3 + b^3 + c^3 + abc} \) involves the positivity condition since \( ab + ac + bc \neq 0 \). This implies that the denominator is never zero.

### Step 2: Analyze the Right Side
The right side of the inequality is \( \sum_{\text{cyc}}(2a^2b + 3a^2c) \), which expands to:
\[
2a^2b + 3a^2c + 2b^2c + 3b^2a + 2c^2a + 3c^2b
\]
This is a polynomial in \( a, b, c \), and it represents a symmetric sum where each term involves products of \( a, b, c \).

### Step 3: Comparison of Both Sides
To establish the relationship between both sides, we will employ specific cases of \( a, b, c \):

1. **Case 1**:  Let \( a = b = c = 1 \):
   - Left Side:
     \[
     1^3 + 1^3 + 1^3 + 2(1)(1)(1) + \frac{4(1)(1)(1)}{1 + 1 + 1 + 1} = 3 + 2 + 1 = 6
     \]
   - Right Side:
     \[
     2(1^2)(1) + 3(1^2)(1) + 2(1^2)(1) + 3(1^2)(1) + 2(1^2)(1) + 3(1^2)(1) = 2 + 3 + 2 + 3 + 2 + 3 = 15
     \]
   - Thus, \( 6 \leq 15 \).

2. **Case 2**: Let \( a = 1, b = 1, c = 0 \):
   - Left Side:
     \[
     1^3 + 1^3 + 0 + 2(1)(1)(0) + \frac{4(1)(1)(0)}{1 + 1 + 0 + 0} = 2
     \]
   - Right Side:
     \[
     2(1^2)(1) + 3(1^2)(0) + 2(1^2)(0) + 3(1^2)(1) + 2(0^2)(1) + 3(0^2)(1) = 2 + 0 + 0 + 3 + 0 + 0 = 5
     \]
   - Thus, \( 2 \leq 5 \).

### Conclusion
From the investigations of both cases, we observe that the left side is consistently less than or equal to the right side under the conditions provided.

### Final Result
Thus, our conclusion after analyzing the inequality confirms:
''The answer is (A) $\leq$''