## Problem

Let $a, b, c, d$ be non-negative numbers. Consider the following inequality:
$$
a^4 +2 b^4 + 3c^4 + d^4 + 3abcd \quad () \quad \frac{1}{2} \sum_{cyc} a^3(b+c+d).
$$

Determine the correct inequality relation to fill in the blank.

Options:

(A) $\leq$ 

(B) $\geq$

(C) $=$ 

(D) $<$

(E) $>$

(F) None of the above

## Query

Task description: Please solve the problem with clear, rigorous, and logically sound steps. At the end of your response, state your answer in exactly this format: 'The answer is (Letter) Symbol', where Letter is one of the given options. Example: 'The answer is (A) $\leq$'.

Problem: Let $a, b, c, d$ be non-negative numbers. Consider the following inequality:
$$
a^4 +2 b^4 + 3c^4 + d^4 + 3abcd \quad () \quad \frac{1}{2} \sum_{cyc} a^3(b+c+d).
$$

Determine the correct inequality relation to fill in the blank.

Options:

(A) $\leq$ 

(B) $\geq$

(C) $=$ 

(D) $<$

(E) $>$

(F) None of the above

Solution:

## Response

To solve this inequality, we will analyze each side step by step.

### Step 1: Understanding the inequality

We need to compare the left side:
\[
L = a^4 + 2b^4 + 3c^4 + d^4 + 3abcd
\]
with the right side:
\[
R = \frac{1}{2} \sum_{\text{cyc}} a^3(b+c+d) = \frac{1}{2} (a^3(b+c+d) + b^3(c+d+a) + c^3(d+a+b) + d^3(a+b+c)).
\]

### Step 2: Analyze both sides

1. **Left Side (L)**:
   - This expression consists of non-negative terms since \(a, b, c, d\) are non-negative.

2. **Right Side (R)**:
   - Each term \(a^3(b+c+d)\), \(b^3(c+d+a)\), etc., is also non-negative for non-negative \(a, b, c, d\).
   - The sum collects contributions from all combinations of variables.

### Step 3: Test with specific values

Let's evaluate the inequality with specific values for \(a, b, c, d\).

**Case 1**: Set \(a = b = c = d = 0\).
- \(L = 0\)
- \(R = 0\)
- \(L = R\)

**Case 2**: Set \(a = 1\), \(b = c = d = 0\).
- \(L = 1^4 + 0 + 0 + 0 + 0 = 1\)
- \(R = \frac{1}{2}(1^3(0 + 0 + 0) + 0 + 0 + 0) = 0\)
- Here, \(L > R\)

**Case 3**: Set \(a = b = 1\) and \(c = d = 0\).
- \(L = 1^4 + 2(1^4) + 0 + 0 + 0 = 3\)
- \(R = \frac{1}{2}(1^3(1 + 0 + 0) + 1^3(0 + 0 + 1)) = \frac{1}{2}(1 + 1) = 1\)
- Thus, \(L > R\)

### Step 4: Considering other configurations

Using symmetry in the variables should yield similar results. The term \(3abcd\) becomes more significant when all variables are involved, enhancing the left side.

### Step 5: Drawing a conclusion

Since each specific test case indicates that the left-hand side can grow larger than the right-hand side given sufficient non-zero values, it prompts the conclusion that the inequality holds in the following manner:

From the explored cases, it’s clear that:
\[
L \geq R
\]

### Conclusion

Thus, the answer that correctly fills the blank in this inequality relation is:

```plaintext
'TThe answer is (B) ≥'
```