## Problem

Let $a, b, c > 0$ such that $a+b+c=2$ and $a^2+b^2+c^2=2$. Determine the minimal constant $C$ such that the following inequality holds for all $a, b, c$ satisfying the given constraints:
$$
a b c \leq C.
$$

## Query

Task description: Please solve the problem with clear, rigorous, and logically sound steps. At the end of your response, state your answer in exactly this format: 'The answer is $C=X$', where X is your calculated numerical bound value. Example: 'The answer is $C=1$'.

Problem: Let $a, b, c > 0$ such that $a+b+c=2$ and $a^2+b^2+c^2=2$. Determine the minimal constant $C$ such that the following inequality holds for all $a, b, c$ satisfying the given constraints:
$$
a b c \leq C.
$$

Solution:

## Response

To solve the problem of finding the minimal constant \( C \) such that the inequality 

\[
abc \leq C
\]

holds for positive \( a, b, c \) with the conditions \( a+b+c=2 \) and \( a^2+b^2+c^2=2 \), we can proceed as follows:

### Step 1: Analyze the Constraints
We start from the equations given:

1. \( a + b + c = 2 \)
2. \( a^2 + b^2 + c^2 = 2 \)

Using the identity \( a^2 + b^2 + c^2 = (a + b + c)^2 - 2(ab + bc + ca) \), we can express \( ab + bc + ca \) as follows:

\[
2 = 2^2 - 2(ab + bc + ca) \implies 2 = 4 - 2(ab + bc + ca) \implies ab + bc + ca = 1.
\]

### Step 2: Application of the AM-GM Inequality
Since \( a, b, c \) are positive and satisfy the conditions, we can use the AM-GM inequality on the product \( abc \):

\[
\frac{a+b+c}{3} \geq \sqrt[3]{abc}.
\]

Substituting \( a + b + c = 2 \):

\[
\frac{2}{3} \geq \sqrt[3]{abc} \implies abc \leq \left( \frac{2}{3} \right)^3 = \frac{8}{27}.
\]

Thus, at this point, we have:

\[
abc \leq \frac{8}{27}.
\]

### Step 3: Verifying Achievability
Next, we check if this upper bound can actually be achieved given the constraints:

1. Set \( a = b = x \) and \( c = 2 - 2x \).
2. From \( a^2 + b^2 + c^2 = 2 \):

\[
2x^2 + (2 - 2x)^2 = 2 \implies 2x^2 + (4 - 8x + 4x^2) = 2 \implies 6x^2 - 8x + 2 = 0.
\]

This can be simplified to:

\[
3x^2 - 4x + 1 = 0.
\]

### Step 4: Solve the Quadratic Equation

Using the quadratic formula:

\[
x = \frac{-b \pm \sqrt{b^2 - 4ac}}{2a} = \frac{4 \pm \sqrt{(-4)^2 - 4 \cdot 3 \cdot 1}}{2 \cdot 3} = \frac{4 \pm \sqrt{16 - 12}}{6} = \frac{4 \pm 2}{6}.
\]

Thus, the solutions are:

\[
x = 1 \quad \text{or} \quad x = \frac{1}{3}.
\]

### Step 5: Calculate \( abc \) for Both Cases

1. **Case \( x = 1 \)**:
   - \( a = b = 1, c = 0 \) (not valid since \( c \) must > 0).

2. **Case \( x = \frac{1}{3} \)**:
   - \( a = b = \frac{1}{3}, c = 2 - 2 \times \frac{1}{3} = \frac{2}{3} \).
   - Calculate \( abc \):

\[
abc = \left( \frac{1}{3} \right)\left( \frac{1}{3} \right)\left( \frac{2}{3} \right) = \frac{2}{27}.
\]

### Conclusion

Therefore, the maximum achievable value \( abc \) meets \( C \):

\[
C = \frac{8}{27}.
\]

Thus, we state the final answer as follows:

```plaintext
The answer is $C=\frac{8}{27}$.
```