## Problem

Let $a, b, c \geq 0$ be real numbers such that $a^2 + b^2 + c^2 = 3$. Consider the following inequality:
$$
\sum_{cyc} \frac{a}{a+2} \quad () \quad 1.
$$

Determine the correct inequality relation to fill in the blank.

Options:

(A) $\leq$ 

(B) $\geq$

(C) $=$ 

(D) $<$

(E) $>$

(F) None of the above

## Query

Task description: Please solve the problem with clear, rigorous, and logically sound steps. At the end of your response, state your answer in exactly this format: 'The answer is (Letter) Symbol', where Letter is one of the given options. Example: 'The answer is (A) $\leq$'.

Problem: Let $a, b, c \geq 0$ be real numbers such that $a^2 + b^2 + c^2 = 3$. Consider the following inequality:
$$
\sum_{cyc} \frac{a}{a+2} \quad () \quad 1.
$$

Determine the correct inequality relation to fill in the blank.

Options:

(A) $\leq$ 

(B) $\geq$

(C) $=$ 

(D) $<$

(E) $>$

(F) None of the above

Solution:

## Response

To solve the problem, we need to analyze the cyclical sum of the terms given the constraint \( a^2 + b^2 + c^2 = 3 \) and determine its relation to \( 1 \).

**Step 1: Identify the Terms**

The inequality we are analyzing is:

\[
\sum_{cyc} \frac{a}{a + 2}
\]

This expands to:

\[
\frac{a}{a + 2} + \frac{b}{b + 2} + \frac{c}{c + 2}
\]

**Step 2: Understand the Function Behavior**

Each term \( \frac{x}{x + 2} \) (for \( x \geq 0 \)) can be rewritten as:

\[
\frac{x}{x + 2} = 1 - \frac{2}{x + 2}
\]

Hence, we have:

\[
\sum_{cyc} \frac{a}{a + 2} = 3 - 2\sum_{cyc} \frac{1}{a + 2}
\]

**Step 3: Analyze the Sum**

Since \( a, b, c \geq 0 \), we can infer that \( a + 2 \geq 2 \). Thus:

\[
\frac{1}{a + 2} \leq \frac{1}{2}
\]

which gives us:

\[
\sum_{cyc} \frac{1}{a + 2} \leq \frac{3}{2}
\]

Putting this back into our sum:

\[
3 - 2\sum_{cyc} \frac{1}{a + 2} \geq 3 - 2 \times \frac{3}{2} = 0
\]

**Step 4: Determine the Maximum of the Sum**

Now, we evaluate:

\[
\sum_{cyc} \frac{a}{a + 2} \leq 1 
\]

We need to check if equality holds or if the sum can actually reach \( 1 \). Testing equal values \( a = b = c = 1 \):

\[
\sum_{cyc} \frac{1}{1 + 2} = \sum_{cyc} \frac{1}{3} = 1
\]

Thus, \( \sum_{cyc} \frac{a}{a + 2} = 1 \) is possible.

Additionally, testing cases like \( a = \sqrt{3}, b = c = 0 \):

\[
\frac{\sqrt{3}}{\sqrt{3} + 2} + 0 + 0 < 1
\]
indicates \( < 1 \).

**Conclusion: Inequality Relation**

We deduce from the analysis that the general form holds as \( \sum_{cyc} \frac{a}{a + 2} \) will always be less than or equal to \( 1 \) given the constraints \( a, b, c \geq 0 \). The upper bound equality can only be attained under specific conditions.

Thus, we conclude:

'"'"'The answer is (A) $\leq$'"'"'