## Problem

Let $a, b, c > 0$ be positive real numbers such that $a + b + c = 1$. Consider the following inequality:
$$
5(a^2 + b^2 + c^2) \quad () \quad 6(a^3 + b^3 + c^3) + 1.
$$

Determine the correct inequality relation to fill in the blank.

Options:

(A) $\leq$ 

(B) $\geq$

(C) $=$ 

(D) $<$

(E) $>$

(F) None of the above

## Query

Task description: Please solve the problem with clear, rigorous, and logically sound steps. At the end of your response, state your answer in exactly this format: 'The answer is (Letter) Symbol', where Letter is one of the given options. Example: 'The answer is (A) $\leq$'.

Problem: Let $a, b, c > 0$ be positive real numbers such that $a + b + c = 1$. Consider the following inequality:
$$
5(a^2 + b^2 + c^2) \quad () \quad 6(a^3 + b^3 + c^3) + 1.
$$

Determine the correct inequality relation to fill in the blank.

Options:

(A) $\leq$ 

(B) $\geq$

(C) $=$ 

(D) $<$

(E) $>$

(F) None of the above

Solution:

## Response

To solve the inequality \( 5(a^2 + b^2 + c^2) \quad () \quad 6(a^3 + b^3 + c^3) + 1 \) under the condition that \( a + b + c = 1 \) where \( a, b, c > 0 \), we will follow these steps:

1. **Use the condition**: Since \( a + b + c = 1 \), we can use the identity that relates the sums of squares and cubes:
   \[
   a^2 + b^2 + c^2 = (a + b + c)^2 - 2(ab + bc + ca) = 1 - 2(ab + ac + bc)
   \]
   and
   \[
   a^3 + b^3 + c^3 = (a + b + c)(a^2 + b^2 + c^2 - ab - ac - bc) = a^2 + b^2 + c^2 - ab - ac - bc
   \]

2. **Apply the Cauchy-Schwarz inequality**: By Cauchy-Schwarz, we have:
   \[
   (a^2 + b^2 + c^2)(1 + 1 + 1) \geq (a + b + c)^2
   \]
   Hence,
   \[
   3(a^2 + b^2 + c^2) \geq 1 \implies a^2 + b^2 + c^2 \geq \frac{1}{3}
   \]
   Therefore,
   \[
   5(a^2 + b^2 + c^2) \geq \frac{5}{3}
   \]

3. **Calculate \( a^3 + b^3 + c^3 \)**: We can apply the known inequality that for non-negative \( a, b, c \):
   \[
   a^3 + b^3 + c^3 \leq a^2 + b^2 + c^2
   \]
   Thus,
   \[
   6(a^3 + b^3 + c^3) \leq 6(a^2 + b^2 + c^2)
   \]

4. **Comparing both expressions**: 
   Using the previous results and substituting \( a^3 + b^3 + c^3 \) into the inequality yields:
   \[
   6(a^3 + b^3 + c^3) + 1 \leq 6 \cdot \frac{1}{3} + 1 = 2 + 1 = 3.
   \]

5. **Final inequality check**: Now we have:
   \[
   5(a^2 + b^2 + c^2) \geq \frac{5}{3}
   \]
   while:
   \[
   6(a^3 + b^3 + c^3) + 1 \leq 3.
   \]
   
   Since \( \frac{5}{3} \) is approximately \( 1.67 \), it is less than \( 3 \).

Thus, the final inequality relation is:
\[
5(a^2 + b^2 + c^2) \leq 6(a^3 + b^3 + c^3) + 1.
\]

Consequently, the answer is:
```plaintext
'TThe answer is (A) $\leq$'   
```