## Problem

Let $a, b, c$ be positive real numbers such that $a + b + c = 1$. Consider the following inequality:
$$
a \sqrt[3]{1+b-c} + b \sqrt[3]{1+c-a} + c \sqrt[3]{1+a-b} \quad () \quad 1.
$$

Determine the correct inequality relation to fill in the blank.

Options:

(A) $\leq$ 

(B) $\geq$

(C) $=$ 

(D) $<$

(E) $>$

(F) None of the above

## Query

Task description: Please solve the problem with clear, rigorous, and logically sound steps. At the end of your response, state your answer in exactly this format: 'The answer is (Letter) Symbol', where Letter is one of the given options. Example: 'The answer is (A) $\leq$'.

Problem: Let $a, b, c$ be positive real numbers such that $a + b + c = 1$. Consider the following inequality:
$$
a \sqrt[3]{1+b-c} + b \sqrt[3]{1+c-a} + c \sqrt[3]{1+a-b} \quad () \quad 1.
$$

Determine the correct inequality relation to fill in the blank.

Options:

(A) $\leq$ 

(B) $\geq$

(C) $=$ 

(D) $<$

(E) $>$

(F) None of the above

Solution:

## Response

We are given the inequality involving positive real numbers \(a\), \(b\), and \(c\) such that \(a + b + c = 1\), and we want to analyze:

\[
a \sqrt[3]{1+b-c} + b \sqrt[3]{1+c-a} + c \sqrt[3]{1+a-b} \quad () \quad 1
\]

**Step 1: Understanding the Expression**

We recognize \(1+b-c\), \(1+c-a\), and \(1+a-b\) can be rewritten:

- Since \(c = 1 - a - b\), we have:
  - \(1 + b - c = 1 + b - (1 - a - b) = a + 2b\)
  - \(1 + c - a = 1 + (1 - a - b) - a = 2 - 2a - b\)
  - \(1 + a - b = 1 + a - b = 1 + a - b\)

Thus, we can rewrite our expression as:

\[
a \sqrt[3]{a + 2b} + b \sqrt[3]{2 - 2a - b} + c \sqrt[3]{1+a-b}
\]

**Step 2: Analyze the Bound**

We evaluate if the left-hand side can exceed, meet, or be less than 1 under the given constraints. 

**Step 3: Applying Cauchy-Schwarz Inequality**

Using the Cauchy-Schwarz inequality in the following form:
- For non-negative reals \(x_1, x_2, \ldots, x_n\) and \(y_1, y_2,\ldots, y_n\):

\[
\left( \sum_{i=1}^n x_i y_i \right)^2 \leq \left( \sum_{i=1}^n x_i^2 \right) \left( \sum_{i=1}^n y_i^2 \right)
\]

We apply Cauchy-Schwarz to:

\[
\left( a \sqrt[3]{1+b-c} + b \sqrt[3]{1+c-a} + c \sqrt[3]{1+a-b} \right)^2 \leq (a^2 + b^2 + c^2) \left( (1+b-c)^{2/3} + (1+c-a)^{2/3} + (1+a-b)^{2/3} \right)
\]

For \( a+b+c = 1 \):

1. Using **AM-GM Inequality** for positive \(a, b, c\) confirms \(a^2 + b^2 + c^2 \leq (a+b+c)^2 = 1\).

2. We notice evaluations lead towards getting bounds but focusing must shift toward sums of cube roots.

**Step 4: Examine Special Cases**

Let's examine \(a = b = c = \frac{1}{3}\):

\[
\text{then,}\\
a + b + c = 1 \\
a \sqrt[3]{1+b-c} + b \sqrt[3]{1+c-a} + c \sqrt[3]{1+a-b} = 3 \cdot \frac{1}{3} \sqrt[3]{1 + \frac{1}{3} - \frac{1}{3}} = \sqrt[3]{1} = 1
\]

This suffices to show equality can be achieved when \(a = b = c\).

**Conclusion**

The determined relation is that the left-hand side can indeed be equal to \(1\) under appropriate pairings of \(a, b, c\). Thus the inequality does not exceed or go less than:

\[
\Rightarrow \text{Therefore, the answer is } \boxed{C}.
\]

Thus, putting it in the required format:

```
'The answer is (C) $=$'
```