## Problem

Let $x, y, z \in \mathbb{R}$. Consider the following expression:
$$
\frac{x^2-y^2}{2x^2+1} + \frac{y^2-z^2}{2y^2+1} + \frac{z^2-x^2}{2z^2+1} \quad () \quad 0.
$$

Determine the correct inequality relation to fill in the blank.

Options:

(A) $\leq$ 

(B) $\geq$

(C) $=$ 

(D) $<$

(E) $>$

(F) None of the above

## Query

Task description: Please solve the problem with clear, rigorous, and logically sound steps. At the end of your response, state your answer in exactly this format: 'The answer is (Letter) Symbol', where Letter is one of the given options. Example: 'The answer is (A) $\leq$'.

Problem: Let $x, y, z \in \mathbb{R}$. Consider the following expression:
$$
\frac{x^2-y^2}{2x^2+1} + \frac{y^2-z^2}{2y^2+1} + \frac{z^2-x^2}{2z^2+1} \quad () \quad 0.
$$

Determine the correct inequality relation to fill in the blank.

Options:

(A) $\leq$ 

(B) $\geq$

(C) $=$ 

(D) $<$

(E) $>$

(F) None of the above

Solution:

## Response

To solve the inequality 

\[
S = \frac{x^2-y^2}{2x^2+1} + \frac{y^2-z^2}{2y^2+1} + \frac{z^2-x^2}{2z^2+1},
\]

we can analyze each term individually.

### Step 1: Understanding Each Term

Each term in the expression can be rewritten in terms of a difference divided by a sum that is always positive:

1. \(\frac{x^2 - y^2}{2x^2 + 1}\)
2. \(\frac{y^2 - z^2}{2y^2 + 1}\)
3. \(\frac{z^2 - x^2}{2z^2 + 1}\)

### Step 2: Applying the Cauchy-Schwarz Inequality

Using Cauchy-Schwarz inequality would be beneficial here. We can state the Cauchy-Schwarz inequality in the following form:

\[
(a_1^2 + a_2^2 + a_3^2)(b_1^2 + b_2^2 + b_3^2) \geq (a_1b_1 + a_2b_2 + a_3b_3)^2
\]

For our analysis, we will take \( a_1 = x^2, a_2 = y^2, a_3 = z^2 \) and \( b_1 = \frac{1}{2x^2 + 1}, b_2 = \frac{1}{2y^2 + 1}, b_3 = \frac{1}{2z^2 + 1} \).

### Step 3: Finding Boundaries

Each fraction \( \frac{a-b}{c} \) behaves particularly around these points. Notably, we will evaluate:

- If \( x^2 \geq y^2 \), then \( x^2 - y^2 \geq 0 \) which implies \( \frac{x^2 - y^2}{2x^2 + 1} \geq 0 \).
- Continuing this reasoning for \( y^2 - z^2 \) and \( z^2 - x^2 \), we can analyze overall behavior based on the values of \( x, y, z \).

### Step 4: Conclusion

By evaluating possibilities through symmetry and cases (e.g. setting \( x = y = z \)), we find that the contributions from each section adequately balance out relative to the denominators, leading to:

\[
S \leq 0
\]

Thus, the correct inequality that fills in the blank is 

\[
\text{The answer is (A) } \leq.
\] 

So, the final answer is: 

```
'The answer is (A) $\leq$'
```