## Problem

Let $a, b, c > 0$ be positive real numbers such that $a + b + c = 3$. Consider the following inequality:
$$
a^2 + 4b^2 + 4b + 8c \quad () \quad 7 + 2\sqrt{2(b^2 + c^2)} + 4\sqrt{bc}.
$$

Determine the correct inequality relation to fill in the blank.

Options:

(A) $\leq$ 

(B) $\geq$

(C) $=$ 

(D) $<$

(E) $>$

(F) None of the above

## Query

Task description: Please solve the problem with clear, rigorous, and logically sound steps. At the end of your response, state your answer in exactly this format: 'The answer is (Letter) Symbol', where Letter is one of the given options. Example: 'The answer is (A) $\leq$'.

Problem: Let $a, b, c > 0$ be positive real numbers such that $a + b + c = 3$. Consider the following inequality:
$$
a^2 + 4b^2 + 4b + 8c \quad () \quad 7 + 2\sqrt{2(b^2 + c^2)} + 4\sqrt{bc}.
$$

Determine the correct inequality relation to fill in the blank.

Options:

(A) $\leq$ 

(B) $\geq$

(C) $=$ 

(D) $<$

(E) $>$

(F) None of the above

Solution:

## Response

To solve the problem, we need to establish the relationship between \( a^2 + 4b^2 + 4b + 8c \) and \( 7 + 2\sqrt{2(b^2 + c^2)} + 4\sqrt{bc} \) given the constraint \( a + b + c = 3 \).

### Step 1: Substitute \( a \)

Since \( a + b + c = 3 \), we can express \( a \) in terms of \( b \) and \( c \):
\[
a = 3 - b - c
\]

Now, let's substitute this expression into our inequality.

### Step 2: Expand Left Side

The left-hand side becomes:
\[
(3 - b - c)^2 + 4b^2 + 4b + 8c
\]
Expanding \( (3 - b - c)^2 \):
\[
= 9 - 6b - 6c + b^2 + 2bc + c^2
\]
Thus, combining all terms, we have:
\[
9 - 6b - 6c + b^2 + 2bc + c^2 + 4b^2 + 4b + 8c
\]
\[
= 9 + (4b^2 + b^2) + (2bc) + (4b - 6b) + (8c - 6c)
\]
\[
= 9 + 5b^2 + 2bc - 2b + 2c
\]

### Step 3: Simplifying the Right Side

We turn our attention to the right-hand side:

\[
7 + 2\sqrt{2(b^2 + c^2)} + 4\sqrt{bc}
\]

Rearranging our original inequality:
\[
9 + 5b^2 + 2bc - 2b + 2c \quad ? \quad 7 + 2\sqrt{2(b^2 + c^2)} + 4\sqrt{bc}
\]

### Step 4: Analyze Special Cases

Letâ€™s analyze specific cases to test the hypothesis.

#### Case 1: \( a = 1, b = 1, c = 1 \)

\[
\text{Left: } 1^2 + 4(1^2) + 4(1) + 8(1) = 1 + 4 + 4 + 8 = 17
\]
\[
\text{Right: } 7 + 2\sqrt{2(1^2 + 1^2)} + 4\sqrt{1 \cdot 1} = 7 + 2\sqrt{4} + 4 = 7 + 4 + 4 = 15
\]
Here \( 17 > 15 \).

#### Case 2: \( b = 0, c = 3, a = 0 \)

\[
\text{Left: } 0 + 4(0^2) + 4(0) + 8(3) = 24
\]
\[
\text{Right: } 7 + 2\sqrt{2(0^2 + 3^2)} + 4\sqrt{0 \cdot 3} = 7 + 2\sqrt{18} = 7 + 6 = 13
\]
Here \( 24 > 13 \).

#### Generalizing

Both cases indicate that the left side tends to dominate. To formulate a conclusion, notice that as \( a, b, c \) vary while satisfying their constraints, you can observe the inequality:

\[
LHS > RHS
\]

### Conclusion

After testing specific cases and reasoning through the general expressions and their possible configurations, we can conjecture:

Therefore, the correct relationship to fill in the blank is:

```plaintext
'The answer is (B) >'
```