## Problem

Let $a, b, c \geq 0$ be non-negative real numbers such that $a + b + c = 1$. Consider the following inequality:
$$
a^3 + b^3 + c^3 + 6abc \quad () \quad \frac{1}{3}.
$$

Determine the correct inequality relation to fill in the blank.

Options:

(A) $\leq$ 

(B) $\geq$

(C) $=$ 

(D) $<$

(E) $>$

(F) None of the above

## Query

Task description: Please solve the problem with clear, rigorous, and logically sound steps. At the end of your response, state your answer in exactly this format: 'The answer is (Letter) Symbol', where Letter is one of the given options. Example: 'The answer is (A) $\leq$'.

Problem: Let $a, b, c \geq 0$ be non-negative real numbers such that $a + b + c = 1$. Consider the following inequality:
$$
a^3 + b^3 + c^3 + 6abc \quad () \quad \frac{1}{3}.
$$

Determine the correct inequality relation to fill in the blank.

Options:

(A) $\leq$ 

(B) $\geq$

(C) $=$ 

(D) $<$

(E) $>$

(F) None of the above

Solution:

## Response

To solve the problem, we'll start by analyzing the expression given in the inequality: 

\[
a^3 + b^3 + c^3 + 6abc 
\]

Given \( a + b + c = 1 \) and \( a, b, c \geq 0 \), we'll use some known results from algebra. We'll utilize the identity for the sum of cubes and some properties of symmetric sums.

### Step 1: Applying the Power Mean Inequality

Using the Power Mean Inequality, we have 

\[
\sqrt[3]{\frac{a^3 + b^3 + c^3}{3}} \geq \frac{a + b + c}{3}
\]

This implies:

\[
a^3 + b^3 + c^3 \geq \frac{(a+b+c)^3}{3^2} = \frac{1}{3}
\]

since we know \( a + b + c = 1 \).

### Step 2: Analyzing the term \( 6abc \)

We will use the AM-GM inequality on \( a + b + c \):

\[
\frac{a + b + c}{3} \geq \sqrt[3]{abc}
\]

which gives us:

\[
abc \leq \left(\frac{1}{3}\right)^3 = \frac{1}{27}
\]

Thus:

\[
6abc \leq 6 \cdot \frac{1}{27} = \frac{2}{9}
\]

### Step 3: Combining results

From Step 1, we have \( a^3 + b^3 + c^3 \geq \frac{1}{3} \). Now we consider:

\[
a^3 + b^3 + c^3 + 6abc \geq \frac{1}{3} + 0 = \frac{1}{3} 
\]

Now assume \( c = 0 \) and \( a + b = 1 \). Then \( a^3 + b^3 + 6abc = a^3 + b^3 \).

Using the power mean inequality for only \( a \) and \( b \):

\[
\frac{a^3 + b^3}{2} \geq \left(\frac{a + b}{2}\right)^3 = \left(\frac{1}{2}\right)^3 = \frac{1}{8}
\]

Thus, \( a^3 + b^3 \geq \frac{1}{4} \).

### Step 4: Testing equality cases

Looking at the extremes, when \( a = 1, b = 0, c = 0 \):

\[
a^3 + b^3 + c^3 + 6abc = 1 + 0 + 0 + 0 = 1
\]

When \( \frac{1}{3} < 1 \), the inequality can hold. Here the maximum value could be above \( \frac{1}{3} + 0 \).

### Conclusion

Finally, based on this reasoning, we conclude:

\[
a^3 + b^3 + c^3 + 6abc \geq \frac{1}{3} 
\]

Thus, the correct relation is:

\[
\text{The answer is (B) } \geq
\]