## Problem

Let $a, b, c \neq 0$ be non-zero real numbers such that $a^2 + b^2 + c^2 = 2(ab + bc + ca)$. Consider the following expression:
$$
(a+b+c)\left(\frac{1}{2a}+\frac{1}{3b}+\frac{1}{c}\right) \quad () \quad 14.
$$

Determine the correct inequality relation to fill in the blank.

Options:

(A) $\leq$ 

(B) $\geq$

(C) $=$ 

(D) $<$

(E) $>$

(F) None of the above

## Query

Task description: Please solve the problem with clear, rigorous, and logically sound steps. At the end of your response, state your answer in exactly this format: 'The answer is (Letter) Symbol', where Letter is one of the given options. Example: 'The answer is (A) $\leq$'.

Problem: Let $a, b, c \neq 0$ be non-zero real numbers such that $a^2 + b^2 + c^2 = 2(ab + bc + ca)$. Consider the following expression:
$$
(a+b+c)\left(\frac{1}{2a}+\frac{1}{3b}+\frac{1}{c}\right) \quad () \quad 14.
$$

Determine the correct inequality relation to fill in the blank.

Options:

(A) $\leq$ 

(B) $\geq$

(C) $=$ 

(D) $<$

(E) $>$

(F) None of the above

Solution:

## Response

To solve the problem, we start by analyzing the equation given:

\[
a^2 + b^2 + c^2 = 2(ab + bc + ca)
\]

This can be rearranged as:

\[
a^2 + b^2 + c^2 - 2(ab + bc + ca) = 0
\]

This implies that:

\[
\frac{1}{2}(a-b)^2 + \frac{1}{2}(b-c)^2 + \frac{1}{2}(c-a)^2 = 0
\]

Thus, \(a = b = c\).

Next, we proceed with the expression given:

\[
(a+b+c)\left(\frac{1}{2a}+\frac{1}{3b}+\frac{1}{c}\right)
\]

Substituting \(a = b = c\) into the expression:

Let \(a = b = c = k\) (for some non-zero real number \(k\)). Then:

\[
a + b + c = 3k
\]

Now, substituting into the second part:

\[
\frac{1}{2a} + \frac{1}{3b} + \frac{1}{c} = \frac{1}{2k} + \frac{1}{3k} + \frac{1}{k}
\]

To combine the fractions, we can find a common denominator, which is \(6k\):

\[
\frac{3}{6k} + \frac{2}{6k} + \frac{6}{6k} = \frac{11}{6k}
\]

Now, substituting back into our expression:

\[
(3k) \left(\frac{11}{6k}\right) = \frac{33k}{6} = \frac{11k}{2}
\]

We need to determine the inequality:

\[
\frac{11k}{2} \quad \text{and} \quad 14
\]

Setting up the inequality:

\[
\frac{11k}{2} \geq 14
\]

To solve for \(k\), we can rewrite this:

\[
11k \geq 28
\]

This gives us:

\[
k \geq \frac{28}{11}
\]

Since \(k\) is a positive real number, the inequality above holds. Thus:

\[
\frac{11k}{2} \geq 14 \quad \text{when} \quad k \geq \frac{28}{11}
\]

Since we stipulated that \(a, b, c \neq 0\), any positive value of \(k\) can be greater than or equal to this threshold.

### Conclusion

Therefore, the expression we have established supports the conclusion that:

\[
(a+b+c)\left(\frac{1}{2a}+\frac{1}{3b}+\frac{1}{c}\right) \geq 14.
\]

Thus, the correct choice to fill in the blank is:

'"'"'The answer is (B) $\geq$'"'"'.