## Problem

Let $a, b > 0$ be positive real numbers such that $a + b \leq \frac{3}{2}$. Consider the following inequality:
$$
\frac{a}{2a^2+1} + \frac{4b}{3b^2+4} \quad () \quad \frac{7}{5}.
$$

Determine the correct inequality relation to fill in the blank.

Options:

(A) $\leq$ 

(B) $\geq$

(C) $=$ 

(D) $<$

(E) $>$

(F) None of the above

## Query

Task description: Please solve the problem with clear, rigorous, and logically sound steps. At the end of your response, state your answer in exactly this format: 'The answer is (Letter) Symbol', where Letter is one of the given options. Example: 'The answer is (A) $\leq$'.

Problem: Let $a, b > 0$ be positive real numbers such that $a + b \leq \frac{3}{2}$. Consider the following inequality:
$$
\frac{a}{2a^2+1} + \frac{4b}{3b^2+4} \quad () \quad \frac{7}{5}.
$$

Determine the correct inequality relation to fill in the blank.

Options:

(A) $\leq$ 

(B) $\geq$

(C) $=$ 

(D) $<$

(E) $>$

(F) None of the above

Solution:

## Response

Let's analyze the given inequality problem step-by-step.

### Problem Breakdown:
We want to compare:

\[
\frac{a}{2a^2+1} + \frac{4b}{3b^2+4}
\]

with 

\[
\frac{7}{5}
\]

given that \( a, b > 0 \) and \( a + b \leq \frac{3}{2} \).

### Step 1: Analyze Each Component

1. **Component \(\frac{a}{2a^2 + 1}\)**:
   
   We will analyze the function \( f(a) = \frac{a}{2a^2 + 1} \). To find its maximum, we take the derivative:

   \[
   f'(a) = \frac{(2a^2 + 1) \cdot 1 - a \cdot 4a}{(2a^2 + 1)^2} = \frac{2a^2 + 1 - 4a^2}{(2a^2 + 1)^2} = \frac{-2a^2 + 1}{(2a^2 + 1)^2}
   \]

   Setting \( f'(a) = 0 \) gives \( -2a^2 + 1 = 0 \) or \( a^2 = \frac{1}{2} \) leading to \( a = \frac{1}{\sqrt{2}} \). 

   Now, we evaluate \( f(a) \) at this critical point:
   
   \[
   f\left(\frac{1}{\sqrt{2}}\right) = \frac{\frac{1}{\sqrt{2}}}{2\left(\frac{1}{2}\right) + 1} = \frac{\frac{1}{\sqrt{2}}}{2} = \frac{1}{2\sqrt{2}} = \frac{\sqrt{2}}{4} \approx 0.354
   \]

2. **Component \(\frac{4b}{3b^2 + 4}\)**:

   Similarly, analyze \( g(b) = \frac{4b}{3b^2 + 4} \). We calculate its maximum using the derivative:

   \[
   g'(b) = \frac{(3b^2 + 4)\cdot 4 - 4b\cdot 6b}{(3b^2 + 4)^2} = \frac{12b^2 + 16 - 24b^2}{(3b^2 + 4)^2} = \frac{-12b^2 + 16}{(3b^2 + 4)^2}
   \]

   Setting \( g'(b) = 0 \) gives \( -12b^2 + 16 = 0 \) leading to \( b^2 = \frac{4}{3} \), so \( b = \frac{2}{\sqrt{3}} \).

   Evaluating \( g(b) \) at this critical point:

   \[
   g\left(\frac{2}{\sqrt{3}}\right) = \frac{4 \cdot \frac{2}{\sqrt{3}}}{3\left(\frac{4}{3}\right) + 4} = \frac{\frac{8}{\sqrt{3}}}{4 + 4} = \frac{8}{8\sqrt{3}} = \frac{1}{\sqrt{3}} \approx 0.577
   \]

### Step 2: Sum of the Maximums

Now we add both components at their potential maximums to check against \( \frac{7}{5} \):

\[
\frac{a}{2a^2 + 1} + \frac{4b}{3b^2 + 4} \approx 0.354 + 0.577 = 0.931
\]

Calculating \( \frac{7}{5} \) gives:

\[
\frac{7}{5} = 1.4
\]

### Conclusion

From the above analysis:

\[
\frac{a}{2a^2 + 1} + \frac{4b}{3b^2 + 4} \leq 0.931 < 1.4
\]

Thus, the correct inequality relation to fill in the blank is 

\[
\boxed{\leq}
\]

### Final Answer

Therefore, the answer is:

```plaintext
'TThe answer is (A) $\leq$'
```