## Problem

Let $a, b, c > 0$. Find the largest constant $C$ such that the following inequality holds for all $a, b, c \in \mathbb{R}^{+}$:
$$
\frac{1}{b(a+b)}+\frac{1}{c(b+c)}+\frac{1}{a(c+a)} \geq \frac{C}{(a+b+c)^2}
$$

## Query

Task description: Please solve the problem with clear, rigorous, and logically sound steps. At the end of your response, state your answer in exactly this format: 'The answer is $C=X$', where X is your calculated numerical bound value. Example: 'The answer is $C=1$'.

Problem: Let $a, b, c > 0$. Find the largest constant $C$ such that the following inequality holds for all $a, b, c \in \mathbb{R}^{+}$:
$$
\frac{1}{b(a+b)}+\frac{1}{c(b+c)}+\frac{1}{a(c+a)} \geq \frac{C}{(a+b+c)^2}
$$

Solution:

## Response

To solve the problem, we want to find the largest constant \( C \) such that the inequality

\[
\frac{1}{b(a+b)}+\frac{1}{c(b+c)}+\frac{1}{a(c+a)} \geq \frac{C}{(a+b+c)^2}
\]

holds for all positive \( a, b, c \).

### Step 1: Analyze the Left Side

Consider the left-hand side of the inequality:

\[
LHS = \frac{1}{b(a+b)}+\frac{1}{c(b+c)}+\frac{1}{a(c+a)}.
\]

We can rewrite each term. For instance, 

\[
\frac{1}{b(a+b)} = \frac{1}{a(b+c)} + \frac{1}{c(a+b)} + \frac{1}{a(c+a)}.
\]

### Step 2: Apply Titu's Lemma

Using Cauchy-Schwarz inequality (also known as Titu's Lemma), we have:

\[
\frac{1}{b(a+b)} + \frac{1}{c(b+c)} + \frac{1}{a(c+a)} \geq \frac{(1+1+1)^2}{b(a+b) + c(b+c) + a(c+a)}.
\]

Thus,

\[
LHS \geq \frac{9}{b(a+b) + c(b+c) + a(c+a)}.
\]

### Step 3: Simplifying the Denominator

To explore \( b(a+b) + c(b+c) + a(c+a) \):

\[
b(a+b) + c(b+c) + a(c+a) = ab + b^2 + bc + cb + c^2 + ac + ac + a^2 = ab + bc + ca + a^2 + b^2 + c^2.
\]

### Step 4: Finding a Relationship

To finalize, recognize that:

- By AM-GM inequality, we have: 
\[
\frac{a^2 + b^2 + c^2}{3} \geq \frac{(a+b+c)^2}{3}.
\]
This implies \( a^2 + b^2 + c^2 \geq \frac{(a+b+c)^2}{3} \).

This means:

\[
ab + bc + ca \leq \frac{(a+b+c)^2}{3}.
\]

### Step 5: Combine Results

From Titu's Lemma:

\[
LHS \geq \frac{9}{(a+b+c)^2}.
\]

Combining with our earlier inequality, we find:

\[
LHS \geq \frac{9}{b(a+b) + c(b+c) + a(c+a)} \Rightarrow LHS \leq \frac{9}{\frac{(a+b+c)^2}{3}} = \frac{27}{(a+b+c)^2}.
\]

Thus, we can safely conclude:

\[
C \leq 27.
\]

### Step 6: Achieving the Bound

By setting \( a = b = c \), we find that the equality holds when \( C = 27 \).

### Conclusion

After rigorous analysis and exploration, we find the largest constant \( C \) such that the inequality holds for all positive \( a, b, c \) is:

\[
\boxed{27}
\]

Thus, our final answer is:

```
'The answer is $C=27$'
```