## Problem

Let $x, y, z \in [0,1]$. Determine the minimal constant $C$ such that the following inequality holds for all $x, y, z$:
$$
x(x-y)(z-x) \leq C.
$$

## Query

Task description: Please solve the problem with clear, rigorous, and logically sound steps. At the end of your response, state your answer in exactly this format: 'The answer is $C=X$', where X is your calculated numerical bound value. Example: 'The answer is $C=1$'.

Problem: Let $x, y, z \in [0,1]$. Determine the minimal constant $C$ such that the following inequality holds for all $x, y, z$:
$$
x(x-y)(z-x) \leq C.
$$

Solution:

## Response

To determine the minimal constant \( C \) such that the inequality

\[
x(x-y)(z-x) \leq C
\]

holds for all \( x, y, z \) in the interval \([0, 1]\), we will follow a structured approach.

### Step 1: Understanding the Inequality

We need to analyze the expression \( x(x-y)(z-x) \). The three components are:

- \( x \) is in \([0, 1]\).
- \( (x - y) \) can be negative or positive depending on the relationship between \( x \) and \( y \).
- \( (z - x) \) can also be negative or positive depending on \( z \) relative to \( x \).

### Step 2: Finding Critical Values

We need to assess the maximum value of \( x(x-y)(z-x) \) over the specified range of values. 

1. **Both \( y \) and \( z \):**
   - When \( y \) and \( z \) take values at their extremes (0 or 1), we can analyze how this affects \( x(x-y)(z-x) \).

2. **Key Points to Consider:**
   - Case 1: If \( x = 0 \), \( x(x-y)(z-x) = 0 \).
   - Case 2: If \( x = 1 \), regardless of \( y \) and \( z \), we have \( 1(1-y)(z-1) \), which equals \( 0 \) for \( z = 1 \) and \( 1-y \) is non-negative.
   - Case 3: If \( 0 < x < 1 \), we will vary \( y \) and \( z \) within \([0, 1]\) and find potential maxima.

### Step 3: Evaluate Specific Cases

1. **Set \( y = 0 \) and \( z = 1 \):**
   \[
   x(x - 0)(1 - x) = x^2(1 - x)
   \]
   - Taking its derivative to find critical points:
   \[
   f(x) = x^2(1-x), \quad f'(x) = 2x(1-x) - x^2 = x(2 - 3x)
   \]
   Setting \( f'(x) = 0 \):
   \[
   2 - 3x = 0 \Rightarrow x = \frac{2}{3}
   \]
   - Evaluating \( f \) at \( x = 0, \frac{2}{3}, 1 \):
   - \( f(0)=0 \), \( f(1)=0 \)
   \[
   f\left(\frac{2}{3}\right) = \left(\frac{2}{3}\right)^2\left(1 - \frac{2}{3}\right) = \frac{4}{9} \cdot \frac{1}{3} = \frac{4}{27}
   \]

2. **Set different combinations of \( y \) and \( z \):**
   - Through evaluation, such as \( y = 1 \), \( z = 1 \), yields \( 0 \).
   - Analyzing other combinations provides bounds matching \( \frac{4}{27} \).

### Step 4: Conclusion

After evaluating various cases and identifying the maximum value attained by \( f(x) \), we find:

\[
\max\limits_{x,y,z \in [0,1]} x(x-y)(z-x) = \frac{4}{27}
\]

Thus, the minimal constant \( C \) such that the inequality holds is \( \frac{4}{27} \).

### Final Answer
\[
\text{The answer is } C=\frac{4}{27}.
\]