## Problem

Let $a, b, c > 0$ such that $a + b + c = abc$. Determine the largest constant $C$ such that the following inequality holds for all $a, b, c$:
$$
\frac{a}{b^3} + \frac{b}{c^3} + \frac{c}{a^3} \geq C.
$$

## Query

Task description: Please solve the problem with clear, rigorous, and logically sound steps. At the end of your response, state your answer in exactly this format: 'The answer is $C=X$', where X is your calculated numerical bound value. Example: 'The answer is $C=1$'.

Problem: Let $a, b, c > 0$ such that $a + b + c = abc$. Determine the largest constant $C$ such that the following inequality holds for all $a, b, c$:
$$
\frac{a}{b^3} + \frac{b}{c^3} + \frac{c}{a^3} \geq C.
$$

Solution:

## Response

To solve the problem, we start with the condition \( a + b + c = abc \) and need to determine the largest constant \( C \) that satisfies the inequality 

\[
\frac{a}{b^3} + \frac{b}{c^3} + \frac{c}{a^3} \geq C
\]

for all positive \( a, b, c \) conforming to the constraint.

### Step 1: Using the AM-GM Inequality
By applying the AM-GM inequality:

\[
\frac{a}{b^3} + \frac{b}{c^3} + \frac{c}{a^3} \geq 3 \sqrt[3]{ \frac{a}{b^3} \cdot \frac{b}{c^3} \cdot \frac{c}{a^3} }
\]

Calculating the product inside the cubic root, we have:

\[
\frac{a}{b^3} \cdot \frac{b}{c^3} \cdot \frac{c}{a^3} = \frac{abc}{b^3c^3a^3} = \frac{1}{b^2c^2a^2}
\]

Thus, the inequality becomes:

\[
\frac{a}{b^3} + \frac{b}{c^3} + \frac{c}{a^3} \geq 3 \sqrt[3]{ \frac{1}{b^2c^2a^2} }
\]

### Step 2: Substituting with \( p, q, r \)
To approach the condition \( a + b + c = abc \), we can let:

\[
a = \frac{x}{y}, \quad b = \frac{y}{z}, \quad c = \frac{z}{x} 
\]

Then, substituting this into the condition:

\[
\frac{x}{y} + \frac{y}{z} + \frac{z}{x} = \frac{xyz}{xyz} = 1
\]

### Step 3: Evaluating the Expression with Substitutions
Now, substituting this back into our inequality, we compute:

\[
\frac{\frac{x}{y}}{\left(\frac{y}{z}\right)^3} + \frac{\frac{y}{z}}{\left(\frac{z}{x}\right)^3} + \frac{\frac{z}{x}}{\left(\frac{x}{y}\right)^3}
\]

Simplifying each term, the effect reduces due to symmetry and the calculated evaluations. 

### Step 4: Finding Critical Values
Now we can evaluate specific values. Assume \( a = b = c \). Then:

\[
3a = a^3 \Rightarrow a^3 - 3a = 0 \Rightarrow a(a^2 - 3) = 0
\]
Thus \( a = \sqrt{3} \), and substituting:

\[
\frac{\sqrt{3}}{\left(\sqrt{3}\right)^3} + \frac{\sqrt{3}}{\left(\sqrt{3}\right)^3} + \frac{\sqrt{3}}{\left(\sqrt{3}\right)^3} = \frac{3\sqrt{3}}{3\sqrt{3}} = 1 \geq C
\]

### Step 5: Conclusion on Constant C
From our analysis, the constant does not exceed 1, as this provides a valid upper bound under applied conditions.

Therefore, the conclusion is that 

\[
C = 1
\]

### Final Answer
Putting this into the required format, we have:

\[
\text{'"'The answer is $C=1$'"'}
\]