## Problem

Let $a, b, c > 0$ be positive real numbers such that $ab + bc + ca = 1$. Consider the following inequality:
$$
a b c\left(a+\sqrt{a^2+1}\right)\left(b+\sqrt{b^2+1}\right)\left(c+\sqrt{c^2+1}\right) \quad () \quad 2.
$$

Determine the correct inequality relation to fill in the blank.

Options:

(A) $\leq$ 

(B) $\geq$

(C) $=$ 

(D) $<$

(E) $>$

(F) None of the above

## Query

Task description: Please solve the problem with clear, rigorous, and logically sound steps. At the end of your response, state your answer in exactly this format: 'The answer is (Letter) Symbol', where Letter is one of the given options. Example: 'The answer is (A) $\leq$'.

Problem: Let $a, b, c > 0$ be positive real numbers such that $ab + bc + ca = 1$. Consider the following inequality:
$$
a b c\left(a+\sqrt{a^2+1}\right)\left(b+\sqrt{b^2+1}\right)\left(c+\sqrt{c^2+1}\right) \quad () \quad 2.
$$

Determine the correct inequality relation to fill in the blank.

Options:

(A) $\leq$ 

(B) $\geq$

(C) $=$ 

(D) $<$

(E) $>$

(F) None of the above

Solution:

## Response

To solve the problem, we begin by analyzing the given inequality:

\[
abc \left( a + \sqrt{a^2 + 1} \right) \left( b + \sqrt{b^2 + 1} \right) \left( c + \sqrt{c^2 + 1} \right) \quad () \quad 2.
\]

### Step 1: Analyze the Expression

We need to estimate the terms \(a + \sqrt{a^2 + 1}\). We can simplify this expression as follows:

\[
a + \sqrt{a^2 + 1} = \sqrt{a^2 + 1} \cdot \left( \frac{a}{\sqrt{a^2 + 1}} + 1 \right).
\]

Using the identity \( \sqrt{x^2 + y^2} \geq \frac{x^2 + y^2}{\sqrt{x^2 + y^2}} \) for non-negative \(x\) and \(y\), we notice that:

\[
a + \sqrt{a^2 + 1} \geq \sqrt{1 + a^2} \, .
\]

### Step 2: Lower Bound Estimation

We can focus on estimating \(abc\):

Utilize the AM-GM inequality on \(ab + ac + bc = 1\):

\[
\frac{ab + bc + ca}{3} \geq \sqrt[3]{(abc)^2}.
\]
So, we have:

\[
\frac{1}{3} \geq \sqrt[3]{(abc)^2} \implies abc \leq \frac{1}{\sqrt{3\sqrt{3}}} \text{ by maximizing } ab, bc, ca.
\]

### Step 3: Combine Inequalities and Formulate

Now, observe:

\[
\left( a + \sqrt{a^2 + 1} \right) \geq \sqrt{1 + a^2} \text{ implies} \left( b + \sqrt{b^2 + 1} \right) \geq \sqrt{1 + b^2}, \quad \left( c + \sqrt{c^2 + 1} \right) \geq \sqrt{1 + c^2}.
\]

By combining:

\[
abcd \left( a + \sqrt{a^2 + 1} \right) \left( b + \sqrt{b^2 + 1} \right) \left( c + \sqrt{c^2 + 1} \right) \text{ grows as } 2\sqrt{3\sqrt{3}} \text{ and therefore must be greater than or equal to \(2\)}.
\]

### Conclusion

After analysis, we can conclude:

\[
abc \left(a + \sqrt{a^2 + 1}\right)\left(b + \sqrt{b^2 + 1}\right)\left(c + \sqrt{c^2 + 1}\right) \geq 2.
\]

Thus, filling in the blank leads us to:

\[
\text{The correct inequality is } \geq.
\]

### Final Answer

Therefore, we state:

'''The answer is (B) $\geq$'''