## Problem

Given $a, b, c \geq 0$, consider the following inequality:
$$
\sum_{cyc} \sqrt{\frac{a+b}{b^2+4bc+c^2}} \quad () \quad \frac{2}{\sqrt{a+2b+4c}}.
$$

Determine the correct inequality relation to fill in the blank.

Options:

(A) $\leq$ 

(B) $\geq$

(C) $=$ 

(D) $<$

(E) $>$

(F) None of the above

## Query

Task description: Please solve the problem with clear, rigorous, and logically sound steps. At the end of your response, state your answer in exactly this format: 'The answer is (Letter) Symbol', where Letter is one of the given options. Example: 'The answer is (A) $\leq$'.

Problem: Given $a, b, c \geq 0$, consider the following inequality:
$$
\sum_{cyc} \sqrt{\frac{a+b}{b^2+4bc+c^2}} \quad () \quad \frac{2}{\sqrt{a+2b+4c}}.
$$

Determine the correct inequality relation to fill in the blank.

Options:

(A) $\leq$ 

(B) $\geq$

(C) $=$ 

(D) $<$

(E) $>$

(F) None of the above

Solution:

## Response

To solve the inequality 

\[
\sum_{cyc} \sqrt{\frac{a+b}{b^2+4bc+c^2}} \quad () \quad \frac{2}{\sqrt{a+2b+4c}},
\]

we need to analyze both sides step by step.

### Step 1: Examining the Left-Hand Side (LHS)

The left-hand side is 

\[
\sum_{cyc} \sqrt{\frac{a+b}{b^2+4bc+c^2}}.
\]

This represents the sum of three terms based on cyclic permutations of \(a, b, c\). Each term in the sum can be simplified and bounded based on non-negativity:

\[
\sqrt{\frac{a+b}{b^2 + 4bc + c^2}}.
\]

### Step 2: Analyzing the Expression Inside the Square Root

For each term:

1. \(a + b\) is non-negative since \(a, b, c \geq 0\).
2. The denominator \(b^2 + 4bc + c^2\) can be rewritten as:

   \[
   b^2 + 4bc + c^2 = (b+c)^2 + 2bc \geq 0.
   \]

Thus, each term \(\sqrt{\frac{a+b}{b^2+4bc+c^2}} \geq 0\).

### Step 3: Finding an Upper Bound for LHS

Now, we make an assumption that helps simplify comparisons. Let's analyze when equality might hold:

Suppose \(a = b = c\). Then each cyclic term becomes:

\[
\sqrt{\frac{2a}{a^2 + 4a^2 + a^2}} = \sqrt{\frac{2a}{6a^2}} = \sqrt{\frac{1}{3a}} = \frac{1}{\sqrt{3a}}.
\]

Thus:

\[
\sum_{cyc} \sqrt{\frac{a+b}{b^2+4bc+c^2}} = 3\cdot \frac{1}{\sqrt{3a}} = \sqrt{3}/a.
\]

Now let's compute the right-hand side (\(RHS\)):

\[
\frac{2}{\sqrt{a+2b+4c}} = \frac{2}{\sqrt{7a}}.
\]

Setting \(x = a\):

For equality:

\[
\sqrt{3}/a \quad ? \quad \frac{2}{\sqrt{7a}}.
\]

Cross Multiply:

\[
\sqrt{21} \quad ? \quad 2\sqrt{3}.
\]

Calculating,

1. \(21 > 4 \cdot 3\), so:

\[
\sqrt{21} > 2 \sqrt{3},
\]

indicating:

\[
\sum_{cyc} \sqrt{\frac{a+b}{b^2 + 4bc + c^2}} > \frac{2}{\sqrt{a+2b+4c}}.
\]

### Conclusion

The inequality holds as:

\[
\sum_{cyc} \sqrt{\frac{a+b}{b^2+4bc+c^2}} \geq \frac{2}{\sqrt{a+2b+4c}}.
\]

Thus, the answer is:

```plaintext
'The answer is (B) â‰¥'
```