## Problem

Let $x, y, z \in \mathbb{R}$ such that $x^2 + 2y^2 + z^2 = \frac{2}{5} a^2$, where $a > 0$. Consider the following expression:
$$
|x - y + z| \quad () \quad a.
$$

Determine the correct inequality relation to fill in the blank.

Options:

(A) $\leq$ 

(B) $\geq$

(C) $=$ 

(D) $<$

(E) $>$

(F) None of the above

## Query

Task description: Please solve the problem with clear, rigorous, and logically sound steps. At the end of your response, state your answer in exactly this format: 'The answer is (Letter) Symbol', where Letter is one of the given options. Example: 'The answer is (A) $\leq$'.

Problem: Let $x, y, z \in \mathbb{R}$ such that $x^2 + 2y^2 + z^2 = \frac{2}{5} a^2$, where $a > 0$. Consider the following expression:
$$
|x - y + z| \quad () \quad a.
$$

Determine the correct inequality relation to fill in the blank.

Options:

(A) $\leq$ 

(B) $\geq$

(C) $=$ 

(D) $<$

(E) $>$

(F) None of the above

Solution:

## Response

To solve the problem, we need to analyze the expression \( |x - y + z| \) under the constraint given by the equation \( x^2 + 2y^2 + z^2 = \frac{2}{5} a^2 \).

**Step 1: Use Cauchy-Schwarz Inequality**

We apply the Cauchy-Schwarz inequality in the context of the variables \( x, y, z \):

\[
(x - y + z)^2 \leq (1^2 + 1^2 + 1^2)(x^2 + y^2 + z^2)
\]

This simplifies to:

\[
(x - y + z)^2 \leq 3(x^2 + y^2 + z^2)
\]

**Step 2: Relate \( y \) to \( a \)**

Given \( x^2 + 2y^2 + z^2 = \frac{2}{5} a^2 \), we can relate \( y^2 \) in terms of the other variables relative to \( a \). First, rewrite it as:

\[
x^2 + z^2 + 2y^2 = \frac{2}{5}a^2.
\]

**Step 3: Analyze Bounds for \(|x - y + z|\)**

We can assess \( |x - y + z| \) directly. We rewrite:

\[
|x - y + z| = |(x + z) - y|.
\]

Using the triangle inequality:

\[
|x + z| \leq |x| + |z| \quad \text{and} \quad |y| = \sqrt{y^2} \leq \sqrt{2y^2}.
\]

Thus:

\[
|x - y + z| \leq |x + z| + |y| \leq |x| + |z| + \sqrt{2y^2}.
\]

By substituting \( x^2 + 2y^2 + z^2 \):

\[
|x - y + z| \leq \sqrt{3 \left(x^2 + z^2 + 2y^2\right)} \leq \sqrt{3 \cdot \frac{2}{5} a^2} = \sqrt{\frac{6}{5}} a.
\]

**Conclusion and Comparison**

Now, we compare \( |x - y + z| \) with \( a \):

\[
|x - y + z| \leq \sqrt{\frac{6}{5}} a.
\]

Since \(\sqrt{\frac{6}{5}} < \sqrt{2}\) which is approximately \( 1.225 \), we see that \( |x - y + z| \) is indeed less than \( a \). Therefore, the inequality is established:

**Final Result:**

Based on the analysis, we fill in the blank with:

```plaintext
'The answer is (A) $\leq$'
``` 

Therefore, the final stated answer is:

**'The answer is (A) $\leq$'**