## Problem

Let $a, b, c > 0$ be positive real numbers such that
$$
\frac{1}{1+a} + \frac{1}{1+b} + \frac{1}{1+c} = 2.
$$

Consider the following inequality:
$$
2(2ab + 3bc + ca) \quad () \quad \sqrt{ab} + \sqrt{bc} + \sqrt{ca}.
$$

Determine the correct inequality relation to fill in the blank.

Options:

(A) $\leq$ 

(B) $\geq$

(C) $=$ 

(D) $<$

(E) $>$

(F) None of the above

## Query

Task description: Please solve the problem with clear, rigorous, and logically sound steps. At the end of your response, state your answer in exactly this format: 'The answer is (Letter) Symbol', where Letter is one of the given options. Example: 'The answer is (A) $\leq$'.

Problem: Let $a, b, c > 0$ be positive real numbers such that
$$
\frac{1}{1+a} + \frac{1}{1+b} + \frac{1}{1+c} = 2.
$$

Consider the following inequality:
$$
2(2ab + 3bc + ca) \quad () \quad \sqrt{ab} + \sqrt{bc} + \sqrt{ca}.
$$

Determine the correct inequality relation to fill in the blank.

Options:

(A) $\leq$ 

(B) $\geq$

(C) $=$ 

(D) $<$

(E) $>$

(F) None of the above

Solution:

## Response

To solve the problem, let's denote \( S = \frac{1}{1+a} + \frac{1}{1+b} + \frac{1}{1+c} \). Given \( S = 2 \), we can manipulate the terms as follows:

1. **Rewrite the Equation**:
   \[
   S = \frac{1}{1+a} + \frac{1}{1+b} + \frac{1}{1+c} \Rightarrow 2 = \frac{(1+b)(1+c) + (1+c)(1+a) + (1+a)(1+b)}{(1+a)(1+b)(1+c)}.
   \]

   Simplifying the numerator:
   \[
   (1+b)(1+c) + (1+c)(1+a) + (1+a)(1+b) = 3 + (ab + ac + bc).
   \]
   Therefore,
   \[
   \frac{3 + (ab + ac + bc)}{(1+a)(1+b)(1+c)} = 2.
   \]

2. **Cross-Multiply**:
   \[
   3 + (ab + ac + bc) = 2(1+a)(1+b)(1+c).
   \]

3. **Expand the Right Side**:
   Expanding \( 2(1+a)(1+b)(1+c) \) yields:
   \[
   2(1 + a + b + c + ab + ac + bc + abc).
   \]
   Thus, we have:
   \[
   3 + ab + ac + bc = 2 + 2a + 2b + 2c + 2ab + 2ac + 2bc + 2abc.
   \] 

4. **Rearranging the Terms**:
   Rearranging gives:
   \[
   1 + ab + ac + bc - 2a - 2b - 2c - 2ab - 2ac - 2bc - 2abc = 0.
   \]
   Which simplifies to:
   \[
   -2(a+b+c+ab+ac+bc) + 1 - 2abc = 0.
   \]

5. **Exploring the Inequality**:
   We need to determine the relationship:
   \[
   2(2ab + 3bc + ca) \quad () \quad \sqrt{ab} + \sqrt{bc} + \sqrt{ca}.
   \]
   We will analyze this using the AM-GM inequality.

6. **Apply the AM-GM Inequality**:
   From AM-GM:
   \[
   \frac{ab + ab + bc + bc + ca}{5} \geq \sqrt[5]{a^2b^2b^2c^2c^2} = \sqrt[5]{a^2b^3c^2}.
   \]
   Therefore:
   \[
   ab + bc + ca \geq 3 \sqrt[3]{abc}.
   \]
   So,
   \[
   2ab + 3bc + ca \geq 2\sqrt[3]{abc} + ...,
   \]
   helps in establishing inequalities between terms.

7. **Final Comparison**:
   Comparing with the right side, using AM-GM:
   \[
   \sqrt{ab} + \sqrt{bc} + \sqrt{ca} \geq \sqrt[3]{abc} + ...,
   \]
   leads us to conclude that the left side dominates under certain conditions.

After evaluating through careful steps and using AM-GM inequality, the result appears consistent:

Thus, based on comparisons and the usage of the inequalities, the answer is:
```
'The answer is (A) â‰¤'
```