## Problem

Let $a, b, c$ be positive numbers such that $a^2 + b^2 + c^2 = 3$. Consider the following inequality:
$$
\frac{b+c}{a^2} + \frac{c+a}{b^2} + \frac{a+b}{c^2} \quad () \quad 3\left(\frac{1}{a} + \frac{1}{b} + \frac{1}{c} - a b c\right).
$$

Determine the correct inequality relation to fill in the blank.

Options:

(A) $\leq$ 

(B) $\geq$

(C) $=$ 

(D) $<$

(E) $>$

(F) None of the above

## Query

Task description: Please solve the problem with clear, rigorous, and logically sound steps. At the end of your response, state your answer in exactly this format: 'The answer is (Letter) Symbol', where Letter is one of the given options. Example: 'The answer is (A) $\leq$'.

Problem: Let $a, b, c$ be positive numbers such that $a^2 + b^2 + c^2 = 3$. Consider the following inequality:
$$
\frac{b+c}{a^2} + \frac{c+a}{b^2} + \frac{a+b}{c^2} \quad () \quad 3\left(\frac{1}{a} + \frac{1}{b} + \frac{1}{c} - a b c\right).
$$

Determine the correct inequality relation to fill in the blank.

Options:

(A) $\leq$ 

(B) $\geq$

(C) $=$ 

(D) $<$

(E) $>$

(F) None of the above

Solution:

## Response

To solve the problem, we need to analyze the given inequality involving the positive numbers \(a\), \(b\), and \(c\) subject to the constraint \(a^2 + b^2 + c^2 = 3\).

### Step 1: Analyze both sides of the inequality

The inequality we need to evaluate is:

\[
\frac{b+c}{a^2} + \frac{c+a}{b^2} + \frac{a+b}{c^2} \quad \_ \quad 3\left(\frac{1}{a} + \frac{1}{b} + \frac{1}{c} - a b c\right).
\]

**Left Side:**

We denote:

\[
L = \frac{b+c}{a^2} + \frac{c+a}{b^2} + \frac{a+b}{c^2}
\]

Using the Cauchy-Schwarz inequality, we can relate the left-hand side to the right-hand side:

\[
L = \sum_{\text{cyc}} \frac{b+c}{a^2} \geq \frac{(b+c+c+a+a+b)^2}{a^2 + b^2 + c^2} = \frac{(2(a+b+c))^2}{3}.
\]

**Right Side:**

Let’s analyze:

\[
R = 3\left(\frac{1}{a} + \frac{1}{b} + \frac{1}{c} - abc\right).
\]

Using the AM-HM inequality:

\[
\frac{a+b+c}{3} \geq \frac{3}{\frac{1}{a} + \frac{1}{b} + \frac{1}{c}} \implies \frac{1}{a} + \frac{1}{b} + \frac{1}{c} \geq \frac{9}{a+b+c}.
\]

### Step 2: Testing specific values

Let’s test with \( a=b=c=1 \):

1. We find that \( a^2 + b^2 + c^2 = 3 \) holds.
2. Calculate both sides:
   - Left Side:
   \[
   L = \frac{1+1}{1^2} + \frac{1+1}{1^2} + \frac{1+1}{1^2} = 2 + 2 + 2 = 6
   \]
   - Right Side:
   \[
   R = 3\left(1 + 1 + 1 - 1\right) = 3 \times 2 = 6.
   \]

### Conclusion

Thus, \( L = R \) for \( a = b = c = 1 \) implies that:

\[
\frac{b+c}{a^2} + \frac{c+a}{b^2} + \frac{a+b}{c^2} = 3\left(\frac{1}{a} + \frac{1}{b} + \frac{1}{c} - abc\right).
\]

Now, since equality can hold for \( a, b, c \) being equal, and using various properties of inequalities, we conclude that the initial inequality can hold as equal, both for the AM-HM and Cauchy-Schwarz inequalities.

Hence, the answer is:

```plaintext
'TThe answer is (C) ='`
```