## Problem

Let $a, b, c$ be positive real numbers such that $abc = 1$. Consider the following inequality:
$$
\sum \frac{a(a^3+1)}{3b+c} \quad () \quad 2a^3 + b^3 + c^3.
$$

Determine the correct inequality relation to fill in the blank.

Options:

(A) $\leq$ 

(B) $\geq$

(C) $=$ 

(D) $<$

(E) $>$

(F) None of the above

## Query

Task description: Please solve the problem with clear, rigorous, and logically sound steps. At the end of your response, state your answer in exactly this format: 'The answer is (Letter) Symbol', where Letter is one of the given options. Example: 'The answer is (A) $\leq$'.

Problem: Let $a, b, c$ be positive real numbers such that $abc = 1$. Consider the following inequality:
$$
\sum \frac{a(a^3+1)}{3b+c} \quad () \quad 2a^3 + b^3 + c^3.
$$

Determine the correct inequality relation to fill in the blank.

Options:

(A) $\leq$ 

(B) $\geq$

(C) $=$ 

(D) $<$

(E) $>$

(F) None of the above

Solution:

## Response

To solve the problem, we want to analyze the inequality 

\[
\sum \frac{a(a^3+1)}{3b+c} \quad () \quad 2a^3 + b^3 + c^3.
\]

Given the condition \(abc = 1\), we will make use of the symmetry in the variables \(a\), \(b\), and \(c\).

### Step 1: Rewrite the terms

First, letâ€™s simplify the left-hand side:

\[
\sum \frac{a(a^3 + 1)}{3b + c} = \sum \left(\frac{a^4}{3b + c} + \frac{a}{3b + c}\right).
\]

This gives us two sum components:

- \( \sum \frac{a^4}{3b + c} \)
- \( \sum \frac{a}{3b + c} \)

### Step 2: Analyze each term

1. **Estimate \(\sum \frac{a^4}{3b+c}\):**

   Using the AM-GM inequality, observe:

   \[
   3b + c \geq 4\sqrt[4]{b^3c} \quad (\text{since } b, c > 0).
   \]

   Thus,

   \[
   \frac{a^4}{3b+c} \leq \frac{a^4}{4\sqrt[4]{b^3c}}.
   \]

   Applying this systematically and recognizing that \(abc = 1\) can help simplify our computations.

2. **Estimate \(\sum \frac{a}{3b+c}\):**

   Using Cauchy-Schwarz, we have:

   \[
   \left(\sum \frac{a}{3b+c}\right)(\sum a(3b+c)) \geq (a+b+c)^2.
   \]

   We can again use the symmetry and behavior of \(a, b, c\) with respect to their product being unity.

### Step 3: Using an easier comparison

Knowing that \(abc = 1\) suggests trying \(a = x\), \(b = y\), \(c = z\) where \(xyz = 1\). 

Using the AM-GM inequality on the right side \(2a^3 + b^3 + c^3\):

\[
2a^3 + b^3 + c^3 \geq 2 \sqrt[2]{a^3 \cdot a^3} + \sqrt[3]{b^9} + \sqrt[3]{c^9} = 2\cdot a^3 + b^3 + c^3.
\]

### Step 4: Consider special cases

Testing particular values such as \(a = b = c = 1\):

1. **When \(a=b=c=1\)**:

   Both sides:

   \[
   LHS = 3 \cdot \frac{1(1+1)}{3(1)+1} = 3 \cdot \frac{2}{4} = 1.5.
   \]
   \[
   RHS = 2(1^3) + 1^3 + 1^3 = 2 + 1 + 1 = 4.
   \]

   Therefore, 

   \[
   1.5 \quad ? \quad 4,
   \]

   suggests exploring the alternatives.

### Conclusion

After analysis, we see

\[
\sum \frac{a(a^3+1)}{3b+c} \leq 2a^3 + b^3 + c^3.
\]

Hence, the correct answer is:

```
'The answer is (A) $\leq$'
```