## Problem

Let $a, b, c > 0$ such that $a+b+c=2$ and $a^2+b^2+c^2=2$. Determine the minimal constant $C$ such that the following inequality holds for all $a, b, c$ satisfying the given constraints:
$$
a b c \leq C.
$$

## Query

Task description: Please solve the problem with clear, rigorous, and logically sound steps. At the end of your response, state your answer in exactly this format: 'The answer is $C=X$', where X is your calculated numerical bound value. Example: 'The answer is $C=1$'.

Problem: Let $a, b, c > 0$ such that $a+b+c=2$ and $a^2+b^2+c^2=2$. Determine the minimal constant $C$ such that the following inequality holds for all $a, b, c$ satisfying the given constraints:
$$
a b c \leq C.
$$

Solution:

## Response

To solve the problem, we will use the given conditions \( a+b+c=2 \) and \( a^2+b^2+c^2=2 \) to derive a relationship involving \( abc \).

### Step 1: Analyze the Conditions

1. The first condition \( a+b+c = 2 \) shows that the sum of the variables is a constant.
2. The second condition \( a^2 + b^2 + c^2 = 2 \) allows us to relate this to \( abc \) using Cauchy-Schwarz Inequality.

### Step 2: Use Cauchy-Schwarz Inequality

Using the identity:
\[
(a+b+c)^2 = a^2 + b^2 + c^2 + 2(ab + ac + bc)
\]
we plug in our known values:
\[
2^2 = 2 + 2(ab + ac + bc)
\]
This simplifies to:
\[
4 = 2 + 2(ab + ac + bc) \implies 2 = 2(ab + ac + bc) \implies ab + ac + bc = 1
\]

### Step 3: Application of AM-GM Inequality

By applying the Arithmetic Mean-Geometric Mean (AM-GM) Inequality to the positive numbers \( a, b, c \), we get:
\[
\frac{a+b+c}{3} \geq \sqrt[3]{abc}
\]
From our conditions, \( a+b+c = 2 \):
\[
\frac{2}{3} \geq \sqrt[3]{abc} \implies abc \leq \left(\frac{2}{3}\right)^3 = \frac{8}{27}
\]

### Step 4: Check For Equality

Next, to find if this bound can be attained, let's assume \( a = b \) and find \( c \). Using \( a + b + c = 2 \) and \( a^2 + b^2 + c^2 = 2 \):
- Let \( a = b = x \) and \( c = 2 - 2x \).
  
Then:
\[
x^2 + x^2 + (2 - 2x)^2 = 2 \implies 2x^2 + 4 - 8x + 4x^2 = 2 \implies 6x^2 - 8x + 2 = 0
\]
Using the quadratic formula:
\[
x = \frac{8 \pm \sqrt{(-8)^2 - 4 \cdot 6 \cdot 2}}{2 \cdot 6} = \frac{8 \pm \sqrt{64 - 48}}{12} = \frac{8 \pm \sqrt{16}}{12} = \frac{8 \pm 4}{12}
\]
This gives:
\[
x = 1 \quad \text{or} \quad x = \frac{1}{3}
\]
### Case of \( x = 1 \):
If \( x = 1 \), then \( c = 0 \), which is not allowed since \( a, b, c > 0 \).

### Case of \( x = \frac{1}{3} \):
If \( x = \frac{1}{3} \):
- Then \( a = b = c = \frac{1}{3} \).
- Thus:
\[
abc = \left(\frac{1}{3}\right)^3 = \frac{1}{27}
\]

### Conclusion

Since \( abc \leq \frac{8}{27} \) holds, and we found \( abc = \frac{1}{27} \) for \( a = b = c = \frac{1}{3} \), the minimal constant \( C \) for which the inequality \( abc \leq C \) holds is:

\[
C = \frac{8}{27}
\]

Thus, the final answer is:
```
'The answer is $C=\frac{8}{27}$'
```