## Problem

Let $a, b, c > 0$ be positive real numbers such that $a + b + c = 1$. Consider the following inequality:
$$
5(a^2 + b^2 + c^2) \quad () \quad 6(a^3 + b^3 + c^3) + 1.
$$

Determine the correct inequality relation to fill in the blank.

Options:

(A) $\leq$ 

(B) $\geq$

(C) $=$ 

(D) $<$

(E) $>$

(F) None of the above

## Query

Task description: Please solve the problem with clear, rigorous, and logically sound steps. At the end of your response, state your answer in exactly this format: 'The answer is (Letter) Symbol', where Letter is one of the given options. Example: 'The answer is (A) $\leq$'.

Problem: Let $a, b, c > 0$ be positive real numbers such that $a + b + c = 1$. Consider the following inequality:
$$
5(a^2 + b^2 + c^2) \quad () \quad 6(a^3 + b^3 + c^3) + 1.
$$

Determine the correct inequality relation to fill in the blank.

Options:

(A) $\leq$ 

(B) $\geq$

(C) $=$ 

(D) $<$

(E) $>$

(F) None of the above

Solution:

## Response

To solve the problem, we need to analyze the given inequality:

\[
5(a^2 + b^2 + c^2) \quad () \quad 6(a^3 + b^3 + c^3) + 1
\]

where \(a + b + c = 1\) and \(a, b, c > 0\).

### Step 1: Use the Cauchy-Schwarz Inequality
According to the Cauchy-Schwarz inequality:

\[
(a^2 + b^2 + c^2)(1 + 1 + 1) \geq (a + b + c)^2
\]

This gives us:
\[
3(a^2 + b^2 + c^2) \geq (a + b + c)^2 = 1^2 = 1 \implies a^2 + b^2 + c^2 \geq \frac{1}{3}
\]

Multiplying by 5:
\[
5(a^2 + b^2 + c^2) \geq 5 \cdot \frac{1}{3} = \frac{5}{3}
\]

### Step 2: Express \(a^3 + b^3 + c^3\) in terms of \(a + b + c\) and \(a^2 + b^2 + c^2\)
Using the identity:
\[
a^3 + b^3 + c^3 = (a+b+c)(a^2 + b^2 + c^2 - ab - ac - bc) + 3abc
\]
and recalling that \(ab + ac + bc = \frac{(a + b + c)^2 - (a^2 + b^2 + c^2)}{2}\).

### Step 3: Calculate \(a^3 + b^3 + c^3\)
Given \(a + b + c = 1\):
\[
6(a^3 + b^3 + c^3) = 6 \left(1(a^2 + b^2 + c^2 - ab - ac - bc) + 3abc\right)
\]

We know:
\[
ab + ac + bc = \frac{1 - (a^2 + b^2 + c^2)}{2}
\]
This implies:
\[
6(a^3 + b^3 + c^3) = 6\left( a^2 + b^2 + c^2 - \frac{1 - (a^2 + b^2 + c^2)}{2} + 3abc \right)
\]

### Step 4: Compare the two sides for specific cases
1. Assuming \(a = b = c = \frac{1}{3}\):
   - \( a^2 + b^2 + c^2 = 3\left(\frac{1}{3}\right)^2 = \frac{1}{3}\)
   - \( a^3 + b^3 + c^3 = 3\left(\frac{1}{3}\right)^3 = \frac{1}{9}\)

Insert these into both sides:
- Left Side: \( 5 \cdot \frac{1}{3} = \frac{5}{3} \)
- Right Side: \( 6 \cdot \frac{1}{9} + 1 = \frac{2}{3} + 1 = \frac{5}{3} \)

So for this case, we have:
\[
5(a^2 + b^2 + c^2) = 6(a^3 + b^3 + c^3) + 1
\]

### Step 5: Conclusion
The calculations show that the inequality holds as an equality for \(a = b = c = \frac{1}{3}\).

Thus, we conclude that the correct relationship to fill in the blank is:
\[
=
\]

### Final Answer
The answer is \( "The answer is (C) =" \)