## Problem

Let $a, b, c$ be positive real numbers such that $a + b + c = 1$. Consider the following inequality:
$$
a \sqrt[3]{1+b-c} + b \sqrt[3]{1+c-a} + c \sqrt[3]{1+a-b} \quad () \quad 1.
$$

Determine the correct inequality relation to fill in the blank.

Options:

(A) $\leq$ 

(B) $\geq$

(C) $=$ 

(D) $<$

(E) $>$

(F) None of the above

## Query

Task description: Please solve the problem with clear, rigorous, and logically sound steps. At the end of your response, state your answer in exactly this format: 'The answer is (Letter) Symbol', where Letter is one of the given options. Example: 'The answer is (A) $\leq$'.

Problem: Let $a, b, c$ be positive real numbers such that $a + b + c = 1$. Consider the following inequality:
$$
a \sqrt[3]{1+b-c} + b \sqrt[3]{1+c-a} + c \sqrt[3]{1+a-b} \quad () \quad 1.
$$

Determine the correct inequality relation to fill in the blank.

Options:

(A) $\leq$ 

(B) $\geq$

(C) $=$ 

(D) $<$

(E) $>$

(F) None of the above

Solution:

## Response

To solve the inequality given the constraints \( a + b + c = 1 \) where \( a, b, c > 0 \), we need to investigate the expression:

\[
S = a \sqrt[3]{1 + b - c} + b \sqrt[3]{1 + c - a} + c \sqrt[3]{1 + a - b}.
\]

**Step 1: Substitute for \(c\)**

Since \( c = 1 - a - b \), we can rewrite \( S \) as follows:

\[
S = a \sqrt[3]{1 + b - (1 - a - b)} + b \sqrt[3]{1 + (1 - a - b) - a} + (1 - a - b) \sqrt[3]{1 + a - b}.
\]

This simplifies to:

\[
S = a \sqrt[3]{a + 2b} + b \sqrt[3]{2 - a - b} + (1 - a - b) \sqrt[3]{1 + a - b}.
\]

**Step 2: Analyze the Limit Case**

To explore the behavior of \( S \), consider the case when \( a = b = c = \frac{1}{3} \):

\[
S = \frac{1}{3} \sqrt[3]{1 + \frac{1}{3} - \frac{1}{3}} + \frac{1}{3} \sqrt[3]{1 + \frac{1}{3} - \frac{1}{3}} + \frac{1}{3} \sqrt[3]{1 + \frac{1}{3} - \frac{1}{3}}.
\]
\[
= \frac{1}{3} \sqrt[3]{1} + \frac{1}{3} \sqrt[3]{1} + \frac{1}{3} \sqrt[3]{1} = 1.
\]

In this case, \( S = 1 \).

**Step 3: Test Other Cases**

Next, we investigate extreme cases such as \( a \to 1, b \to 0, c \to 0 \):

\[
S \to 1 \cdot \sqrt[3]{1 + 0 - 0} = 1.
\]

Simulating the extreme conditions \( a \to 1, b \to 0, c \to 0 \) or permuting other combinations leads to:

1. \( S < 1 \) when either \( 0 < a < 1 \) and both \( b \) or \( c \) are small.
2. The general case suggests \( S \) remains less than or equal to \( 1 \).

By Jensen's inequality, since the function \( f(x) = x^{1/3} \) is concave on the positive numbers, applying it gives:

\[
S \leq f(a + b + c) = f(1) = 1.
\]

Thus, concluding:

\[
S \leq 1.
\]

**Conclusion:**

From the analysis and testing, the relationship that always holds is \( S \leq 1 \).

Hence, the final answer is:

```plaintext
'TThe answer is (A) $\leq$'
```