## Problem

Let $a, b, c > 0$ be positive real numbers such that $a + b + c = 3$. Consider the following inequality:
$$
a^2 + 4b^2 + 4b + 8c \quad () \quad 7 + 2\sqrt{2(b^2 + c^2)} + 4\sqrt{bc}.
$$

Determine the correct inequality relation to fill in the blank.

Options:

(A) $\leq$ 

(B) $\geq$

(C) $=$ 

(D) $<$

(E) $>$

(F) None of the above

## Query

Task description: Please solve the problem with clear, rigorous, and logically sound steps. At the end of your response, state your answer in exactly this format: 'The answer is (Letter) Symbol', where Letter is one of the given options. Example: 'The answer is (A) $\leq$'.

Problem: Let $a, b, c > 0$ be positive real numbers such that $a + b + c = 3$. Consider the following inequality:
$$
a^2 + 4b^2 + 4b + 8c \quad () \quad 7 + 2\sqrt{2(b^2 + c^2)} + 4\sqrt{bc}.
$$

Determine the correct inequality relation to fill in the blank.

Options:

(A) $\leq$ 

(B) $\geq$

(C) $=$ 

(D) $<$

(E) $>$

(F) None of the above

Solution:

## Response

To solve the inequality involving positive real numbers \(a, b, c\) such that \(a + b + c = 3\), we need to analyze the expression:

\[
E = a^2 + 4b^2 + 4b + 8c
\]
in relation to:

\[
F = 7 + 2\sqrt{2(b^2 + c^2)} + 4\sqrt{bc}.
\]

### Step 1: Rewrite the expressions
Since \(a + b + c = 3\), we can express \(c = 3 - a - b\). Thus, substituting \(c\) in \(E\) gives:

\[
E = a^2 + 4b^2 + 4b + 8(3 - a - b) = a^2 + 4b^2 + 4b + 24 - 8a - 8b.
\]

### Step 2: Combine like terms
Reorganizing \(E\) leads to:

\[
E = a^2 - 8a + 4b^2 - 4b + 24.
\]

### Step 3: Calculate \(b^2 + c^2\) and \(bc\)
We need to work with the components of \(F\):

1. **Finding \(b^2 + c^2\)**:
   \[
   c = 3 - a - b \implies b^2 + c^2 = b^2 + (3 - a - b)^2 = b^2 + (9 - 6(a+b) + a^2 + 2ab).
   \]

   Simplifying gives:

   \[
   = 9 - 6(a + b) + a^2 + 3b - 2ab.
   \]

2. **Finding \(bc\)**:
   \[
   bc = b(3 - a - b) = 3b - ab - b^2.
   \]

### Step 4: Analyzing the inequality

We now need to determine if \(E\) is less than, greater than, or equal to \(F\). 

We will evaluate special cases to understand the relationship between \(E\) and \(F\).

### Case 1: \(a = 0\), \(b = c = 1.5\)

Calculating \(E\):

\[
E = 0^2 + 4(1.5)^2 + 4(1.5) + 8(1.5) = 0 + 4 \cdot 2.25 + 6 + 12 = 9 + 6 + 12 = 27.
\]

Calculating \(F\):

\[
F = 7 + 2\sqrt{2((1.5)^2 + (1.5)^2)} + 4\sqrt{(1.5)(1.5)} = 7 + 2\sqrt{2(4.5)} + 4(1.5).
\]
\[
= 7 + 2\sqrt{9} + 6 = 7 + 6 + 6 = 19.
\]

Here \(E = 27\) and \(F = 19\), so \(E \geq F\).

### Case 2: \(a = 1\), \(b = 1\), \(c = 1\)

Calculating \(E\):

\[
E = 1^2 + 4(1)^2 + 4(1) + 8(1) = 1 + 4 + 4 + 8 = 17.
\]

Calculating \(F\):

\[
F = 7 + 2\sqrt{2(1^2 + 1^2)} + 4\sqrt{1 \cdot 1} = 7 + 2\sqrt{4} + 4 = 7 + 4 + 4 = 15.
\]

Again, \(E \geq F\).

### Conclusion

Given multiple evaluations showing \(E\) consistently greater than \(F\) under the given constraints, we deduce that:

\[
E \geq F.
\]

Thus, the correct inequality relation is:

``'The answer is (B) $\geq$''``