## Problem

Let $a, b, c \neq 0$ be non-zero real numbers such that $a^2 + b^2 + c^2 = 2(ab + bc + ca)$. Consider the following expression:
$$
(a+b+c)\left(\frac{1}{2a}+\frac{1}{3b}+\frac{1}{c}\right) \quad () \quad 14.
$$

Determine the correct inequality relation to fill in the blank.

Options:

(A) $\leq$ 

(B) $\geq$

(C) $=$ 

(D) $<$

(E) $>$

(F) None of the above

## Query

Task description: Please solve the problem with clear, rigorous, and logically sound steps. At the end of your response, state your answer in exactly this format: 'The answer is (Letter) Symbol', where Letter is one of the given options. Example: 'The answer is (A) $\leq$'.

Problem: Let $a, b, c \neq 0$ be non-zero real numbers such that $a^2 + b^2 + c^2 = 2(ab + bc + ca)$. Consider the following expression:
$$
(a+b+c)\left(\frac{1}{2a}+\frac{1}{3b}+\frac{1}{c}\right) \quad () \quad 14.
$$

Determine the correct inequality relation to fill in the blank.

Options:

(A) $\leq$ 

(B) $\geq$

(C) $=$ 

(D) $<$

(E) $>$

(F) None of the above

Solution:

## Response

To solve the given problem, we start by analyzing the condition provided: 

**Step 1: Analyze the Condition**

The equation \( a^2 + b^2 + c^2 = 2(ab + bc + ca) \) can be rearranged as follows:

\[
a^2 + b^2 + c^2 - 2(ab + bc + ca) = 0
\]
This implies:

\[
\frac{1}{2}(a-b)^2 + \frac{1}{2}(b-c)^2 + \frac{1}{2}(c-a)^2 = 0
\]
For this sum of squares to be zero, each individual square must be zero. Therefore:

\[
a = b = c
\]

**Step 2: Substitute into the Expression**

Now, substituting \( a = b = c \) into the expression \( (a+b+c)\left(\frac{1}{2a}+\frac{1}{3b}+\frac{1}{c}\right) \):

Let \( a = b = c = x \). Then,

\[
a + b + c = 3x
\]

and substituting into the fraction, we have:

\[
\frac{1}{2a} + \frac{1}{3b} + \frac{1}{c} = \frac{1}{2x} + \frac{1}{3x} + \frac{1}{x}
\]

Finding a common denominator gives:

\[
\frac{1}{2x} + \frac{1}{3x} + \frac{1}{x} = \frac{3}{6x} + \frac{2}{6x} + \frac{6}{6x} = \frac{11}{6x}
\]

**Step 3: Calculate the Whole Expression**

Substituting into the whole expression, we have:

\[
(3x)\left(\frac{11}{6x}\right) = \frac{33}{6} = 5.5
\]

**Step 4: Compare to 14**

Now we compare this value to 14:

\[
5.5 < 14
\]

**Conclusion**

From our calculations, we established that:

\[
(a+b+c)\left(\frac{1}{2a}+\frac{1}{3b}+\frac{1}{c}\right) < 14
\]

Thus, the correct inequality relation to fill in the blank is:

**The answer is (D) $<$**.