## Problem

Let $a, b > 0$ be positive real numbers such that $a^2 + b^2 + 3 = 4ab$. Consider the following inequality:
$$
2\sqrt{2ab} - \frac{1}{2}a - b \quad () \quad \frac{1}{2}.
$$

Determine the correct inequality relation to fill in the blank.

Options:

(A) $\leq$ 

(B) $\geq$

(C) $=$ 

(D) $<$

(E) $>$

(F) None of the above

## Query

Task description: Please solve the problem with clear, rigorous, and logically sound steps. At the end of your response, state your answer in exactly this format: 'The answer is (Letter) Symbol', where Letter is one of the given options. Example: 'The answer is (A) $\leq$'.

Problem: Let $a, b > 0$ be positive real numbers such that $a^2 + b^2 + 3 = 4ab$. Consider the following inequality:
$$
2\sqrt{2ab} - \frac{1}{2}a - b \quad () \quad \frac{1}{2}.
$$

Determine the correct inequality relation to fill in the blank.

Options:

(A) $\leq$ 

(B) $\geq$

(C) $=$ 

(D) $<$

(E) $>$

(F) None of the above

Solution:

## Response

To solve the problem, let's first rewrite the given condition from the problem statement.

**Step 1: Rearrange the equation**

The equation provided is:

\[
a^2 + b^2 + 3 = 4ab
\]

Rearranging it gives:

\[
a^2 - 4ab + b^2 + 3 = 0
\]

This resembles a quadratic equation in terms of \(a\) (or \(b\)). 

**Step 2: Apply the Quadratic Formula**

Rearranging to have terms involving \(a\):

\[
a^2 - 4ab + b^2 + 3 = 0
\]

The standard form \(Ax^2 + Bx + C = 0\) suggests we can use the quadratic formula \(a = \frac{-B \pm \sqrt{B^2 - 4AC}}{2A}\).

Setting up terms:
- \(A = 1\)
- \(B = -4b\)
- \(C = b^2 + 3\)

Calculating the discriminant:
\[
D = (-4b)^2 - 4(1)(b^2 + 3) = 16b^2 - 4b^2 - 12 = 12b^2 - 12 = 12(b^2 - 1)
\]

For \(D\) to be non-negative, we need:
\[
b^2 - 1 \geq 0 \implies b \geq 1 \quad (\text{since } b > 0)
\]

**Step 3: Analyze the Inequality**

We need to evaluate:

\[
2\sqrt{2ab} - \frac{1}{2}a - b \quad \text{ and } \frac{1}{2}
\]

Let's reorganize and simplify the left-hand side:
Setting \(x = a\) and \(y=b\), the expression can be rewritten as:

\[
2\sqrt{2xy} - \frac{1}{2}x - y
\]

**Step 4: Substitute and Analyze**

Now let's find \(2\sqrt{2ab}\):
From earlier, we can consider positive \(a, b\) satisfying the original equation. Substituting back and using \(a = kb\), we get bounds:

Assume \(k = 1\) for symmetry, yielding:
\[
2\sqrt{2bb} = 2\sqrt{2b^2} = 2b\sqrt{2}
\]
From the inequality we need:
\[
2b\sqrt{2} - \frac{1}{2}b - b < \frac{1}{2}
\]

Rearranging to find the bounds:
\[
2\sqrt{2}b - \frac{3}{2}b < \frac{1}{2}
\]

This gives:
\[
(2\sqrt{2} - \frac{3}{2})b < \frac{1}{2}
\]

**Step 5: Analyze coefficients**

Now we compare:
The number \(2\sqrt{2} \approx 2.828\), and \(\frac{3}{2} = 1.5\). Thus,
\[
(2\sqrt{2}-\frac{3}{2}) \approx 2.828 - 1.5 = 1.328
\]

Whether this holds for a range of \(b\) (which can vary based on \(x/y\) symmetry, but returning appropriations of positive reals).

Thus, simplifying:

1. **Conclusion**: 
The behavior around estimates show:
\[
\text{Left} < \text{Right} \implies 2\sqrt{2ab} - \frac{1}{2}a - b < \frac{1}{2}
\]

So filling in the blank leads to:

**Final Answer**: 
```
The answer is (D) <
```